Port system D example calculus

theories/Examples/Mu/PolarizedSystemD.v
@@ -1,16 +1,46 @@
 From OGS Require Import Prelude.
-From OGS.Utils Require Import Psh Rel Ctx.
+From OGS.Utils Require Import Psh Rel.
+From OGS.Ctx Require Import All Ctx Covering Subset.
 From OGS.ITree Require Import Event ITree Eq Delay Structure Properties.
-From OGS.OGS Require Import Soundness.
-Set Equations Transparent.
- 
-Variant pol : Type := pos | neg .
-Derive NoConfusion for pol.
+From OGS.OGS Require Import Soundness. 
+(*|
+In this file we instanciate our OGS construction with the fully-dual polarized mu-mu-tilde
+calculus 'System D' from P. Downen & Z. Ariola. The presentation may be slightly unusual
+as we go for one-sided sequent. The only real divergence from the original calculus
+is the addition of a restricted form of recursion, making the language non-normalizing. 
 
+Types
+=====
+
+Type have polarities, basically whether their values are CBV-biased
+or CBN-biased
+|*)
+Variant pol : Type := pos | neg .
+(*| .. coq:: none |*)
+Derive NoConfusion for pol.
+(*
 Equations pneg : pol -> pol :=
   pneg pos := neg ;
   pneg neg := pos .
+*)
+(*|
+Syntax of types. We have a fully dual type system with:
 
+- `0`, positive void (no constructor),
+- `⊤`, negative unit (no destructor),
+- `⊥`, negative void (one trivial destructor),
+- `1`, positive unit (one trivial constructor),
+- `A ⊗ B`, positive product (pairs with pattern-matching),
+- `A ⅋ B`, negative sum (one binary destructor),
+- `A ⊕ B`, positive sum (usual coproduct with injections),
+- `A & B`, negative product (usual product with projections),
+- `↓ A`, positive shift (thunking),
+- `↑ A`, negative shift ('returners'),
+- `⊖ A`, positive negation (approximately continuations accepting an `A`),
+- `¬ A`, negative negation (approximately refutations of `A`).
+
+We opt for an explicit treatment of polarity, by indexing the family of types.
+|*)
 Inductive ty0 : pol -> Type :=
 | Zer : ty0 pos
 | Top : ty0 neg
@@ -25,13 +55,11 @@ Inductive ty0 : pol -> Type :=
 | NegP : ty0 neg -> ty0 pos
 | NegN : ty0 pos -> ty0 neg
 .
-
 (*| .. coq:: none |*)
-Derive NoConfusion for ty0.
+Derive Signature NoConfusion NoConfusionHom for ty0.
 Declare Scope ty_scope.
 Delimit Scope ty_scope with ty.
 Bind Scope ty_scope with ty0.
-
 (*||*)
 Notation "0" := (Zer) : ty_scope .
 Notation "1" := (One) : ty_scope .
@@ -43,141 +71,200 @@ Notation "A ⊕ B" := (Or A B) (at level 40) : ty_scope.
 Notation "A & B" := (And A B) (at level 40) : ty_scope.
 Notation "↓ A" := (ShiftP A) (at level 40) : ty_scope.
 Notation "↑ A" := (ShiftN A) (at level 40) : ty_scope.
-Notation "⊖ A" := (NegP A) (at level 40) : ty_scope .
-Notation "¬ A" := (NegN A) (at level 40) : ty_scope .
-Notation "A → B" := (¬ A ⅋ B)%ty (at level 40) : ty_scope.
-
-
+Notation "⊖ A" := (NegP A) (at level 5) : ty_scope .
+Notation "¬ A" := (NegN A) (at level 5) : ty_scope .
+(*|
+As hinted above, we go for one-sided sequents. This enables to have only one context
+instead of two, simplifying the theory of substitution. On the flip-side, as we still
+need two kinds of variables, the 'normal' ones and the co-variables, our contexts will
+not contain bare types but side-annotated types. A variable of type `A` will thus be
+stored as `\`-A` in the context while a co-variable of type `A` will be stored as `\`-A`. 
+|*)
 Variant ty : Type :=
 | VTy {p} : ty0 p -> ty
 | KTy {p} : ty0 p -> ty
 .
-
-Derive NoConfusion for ty.
+(*| .. coq:: none |*)
+Derive NoConfusion NoConfusionHom for ty.
 Bind Scope ty_scope with ty.
-Notation "'t+' t" := (VTy t) (at level 20) : ty_scope .
-Notation "'t-' t" := (KTy t) (at level 20) : ty_scope .
 Open Scope ty_scope.
+(*||*)
+Notation "'`+' t" := (VTy t) (at level 5) : ty_scope .
+Notation "'`-' t" := (KTy t) (at level 5) : ty_scope .
 
 Equations t_neg : ty -> ty :=
-  t_neg (t+ a) := t- a ;
-  t_neg (t- a) := t+ a .
-
+  t_neg `+a := `-a ;
+  t_neg `-a := `+a .
+Notation "a †" := (t_neg a) (at level 5) : ty_scope.
+(*|
+Finally we define contexts as backward lists of side-annotated types.
+|*)
 Definition t_ctx : Type := Ctx.ctx ty.
+(*| .. coq:: none |*)
 Bind Scope ctx_scope with t_ctx.
+(*|
+Terms
+=====
 
+We define the well-typed syntax of the language with 3 mutually defined syntactic
+categories: terms, weak head-normal forms and states ('language configurations' in
+the paper).
+
+Nothing should be too surprising. A first notable point is that by choosing to have an
+explicit notion of 'side' of a variable, we can have a single construct
+for both mu and mu-tilde. A second notable point is our new slightly exotic `RecL` and
+`RecR` constructions. They allow arbitrary recursion at co-terms of positive types and
+at terms of negative types. These polarity restrictions allow us to have minimal
+disruption of the evaluation rules. 
+|*)
 Inductive term : t_ctx -> ty -> Type :=
-| Mu {Γ A} : state (Γ ▶ t_neg A) -> term Γ A
-| RecL {Γ} {A : ty0 pos} : term (Γ ▶ t- A) (t- A) -> term Γ (t- A)
-| RecR {Γ} {A : ty0 neg} : term (Γ ▶ t+ A) (t+ A) -> term Γ (t+ A)
+| Mu {Γ A} : state (Γ ▶ₓ A†) -> term Γ A
+| RecL {Γ} {A : ty0 pos} : term (Γ ▶ₓ `-A) `-A -> term Γ `-A
+| RecR {Γ} {A : ty0 neg} : term (Γ ▶ₓ `+A) `+A -> term Γ `+A
 | Whn {Γ A} : whn Γ A -> term Γ A
 with whn : t_ctx -> ty -> Type :=
 | Var {Γ A} : Γ ∋ A -> whn Γ A
-| ZerL {Γ} : whn Γ (t- 0)
-| TopR {Γ} : whn Γ (t+ ⊤)
-| OneR {Γ} : whn Γ (t+ 1)
-| OneL {Γ} : state Γ -> whn Γ (t- 1)
-| BotR {Γ} : state Γ -> whn Γ (t+ ⊥)
-| BotL {Γ} : whn Γ (t- ⊥)
-| TenR {Γ A B} : whn Γ (t+ A) -> whn Γ (t+ B) -> whn Γ (t+ (A ⊗ B))
-| TenL {Γ A B} : state (Γ ▶ t+ A ▶ t+ B) -> whn Γ (t- (A ⊗ B))
-| ParR {Γ A B} : state (Γ ▶ t- A ▶ t- B) -> whn Γ (t+ (A ⅋ B))
-| ParL {Γ A B} : whn Γ (t- A) -> whn Γ (t- B) -> whn Γ (t- (A ⅋ B))
-| OrR1 {Γ A B} : whn Γ (t+ A) -> whn Γ (t+ (A ⊕ B))
-| OrR2 {Γ A B} : whn Γ (t+ B) -> whn Γ (t+ (A ⊕ B))
-| OrL {Γ A B} : state (Γ ▶ t+ A) -> state (Γ ▶ t+ B) -> whn Γ (t- (A ⊕ B))
-| AndR {Γ A B} : state (Γ ▶ t- A) -> state (Γ ▶ t- B) -> whn Γ (t+ (A & B))
-| AndL1 {Γ A B} : whn Γ (t- A) -> whn Γ (t- (A & B))
-| AndL2 {Γ A B} : whn Γ (t- B) -> whn Γ (t- (A & B))
-| ShiftPR {Γ A} : term Γ (t+ A) -> whn Γ (t+ (↓ A))
-| ShiftPL {Γ A} : state (Γ ▶ t+ A) -> whn Γ (t- (↓ A))
-| ShiftNR {Γ A} : state (Γ ▶ t- A) -> whn Γ (t+ (↑ A))
-| ShiftNL {Γ A} : term Γ (t- A) -> whn Γ (t- (↑ A))
-| NegPR {Γ A} : whn Γ (t- A) -> whn Γ (t+ (⊖ A))
-| NegPL {Γ A} : state (Γ ▶ t- A) -> whn Γ (t- (⊖ A))
-| NegNR {Γ A} : state (Γ ▶ t+ A) -> whn Γ (t+ (¬ A))
-| NegNL {Γ A} : whn Γ (t+ A) -> whn Γ (t- (¬ A))
+| ZerL {Γ} : whn Γ `-0
+| TopR {Γ} : whn Γ `+⊤
+| OneR {Γ} : whn Γ `+1
+| OneL {Γ} : state Γ -> whn Γ `-1
+| BotR {Γ} : state Γ -> whn Γ `+⊥
+| BotL {Γ} : whn Γ `-⊥
+| TenR {Γ A B} : whn Γ `+A -> whn Γ `+B -> whn Γ `+(A ⊗ B)
+| TenL {Γ A B} : state (Γ ▶ₓ `+A ▶ₓ `+B) -> whn Γ `-(A ⊗ B)
+| ParR {Γ A B} : state (Γ ▶ₓ `-A ▶ₓ `-B) -> whn Γ `+(A ⅋ B)
+| ParL {Γ A B} : whn Γ `-A -> whn Γ `-B -> whn Γ `-(A ⅋ B)
+| OrR1 {Γ A B} : whn Γ `+A -> whn Γ `+(A ⊕ B)
+| OrR2 {Γ A B} : whn Γ `+B -> whn Γ `+(A ⊕ B)
+| OrL {Γ A B} : state (Γ ▶ₓ `+A) -> state (Γ ▶ₓ `+B) -> whn Γ `-(A ⊕ B)
+| AndR {Γ A B} : state (Γ ▶ₓ `-A) -> state (Γ ▶ₓ `-B) -> whn Γ `+(A & B)
+| AndL1 {Γ A B} : whn Γ `-A -> whn Γ `-(A & B)
+| AndL2 {Γ A B} : whn Γ `-B -> whn Γ `-(A & B)
+| ShiftPR {Γ A} : term Γ `+A -> whn Γ `+(↓ A)
+| ShiftPL {Γ A} : state (Γ ▶ₓ `+A) -> whn Γ `-(↓ A)
+| ShiftNR {Γ A} : state (Γ ▶ₓ `-A) -> whn Γ `+(↑ A)
+| ShiftNL {Γ A} : term Γ `-A -> whn Γ `-(↑ A)
+| NegPR {Γ A} : whn Γ `-A -> whn Γ `+(⊖ A)
+| NegPL {Γ A} : state (Γ ▶ₓ `-A) -> whn Γ `-(⊖ A)
+| NegNR {Γ A} : state (Γ ▶ₓ `+A) -> whn Γ `+(¬ A)
+| NegNL {Γ A} : whn Γ `+A -> whn Γ `-(¬ A)
 with state : t_ctx -> Type :=
-| Cut {Γ} p {A : ty0 p} : term Γ (t+ A) -> term Γ (t- A) -> state Γ
+| Cut {Γ} p {A : ty0 p} : term Γ `+A -> term Γ `-A -> state Γ
 .
 
+Definition Cut' {Γ A} : term Γ A -> term Γ A† -> state Γ :=
+  match A with
+  | `+A => fun t1 t2 => Cut _ t1 t2
+  | `-A => fun t1 t2 => Cut _ t2 t1
+  end .
+(*| .. coq:: none |*)
+Derive Signature NoConfusion NoConfusionHom for term.
+Derive Signature NoConfusion NoConfusionHom for whn.
+Derive Signature NoConfusion NoConfusionHom for state.
+
+(*|
+Values are not exactly weak head-normal forms, but depend on the polarity of the type.
+As positive types have CBV evaluation, their values are weak head-normal forms, but their
+co-values (evaluation contexts) are just any co-term (context) as they are delayed anyways.
+Dually for negative types, values are delayed hence can be any term while co-values must
+be weak head-normal form contexts.
+|*)
 Equations val : t_ctx -> ty -> Type :=
-  val Γ (@VTy pos A) := whn Γ (t+ A) ;
-  val Γ (@KTy pos A) := term Γ (t- A) ;
-  val Γ (@VTy neg A) := term Γ (t+ A) ;
-  val Γ (@KTy neg A) := whn Γ (t- A) .
+  val Γ (@VTy pos A) := whn Γ `+A ;
+  val Γ (@KTy pos A) := term Γ `-A ;
+  val Γ (@VTy neg A) := term Γ `+A ;
+  val Γ (@KTy neg A) := whn Γ `-A .
+Arguments val _ _ /.
+(*|
+We provide a 'smart-constructor' for variables, embedding variables in values.
+|*)
+Equations var : c_var ⇒₁ val :=
+  var _ (@VTy pos _) i := Var i ;
+  var _ (@KTy pos _) i := Whn (Var i) ;
+  var _ (@VTy neg _) i := Whn (Var i) ;
+  var _ (@KTy neg _) i := Var i .
+#[global] Arguments var {Γ} [x] / i.
+(*|
+Renaming
+========
 
-Equations s_var {Γ} : has Γ ⇒ᵢ val Γ :=
-  s_var (@VTy pos _) i := Var i ;
-  s_var (@KTy pos _) i := Whn (Var i) ;
-  s_var (@VTy neg _) i := Whn (Var i) ;
-  s_var (@KTy neg _) i := Var i .
+Without surprise parallel renaming goes by a big mutual induction, shifting the renaming
+apropriately while going under binders. Note the use of the internal substitution hom
+to type it.
+|*)
+Equations t_rename : term ⇒₁ ⟦ c_var , term ⟧₁ :=
+  t_rename _ _ (Mu c)    _ f := Mu (s_rename _ c _ (r_shift1 f)) ;
+  t_rename _ _ (RecL t)  _ f := RecL (t_rename _ _ t _ (r_shift1 f)) ;
+  t_rename _ _ (RecR t)  _ f := RecR (t_rename _ _ t _ (r_shift1 f)) ;
+  t_rename _ _ (Whn v)   _ f := Whn (w_rename _ _ v _ f) ;
+with w_rename : whn ⇒₁ ⟦ c_var , whn ⟧₁ :=
+  w_rename _  _ (Var i)       _ f := Var (f _ i) ;
+  w_rename _  _ (ZerL)        _ f := ZerL ;
+  w_rename _  _ (TopR)        _ f := TopR ;
+  w_rename _  _ (OneR)        _ f := OneR ;
+  w_rename _  _ (OneL c)      _ f := OneL (s_rename _ c _ f) ;
+  w_rename _  _ (BotR c)      _ f := BotR (s_rename _ c _ f) ;
+  w_rename _  _ (BotL)        _ f := BotL ;
+  w_rename _  _ (TenR v1 v2)  _ f := TenR (w_rename _ _ v1 _ f) (w_rename _ _ v2 _ f) ;
+  w_rename _  _ (TenL c)      _ f := TenL (s_rename _ c _ (r_shift2 f)) ;
+  w_rename _  _ (ParR c)      _ f := ParR (s_rename _ c _ (r_shift2 f)) ;
+  w_rename _  _ (ParL k1 k2)  _ f := ParL (w_rename _ _ k1 _ f) (w_rename _ _ k2 _ f) ;
+  w_rename _  _ (OrR1 v)      _ f := OrR1 (w_rename _ _ v _ f) ;
+  w_rename _  _ (OrR2 v)      _ f := OrR2 (w_rename _ _ v _ f) ;
+  w_rename _  _ (OrL c1 c2)   _ f := OrL (s_rename _ c1 _ (r_shift1 f))
+                                         (s_rename _ c2 _ (r_shift1 f)) ;
+  w_rename _  _ (AndR c1 c2)  _ f := AndR (s_rename _ c1 _ (r_shift1 f))
+                                          (s_rename _ c2 _ (r_shift1 f)) ;
+  w_rename _  _ (AndL1 k)     _ f := AndL1 (w_rename _ _ k _ f) ;
+  w_rename _  _ (AndL2 k)     _ f := AndL2 (w_rename _ _ k _ f) ;
+  w_rename _  _ (ShiftPR t)   _ f := ShiftPR (t_rename _ _ t _ f) ;
+  w_rename _  _ (ShiftPL c)   _ f := ShiftPL (s_rename _ c _ (r_shift1 f)) ;
+  w_rename _  _ (ShiftNR c)   _ f := ShiftNR (s_rename _ c _ (r_shift1 f)) ;
+  w_rename _  _ (ShiftNL t)   _ f := ShiftNL (t_rename _ _ t _ f) ;
+  w_rename _  _ (NegPR k)     _ f := NegPR (w_rename _ _ k _ f) ;
+  w_rename _  _ (NegPL c)     _ f := NegPL (s_rename _ c _ (r_shift1 f)) ;
+  w_rename _  _ (NegNR c)     _ f := NegNR (s_rename _ c _ (r_shift1 f)) ;
+  w_rename _  _ (NegNL v)     _ f := NegNL (w_rename _ _ v _ f) ;
+with s_rename : state ⇒₀ ⟦ c_var , state ⟧₀ :=
+  s_rename _ (Cut _ v k) _ f := Cut _ (t_rename _ _ v _ f) (t_rename _ _ k _ f) .
+(*|
+We extend it to values...
+|*)
+Equations v_rename : val ⇒₁ ⟦ c_var , val ⟧₁ :=
+  v_rename _ (@VTy pos a) := w_rename _ _ ;
+  v_rename _ (@KTy pos a) := t_rename _ _ ;
+  v_rename _ (@VTy neg a) := t_rename _ _ ;
+  v_rename _ (@KTy neg a) := w_rename _ _ .
+(*|
+... provide a couple infix notations...
+|*)
+Notation "t ₜ⊛ᵣ r" := (t_rename _ _ t _ r%asgn) (at level 14).
+Notation "w `ᵥ⊛ᵣ r" := (w_rename _ _ w _ r%asgn) (at level 14).
+Notation "v ᵥ⊛ᵣ r" := (v_rename _ _ v _ r%asgn) (at level 14).
+Notation "s ₛ⊛ᵣ r" := (s_rename _ s _ r%asgn) (at level 14).
 
-Definition r_shift3 {Γ Δ : t_ctx} {a b c} (f : Γ ⊆ Δ) : (Γ ▶ a ▶ b ▶ c) ⊆ (Δ ▶ a ▶ b ▶ c)
-  := r_shift (r_shift (r_shift f)).
-
-Equations t_rename {Γ Δ} : Γ ⊆ Δ -> term Γ ⇒ᵢ term Δ :=
-  t_rename f _ (Mu c)    := Mu (s_rename (r_shift f) c) ;
-  t_rename f _ (RecL t)  := RecL (t_rename (r_shift f) _ t) ;
-  t_rename f _ (RecR t)  := RecR (t_rename (r_shift f) _ t) ;
-  t_rename f _ (Whn v)   := Whn (w_rename f _ v) ;
-with w_rename {Γ Δ} : Γ ⊆ Δ -> whn Γ ⇒ᵢ whn Δ :=
-  w_rename f _ (Var i)       := Var (f _ i) ;
-  w_rename f _ (ZerL)        := ZerL ;
-  w_rename f _ (TopR)        := TopR ;
-  w_rename f _ (OneR)        := OneR ;
-  w_rename f _ (OneL c)      := OneL (s_rename f c) ;
-  w_rename f _ (BotR c)      := BotR (s_rename f c) ;
-  w_rename f _ (BotL)        := BotL ;
-  w_rename f _ (TenR v1 v2)  := TenR (w_rename f _ v1) (w_rename f _ v2) ;
-  w_rename f _ (TenL c)      := TenL (s_rename (r_shift2 f) c) ;
-  w_rename f _ (ParR c)      := ParR (s_rename (r_shift2 f) c) ;
-  w_rename f _ (ParL k1 k2)  := ParL (w_rename f _ k1) (w_rename f _ k2) ;
-  w_rename f _ (OrR1 v)      := OrR1 (w_rename f _ v) ;
-  w_rename f _ (OrR2 v)      := OrR2 (w_rename f _ v) ;
-  w_rename f _ (OrL c1 c2)   := OrL (s_rename (r_shift f) c1) (s_rename (r_shift f) c2) ;
-  w_rename f _ (AndR c1 c2)  := AndR (s_rename (r_shift f) c1) (s_rename (r_shift f) c2) ;
-  w_rename f _ (AndL1 k)     := AndL1 (w_rename f _ k) ;
-  w_rename f _ (AndL2 k)     := AndL2 (w_rename f _ k) ;
-  w_rename f _ (ShiftPR t)   := ShiftPR (t_rename f _ t) ;
-  w_rename f _ (ShiftPL c)   := ShiftPL (s_rename (r_shift f) c) ;
-  w_rename f _ (ShiftNR c)   := ShiftNR (s_rename (r_shift f) c) ;
-  w_rename f _ (ShiftNL t)   := ShiftNL (t_rename f _ t) ;
-  w_rename f _ (NegPR k)     := NegPR (w_rename f _ k) ;
-  w_rename f _ (NegPL c)     := NegPL (s_rename (r_shift f) c) ;
-  w_rename f _ (NegNR c)     := NegNR (s_rename (r_shift f) c) ;
-  w_rename f _ (NegNL v)     := NegNL (w_rename f _ v) ;
-with s_rename {Γ Δ} : Γ ⊆ Δ -> state Γ -> state Δ :=
-   s_rename f (Cut _ v k) := Cut _ (t_rename f _ v) (t_rename f _ k) .
-
-Equations v_rename {Γ Δ} : Γ ⊆ Δ -> val Γ ⇒ᵢ val Δ :=
-  v_rename f (@VTy pos a) v := w_rename f _ v ;
-  v_rename f (@KTy pos a) t := t_rename f _ t ;
-  v_rename f (@VTy neg a) t := t_rename f _ t ;
-  v_rename f (@KTy neg a) k := w_rename f _ k .
-
-Definition a_ren {Γ1 Γ2 Γ3} : Γ2 ⊆ Γ3 -> Γ1 =[val]> Γ2 -> Γ1 =[val]> Γ3 :=
-  fun f g _ i => v_rename f _ (g _ i) .
-
-Definition t_shift {Γ} [y] : term Γ ⇒ᵢ term (Γ ▶ y)  := @t_rename _ _ r_pop.
-Definition w_shift {Γ} [y] : whn Γ ⇒ᵢ whn (Γ ▶ y)  := @w_rename _ _ r_pop.
-Definition s_shift {Γ} [y] : state Γ -> state (Γ ▶ y) := @s_rename _ _ r_pop.
-Definition v_shift {Γ} [y] : val Γ ⇒ᵢ val (Γ ▶ y)    := @v_rename _ _ r_pop.
-Definition v_shift2 {Γ} [y z] : val Γ ⇒ᵢ val (Γ ▶ y ▶ z)  := @v_rename _ _ (r_pop ⊛ᵣ r_pop).
-Definition v_shift3 {Γ} [x y z] : val Γ ⇒ᵢ val (Γ ▶ x ▶ y ▶ z)  := @v_rename _ _ (r_pop ⊛ᵣ r_pop ⊛ᵣ r_pop).
-
-Definition a_shift {Γ Δ} [y] (a : Γ =[val]> Δ) : (Γ ▶ y) =[val]> (Δ ▶ y) :=
-  a_append (fun _ i => v_shift _ (a _ i)) (s_var _ top).
-
-Definition a_shift2 {Γ Δ} [y z] (a : Γ =[val]> Δ) : (Γ ▶ y ▶ z) =[val]> (Δ ▶ y ▶ z) :=
-  a_append (a_append (fun _ i => v_shift2 _ (a _ i)) (s_var _ (pop (top)))) (s_var _ top).
-
-Definition a_shift3 {Γ Δ} [x y z] (a : Γ =[val]> Δ) : (Γ ▶ x ▶ y ▶ z) =[val]> (Δ ▶ x ▶ y ▶ z) :=
-  a_append (a_append (a_append (fun _ i => v_shift3 _ (a _ i))
-                        (s_var _ (pop (pop top))))
-              (s_var _ (pop top)))
-    (s_var _ top).
-
+(*|
+... and extend it to assignments.
+|*)
+Definition a_ren {Γ1 Γ2 Γ3} : Γ1 =[val]> Γ2 -> Γ2 ⊆ Γ3 -> Γ1 =[val]> Γ3 :=
+  fun f g _ i => v_rename _ _ (f _ i) _ g .
+Arguments a_ren {_ _ _} _ _ _ _ /.
+Notation "a ⊛ᵣ r" := (a_ren a r%asgn) (at level 14) : asgn_scope.
+(*|
+The following bunch of shifting functions will help us define parallel substitution.
+|*)
+Definition t_shift1 {Γ y} : term Γ ⇒ᵢ term (Γ ▶ₓ y)  := fun _ t => t ₜ⊛ᵣ r_pop.
+Definition w_shift1 {Γ y} : whn Γ ⇒ᵢ whn (Γ ▶ₓ y)    := fun _ w => w `ᵥ⊛ᵣ r_pop.
+Definition s_shift1 {Γ y} : state Γ -> state (Γ ▶ₓ y) := fun s => s ₛ⊛ᵣ r_pop.
+Definition v_shift1 {Γ y} : val Γ ⇒ᵢ val (Γ ▶ₓ y)    := fun _ v => v ᵥ⊛ᵣ r_pop.
+Definition v_shift2 {Γ y z} : val Γ ⇒ᵢ val (Γ ▶ₓ y ▶ₓ z) := fun _ v => v ᵥ⊛ᵣ (r_pop ᵣ⊛ r_pop).
+Definition a_shift1 {Γ Δ} [y] (a : Γ =[val]> Δ) : (Γ ▶ₓ y) =[val]> (Δ ▶ₓ y)
+  := [ fun _ i => v_shift1 _ (a _ i) ,ₓ var top ].
+Definition a_shift2 {Γ Δ} [y z] (a : Γ =[val]> Δ) : (Γ ▶ₓ y ▶ₓ z) =[val]> (Δ ▶ₓ y ▶ₓ z)
+  := [ [ fun _ i => v_shift2 _ (a _ i) ,ₓ var (pop top) ] ,ₓ var top ].
+(*|
+We also define two embeddings linking the various syntactical categories.
+|*)
 Equations v_of_w {Γ} : whn Γ ⇒ᵢ val Γ :=
   v_of_w (@VTy pos _) v := v ;
   v_of_w (@KTy pos _) u := Whn u ;
@@ -190,114 +277,135 @@ Equations t_of_v {Γ} : val Γ ⇒ᵢ term Γ :=
   t_of_v (@VTy neg _) u := u ;
   t_of_v (@KTy neg _) k := Whn k .
 
-Equations t_subst {Γ Δ} : Γ =[val]> Δ -> term Γ ⇒ᵢ term Δ :=
-  t_subst f _ (Mu c)    := Mu (s_subst (a_shift f) c) ;
-  t_subst f _ (RecL t)  := RecL (t_subst (a_shift f) _ t) ;
-  t_subst f _ (RecR t)  := RecR (t_subst (a_shift f) _ t) ;
-  t_subst f _ (Whn v)   := t_of_v _ (w_subst f _ v) ;
-with w_subst {Γ Δ} : Γ =[val]> Δ -> whn Γ ⇒ᵢ val Δ :=
-  w_subst f _ (Var i)      := f _ i ;
-  w_subst f _ (ZerL)       := Whn ZerL ;
-  w_subst f _ (TopR)       := Whn TopR ;
-  w_subst f _ (OneR)       := OneR ;
-  w_subst f _ (OneL c)     := Whn (OneL (s_subst f c)) ;
-  w_subst f _ (BotR c)     := Whn (BotR (s_subst f c)) ;
-  w_subst f _ (BotL)       := BotL ;
-  w_subst f _ (TenR v1 v2) := TenR (w_subst f _ v1) (w_subst f _ v2) ;
-  w_subst f _ (TenL c)     := Whn (TenL (s_subst (a_shift2 f) c)) ;
-  w_subst f _ (ParR c)     := Whn (ParR (s_subst (a_shift2 f) c)) ;
-  w_subst f _ (ParL k1 k2) := ParL (w_subst f _ k1) (w_subst f _ k2) ;
-  w_subst f _ (OrR1 v)     := OrR1 (w_subst f _ v) ;
-  w_subst f _ (OrR2 v)     := OrR2 (w_subst f _ v) ;
-  w_subst f _ (OrL c1 c2)  := Whn (OrL (s_subst (a_shift f) c1) (s_subst (a_shift f) c2)) ;
-  w_subst f _ (AndR c1 c2) := Whn (AndR (s_subst (a_shift f) c1) (s_subst (a_shift f) c2)) ;
-  w_subst f _ (AndL1 k)    := AndL1 (w_subst f _ k) ;
-  w_subst f _ (AndL2 k)    := AndL2 (w_subst f _ k) ;
-  w_subst f _ (ShiftPR t)  := ShiftPR (t_subst f _ t) ;
-  w_subst f _ (ShiftPL c)  := Whn (ShiftPL (s_subst (a_shift f) c)) ;
-  w_subst f _ (ShiftNR c)  := Whn (ShiftNR (s_subst (a_shift f) c)) ;
-  w_subst f _ (ShiftNL t)  := ShiftNL (t_subst f _ t) ;
-  w_subst f _ (NegPR k)    := NegPR (w_subst f _ k) ;
-  w_subst f _ (NegPL c)    := Whn (NegPL (s_subst (a_shift f) c)) ;
-  w_subst f _ (NegNR c)    := Whn (NegNR (s_subst (a_shift f) c)) ;
-  w_subst f _ (NegNL v)    := NegNL (w_subst f _ v) ;
-with s_subst {Γ Δ} : Γ =[val]> Δ -> state Γ -> state Δ :=
-   s_subst f (Cut p v k) := Cut p (t_subst f _ v) (t_subst f _ k) .
+(*|
+Substitution
+============
 
-Equations v_subst {Γ Δ} : Γ =[val]> Δ -> val Γ ⇒ᵢ val Δ :=
-  v_subst f (@VTy pos a) v := w_subst f _ v ;
-  v_subst f (@KTy pos a) t := t_subst f _ t ;
-  v_subst f (@VTy neg a) t := t_subst f _ t ;
-  v_subst f (@KTy neg a) k := w_subst f _ k .
+Having done with renaming, we reapply the same pattern to define parallel substitution.
+Note that substituting a weak head-normal form with values may not yield a weak
+head-normal form, but only a value!
+|*)
+Equations t_subst : term ⇒₁ ⟦ val , term ⟧₁ :=
+  t_subst _ _ (Mu c)    _ f := Mu (s_subst _ c _ (a_shift1 f)) ;
+  t_subst _ _ (RecL t)  _ f := RecL (t_subst _ _ t _ (a_shift1 f)) ;
+  t_subst _ _ (RecR t)  _ f := RecR (t_subst _ _ t _ (a_shift1 f)) ;
+  t_subst _ _ (Whn v)   _ f := t_of_v _ (w_subst _ _ v _ f) ;
+with w_subst : whn ⇒₁ ⟦ val , val ⟧₁ :=
+  w_subst _  _ (Var i)      _ f := f _ i ;
+  w_subst _  _ (ZerL)       _ f := Whn ZerL ;
+  w_subst _  _ (TopR)       _ f := Whn TopR ;
+  w_subst _  _ (OneR)       _ f := OneR ;
+  w_subst _  _ (OneL c)     _ f := Whn (OneL (s_subst _ c _ f)) ;
+  w_subst _  _ (BotR c)     _ f := Whn (BotR (s_subst _ c _ f)) ;
+  w_subst _  _ (BotL)       _ f := BotL ;
+  w_subst _  _ (TenR v1 v2) _ f := TenR (w_subst _ _ v1 _ f) (w_subst _ _ v2 _ f) ;
+  w_subst _  _ (TenL c)     _ f := Whn (TenL (s_subst _ c _ (a_shift2 f))) ;
+  w_subst _  _ (ParR c)     _ f := Whn (ParR (s_subst _ c _ (a_shift2 f))) ;
+  w_subst _  _ (ParL k1 k2) _ f := ParL (w_subst _ _ k1 _ f) (w_subst _ _ k2 _ f) ;
+  w_subst _  _ (OrR1 v)     _ f := OrR1 (w_subst _ _ v _ f) ;
+  w_subst _  _ (OrR2 v)     _ f := OrR2 (w_subst _ _ v _ f) ;
+  w_subst _  _ (OrL c1 c2)  _ f := Whn (OrL (s_subst _ c1 _ (a_shift1 f))
+                                            (s_subst _ c2 _ (a_shift1 f))) ;
+  w_subst _  _ (AndR c1 c2) _ f := Whn (AndR (s_subst _ c1 _ (a_shift1 f))
+                                             (s_subst _ c2 _ (a_shift1 f))) ;
+  w_subst _  _ (AndL1 k)    _ f := AndL1 (w_subst _ _ k _ f) ;
+  w_subst _  _ (AndL2 k)    _ f := AndL2 (w_subst _ _ k _ f) ;
+  w_subst _  _ (ShiftPR t)  _ f := ShiftPR (t_subst _ _ t _ f) ;
+  w_subst _  _ (ShiftPL c)  _ f := Whn (ShiftPL (s_subst _ c _ (a_shift1 f))) ;
+  w_subst _  _ (ShiftNR c)  _ f := Whn (ShiftNR (s_subst _ c _ (a_shift1 f))) ;
+  w_subst _  _ (ShiftNL t)  _ f := ShiftNL (t_subst _ _ t _ f) ;
+  w_subst _  _ (NegPR k)    _ f := NegPR (w_subst _ _ k _ f) ;
+  w_subst _  _ (NegPL c)    _ f := Whn (NegPL (s_subst _ c _ (a_shift1 f))) ;
+  w_subst _  _ (NegNR c)    _ f := Whn (NegNR (s_subst _ c _ (a_shift1 f))) ;
+  w_subst _  _ (NegNL v)    _ f := NegNL (w_subst _ _ v _ f) ;
+with s_subst : state ⇒₀ ⟦ val , state ⟧₀ :=
+   s_subst _ (Cut p v k) _ f := Cut p (t_subst _ _ v _ f) (t_subst _ _ k _ f) .
 
-Definition a_comp {Γ1 Γ2 Γ3} : Γ2 =[val]> Γ3 -> Γ1 =[val]> Γ2 -> Γ1 =[val]> Γ3 :=
-  fun f g _ i => v_subst f _ (g _ i) .
+Notation "t `ₜ⊛ a" := (t_subst _ _ t _ a%asgn) (at level 30).
+Notation "w `ᵥ⊛ a" := (w_subst _ _ w _ a%asgn) (at level 30).
 
-Definition ass1 {Γ a} (v : val Γ a) : (Γ ▶ a) =[val]> Γ := a_append s_var v .
+Equations v_subst : val ⇒₁ ⟦ val , val ⟧₁ :=
+  v_subst _ (@VTy pos a) v _ f := v `ᵥ⊛ f ;
+  v_subst _ (@KTy pos a) t _ f := t `ₜ⊛ f ;
+  v_subst _ (@VTy neg a) t _ f := t `ₜ⊛ f ;
+  v_subst _ (@KTy neg a) k _ f := k `ᵥ⊛ f .
+(*|
+With this in hand we can instanciate the relevant part of substitution monoid and module
+structures for values and states. This will provide us with the missing infix notations.
+|*)
+#[global] Instance val_m_monoid : subst_monoid val :=
+  {| v_var := @var ; v_sub := v_subst |} .
+#[global] Instance state_module : subst_module val state :=
+  {| c_sub := s_subst |} .
+(*|
+We now define helpers for substituting the top one or top two variables from a context.
+|*)
+Definition asgn1 {Γ a} (v : val Γ a) : (Γ ▶ₓ a) =[val]> Γ := [ var ,ₓ v ] .
+Definition asgn2 {Γ a b} (v1 : val Γ a) (v2 : val Γ b) : (Γ ▶ₓ a ▶ₓ b) =[val]> Γ
+  := [ [ var ,ₓ v1 ] ,ₓ v2 ].
 
-Definition t_subst1 {Γ a b} u v := t_subst (@ass1 Γ a v) b u.
-Definition w_subst1 {Γ a b} u v := w_subst (@ass1 Γ a v) b u.
-Definition v_subst1 {Γ a b} u v := v_subst (@ass1 Γ a v) b u.
-Definition s_subst1 {Γ a} u v := s_subst (@ass1 Γ a v) u.
+Arguments asgn1 {_ _} & _.
+Arguments asgn2 {_ _ _} & _ _.
 
-Equations ass2 {Γ a b} (v1 : val Γ a) (v2 : val Γ b) : (Γ ▶ a ▶ b) =[val]> Γ :=
-  ass2 v1 v2 _ top           := v2 ;
-  ass2 v1 v2 _ (pop top)     := v1 ;
-  ass2 v1 v2 _ (pop (pop i)) := s_var _ i .
+Notation "₁[ v ]" := (asgn1 v).
+Notation "₂[ v1 , v2 ]" := (asgn2 v1 v2).
+(*|
+Observations
+============
 
-Equations ass3 {Γ a b c} (v1 : val Γ a) (v2 : val Γ b) (v3 : val Γ c)
-  : (Γ ▶ a ▶ b ▶ c) =[val]> Γ :=
-  ass3 v1 v2 v3 _ top                 := v3 ;
-  ass3 v1 v2 v3 _ (pop top)           := v2 ;
-  ass3 v1 v2 v3 _ (pop (pop top))     := v1 ;
-  ass3 v1 v2 v3 _ (pop (pop (pop i))) := s_var _ i .
-
-Definition s_subst2 {Γ a b} s v1 v2 := s_subst (@ass2 Γ a b v1 v2) s .
-Definition s_subst3 {Γ a b c} s v1 v2 v3 := s_subst (@ass3 Γ a b c v1 v2 v3) s .
-
-Notation "u ₜ/[ v ]" := (t_subst1 u v) (at level 50, left associativity).
-Notation "u ᵥ/[ v ]" := (v_subst1 u v) (at level 50, left associativity).
-Notation "u ₛ/[ v ]" := (s_subst1 u v) (at level 50, left associativity).
-Notation "u ₛ/[ v , w ]" := (s_subst2 u v w) (at level 50, left associativity).
-Notation "u /ₛ[ v , w , z ]" := (s_subst3 u v w z) (at level 50, left associativity).
-
+When defining (co-)patterns, we will enforce a form of focalisation, where no negative
+variables are introduced. In this context, 'negative' is a new notion applying to
+side-annotated types, mixing both type polarity and side annotation: a side-annotated
+variable is positive iff it is a positive variable or a negative co-variable.
+|*)
 Equations is_neg : ty -> SProp :=
   is_neg (@VTy pos a) := sEmpty ;
   is_neg (@KTy pos a) := sUnit ;
   is_neg (@VTy neg a) := sUnit ;
   is_neg (@KTy neg a) := sEmpty .
-
+(*|
+We define negative types as a subset of types, and negative contexts as a subset of
+contexts. Our generic infrastructure for contexts and variables really shines here as
+the type of variables in a negative context is convertible to the type of variables in
+the underlying context. See `Ctx/Subset.v`. 
+|*)
 Definition neg_ty : Type := sigS is_neg.
 Definition neg_coe : neg_ty -> ty := sub_elt.
 Global Coercion neg_coe : neg_ty >-> ty.
 
-Definition neg_ctx : Type := ctx_s is_neg.
+Definition neg_ctx : Type := ctxS ty t_ctx is_neg.
 Definition neg_c_coe : neg_ctx -> ctx ty := sub_elt.
 Global Coercion neg_c_coe : neg_ctx >-> ctx.
-
+(*| .. coq:: none |*)
 Bind Scope ctx_scope with neg_ctx.
 Bind Scope ctx_scope with ctx.
-
+(*|
+We can now define patterns...
+|*)
 Inductive pat : ty -> Type :=
-| PVarP (A : ty0 neg) : pat (t+ A)
-| PVarN (A : ty0 pos) : pat (t- A)
-| POne : pat (t+ 1)
-| PBot : pat (t- ⊥)
-| PTen {A B} : pat (t+ A) -> pat (t+ B) -> pat (t+ (A ⊗ B))
-| PPar {A B} : pat (t- A) -> pat (t- B) -> pat (t- (A ⅋ B))
-| POr1 {A B} : pat (t+ A) -> pat (t+ (A ⊕ B))
-| POr2 {A B} : pat (t+ B) -> pat (t+ (A ⊕ B))
-| PAnd1 {A B} : pat (t- A) -> pat (t- (A & B))
-| PAnd2 {A B} : pat (t- B) -> pat (t- (A & B))
-| PShiftP A : pat (t+ (↓ A))
-| PShiftN A : pat (t- (↑ A))
-| PNegP {A} : pat (t- A) -> pat (t+ (⊖ A))
-| PNegN {A} : pat (t+ A) -> pat (t- (¬ A))
+| PVarP (A : ty0 neg) : pat `+A
+| PVarN (A : ty0 pos) : pat `-A
+| POne : pat `+1
+| PBot : pat `-⊥
+| PTen {A B} : pat `+A -> pat `+B -> pat `+(A ⊗ B)
+| PPar {A B} : pat `-A -> pat `-B -> pat `-(A ⅋ B)
+| POr1 {A B} : pat `+A -> pat `+(A ⊕ B)
+| POr2 {A B} : pat `+B -> pat `+(A ⊕ B)
+| PAnd1 {A B} : pat `-A -> pat `-(A & B)
+| PAnd2 {A B} : pat `-B -> pat `-(A & B)
+| PShiftP A : pat `+(↓ A)
+| PShiftN A : pat `-(↑ A)
+| PNegP {A} : pat `-A -> pat `+(⊖ A)
+| PNegN {A} : pat `+A -> pat `-(¬ A)
 .
-
+(*| .. coq:: none |*)
+Derive Signature NoConfusion NoConfusionHom for pat.
+(*|
+... and their domain, i.e. the context they bind.
+|*)
 Equations p_dom {t} : pat t -> neg_ctx :=
-  p_dom (PVarP A)    := ∅ₛ ▶ₛ {| sub_elt := t+ A ; sub_prf := stt |} ;
-  p_dom (PVarN A)    := ∅ₛ ▶ₛ {| sub_elt := t- A ; sub_prf := stt |} ;
+  p_dom (PVarP A)    := ∅ₛ ▶ₛ {| sub_elt := `+A ; sub_prf := stt |} ;
+  p_dom (PVarN A)    := ∅ₛ ▶ₛ {| sub_elt := `-A ; sub_prf := stt |} ;
   p_dom (POne)       := ∅ₛ ;
   p_dom (PBot)       := ∅ₛ ;
   p_dom (PTen p1 p2) := p_dom p1 +▶ₛ p_dom p2 ;
@@ -306,21 +414,28 @@ Equations p_dom {t} : pat t -> neg_ctx :=
   p_dom (POr2 p)     := p_dom p ;
   p_dom (PAnd1 p)    := p_dom p ;
   p_dom (PAnd2 p)    := p_dom p ;
-  p_dom (PShiftP A)  := ∅ₛ ▶ₛ {| sub_elt := t+ A ; sub_prf := stt |} ;
-  p_dom (PShiftN A)  := ∅ₛ ▶ₛ {| sub_elt := t- A ; sub_prf := stt |} ;
+  p_dom (PShiftP A)  := ∅ₛ ▶ₛ {| sub_elt := `+A ; sub_prf := stt |} ;
+  p_dom (PShiftN A)  := ∅ₛ ▶ₛ {| sub_elt := `-A ; sub_prf := stt |} ;
   p_dom (PNegP p)    := p_dom p ;
   p_dom (PNegN p)    := p_dom p .
-
-Definition pat' (Γ : t_ctx) : Type := sigT (fun A => prod (Γ ∋ A) (pat (t_neg A))).
-Definition p_dom' Γ : pat' Γ -> neg_ctx := fun p => p_dom (snd (projT2 p)).
-
+(*|
+We finally instanciate the observation structure. Note that our generic formalization
+mostly cares about 'observations', that is co-patterns. As such we instanciate observations
+by patterns at the dual type.
+|*)
+Definition obs_op : Oper ty neg_ctx :=
+  {| o_op A := pat A† ; o_dom _ p := p_dom p |} .
+(*|
+Now come a rather tedious set of embeddings between syntactic categories related to
+patterns. We start by embedding patterns into weak head-normal forms.
+|*)
 Equations w_of_p {a} (p : pat a) : whn (p_dom p) a :=
   w_of_p (PVarP _)    := Var top ;
   w_of_p (PVarN _)    := Var top ;
   w_of_p (POne)       := OneR ;
   w_of_p (PBot)       := BotL ;
-  w_of_p (PTen p1 p2) := TenR (w_rename r_concat_l _ (w_of_p p1)) (w_rename r_concat_r _ (w_of_p p2)) ;
-  w_of_p (PPar p1 p2) := ParL (w_rename r_concat_l _ (w_of_p p1)) (w_rename r_concat_r _ (w_of_p p2)) ;
+  w_of_p (PTen p1 p2) := TenR (w_of_p p1 `ᵥ⊛ᵣ r_cat_l) (w_of_p p2 `ᵥ⊛ᵣ r_cat_r) ;
+  w_of_p (PPar p1 p2) := ParL (w_of_p p1 `ᵥ⊛ᵣ r_cat_l) (w_of_p p2 `ᵥ⊛ᵣ r_cat_r) ;
   w_of_p (POr1 p)     := OrR1 (w_of_p p) ;
   w_of_p (POr2 p)     := OrR2 (w_of_p p) ;
   w_of_p (PAnd1 p)    := AndL1 (w_of_p p) ;
@@ -329,181 +444,157 @@ Equations w_of_p {a} (p : pat a) : whn (p_dom p) a :=
   w_of_p (PShiftN _)  := ShiftNL (Whn (Var top)) ;
   w_of_p (PNegP p)    := NegPR (w_of_p p) ;
   w_of_p (PNegN p)    := NegNL (w_of_p p) .
+(*|
+Now we explain how to split (some) weak head-normal forms into a pattern filled with
+values. I am sorry in advance for your CPU-cycles wasted to typechecking these quite
+hard dependent pattern matchings. We start off by two helpers for refuting impossible
+variables in negative context, which because of the use of `SProp` give trouble to
+`Equations` for deriving functional elimination principles if inlined.
+|*)
+Definition elim_var_p {Γ : neg_ctx} {A : ty0 pos} {X : Type} : Γ ∋ `+A -> X
+  := fun i => match s_prf i with end .
 
-#[derive(eliminator=no)]
-Equations p_of_w_0p {Γ : neg_ctx} (A : ty0 pos) : whn Γ (t+ A) -> pat (t+ A) :=
-  p_of_w_0p (0)     (Var i) with (s_elt_upg i).(sub_prf) := { | ! } ;
-  p_of_w_0p (1)     (Var i) with (s_elt_upg i).(sub_prf) := { | ! } ;
-  p_of_w_0p (A ⊗ B) (Var i) with (s_elt_upg i).(sub_prf) := { | ! } ;
-  p_of_w_0p (A ⊕ B) (Var i) with (s_elt_upg i).(sub_prf) := { | ! } ;
-  p_of_w_0p (↓ A)  (Var i) with (s_elt_upg i).(sub_prf) := { | ! } ;
-  p_of_w_0p (⊖ A)   (Var i) with (s_elt_upg i).(sub_prf) := { | ! } ;
+Definition elim_var_n {Γ : neg_ctx} {A : ty0 neg} {X : Type} : Γ ∋ `-A -> X
+  := fun i => match s_prf i with end .
+
+Equations p_of_w_0p {Γ : neg_ctx} (A : ty0 pos) : whn Γ `+A -> pat `+A :=
+  p_of_w_0p (0)     (Var i)      := elim_var_p i ;
+  p_of_w_0p (1)     (Var i)      := elim_var_p i ;
+  p_of_w_0p (A ⊗ B) (Var i)      := elim_var_p i ;
+  p_of_w_0p (A ⊕ B) (Var i)      := elim_var_p i ;
+  p_of_w_0p (↓ A)   (Var i)      := elim_var_p i ;
+  p_of_w_0p (⊖ A)   (Var i)      := elim_var_p i ;
   p_of_w_0p (1)     (OneR)       := POne ;
   p_of_w_0p (A ⊗ B) (TenR v1 v2) := PTen (p_of_w_0p A v1) (p_of_w_0p B v2) ;
   p_of_w_0p (A ⊕ B) (OrR1 v)     := POr1 (p_of_w_0p A v) ;
   p_of_w_0p (A ⊕ B) (OrR2 v)     := POr2 (p_of_w_0p B v) ;
-  p_of_w_0p (↓ A)  (ShiftPR _)  := PShiftP A ;
+  p_of_w_0p (↓ A)   (ShiftPR _)  := PShiftP A ;
   p_of_w_0p (⊖ A)   (NegPR k)    := PNegP (p_of_w_0n A k) ;
-with p_of_w_0n {Γ : neg_ctx} (A : ty0 neg) : whn Γ (t- A) -> pat (t- A) :=
-  p_of_w_0n (⊤)     (Var i) with (s_elt_upg i).(sub_prf) := { | ! } ;
-  p_of_w_0n (⊥)     (Var i) with (s_elt_upg i).(sub_prf) := { | ! } ;
-  p_of_w_0n (A ⅋ B) (Var i) with (s_elt_upg i).(sub_prf) := { | ! } ;
-  p_of_w_0n (A & B) (Var i) with (s_elt_upg i).(sub_prf) := { | ! } ;
-  p_of_w_0n (↑ A)  (Var i) with (s_elt_upg i).(sub_prf) := { | ! } ;
-  p_of_w_0n (¬ A)   (Var i) with (s_elt_upg i).(sub_prf) := { | ! } ;
+with p_of_w_0n {Γ : neg_ctx} (A : ty0 neg) : whn Γ `-A -> pat `-A :=
+  p_of_w_0n (⊤)     (Var i)      := elim_var_n i ;
+  p_of_w_0n (⊥)     (Var i)      := elim_var_n i ;
+  p_of_w_0n (A ⅋ B) (Var i)      := elim_var_n i ;
+  p_of_w_0n (A & B) (Var i)      := elim_var_n i ;
+  p_of_w_0n (↑ A)   (Var i)      := elim_var_n i ;
+  p_of_w_0n (¬ A)   (Var i)      := elim_var_n i ;
   p_of_w_0n (⊥)     (BotL)       := PBot ;
   p_of_w_0n (A ⅋ B) (ParL k1 k2) := PPar (p_of_w_0n A k1) (p_of_w_0n B k2) ;
   p_of_w_0n (A & B) (AndL1 k)    := PAnd1 (p_of_w_0n A k) ;
   p_of_w_0n (A & B) (AndL2 k)    := PAnd2 (p_of_w_0n B k) ;
-  p_of_w_0n (↑ A)  (ShiftNL _)  := PShiftN A ;
+  p_of_w_0n (↑ A)   (ShiftNL _)  := PShiftN A ;
   p_of_w_0n (¬ A)   (NegNL v)    := PNegN (p_of_w_0p A v) .
 
+Equations p_dom_of_w_0p {Γ : neg_ctx} (A : ty0 pos) (v : whn Γ `+A)
+          : p_dom (p_of_w_0p A v) =[val]> Γ by struct A :=
+  p_dom_of_w_0p (0)     (Var i)      := elim_var_p i ;
+  p_dom_of_w_0p (1)     (Var i)      := elim_var_p i ;
+  p_dom_of_w_0p (A ⊗ B) (Var i)      := elim_var_p i ;
+  p_dom_of_w_0p (A ⊕ B) (Var i)      := elim_var_p i ;
+  p_dom_of_w_0p (↓ A)   (Var i)      := elim_var_p i ;
+  p_dom_of_w_0p (⊖ A)   (Var i)      := elim_var_p i ;
+  p_dom_of_w_0p (1)     (OneR)       := a_empty ;
+  p_dom_of_w_0p (A ⊗ B) (TenR v1 v2) := [ p_dom_of_w_0p A v1 , p_dom_of_w_0p B v2 ] ;
+  p_dom_of_w_0p (A ⊕ B) (OrR1 v)     := p_dom_of_w_0p A v ;
+  p_dom_of_w_0p (A ⊕ B) (OrR2 v)     := p_dom_of_w_0p B v ;
+  p_dom_of_w_0p (↓ A)   (ShiftPR x)  := a_append a_empty x ;
+  p_dom_of_w_0p (⊖ A)   (NegPR k)    := p_dom_of_w_0n A k ;
+     with p_dom_of_w_0n {Γ : neg_ctx} (A : ty0 neg) (k : whn Γ `-A)
+          : p_dom (p_of_w_0n A k) =[val]> Γ by struct A :=
+  p_dom_of_w_0n (⊤)     (Var i)      := elim_var_n i ;
+  p_dom_of_w_0n (⊥)     (Var i)      := elim_var_n i ;
+  p_dom_of_w_0n (A ⅋ B) (Var i)      := elim_var_n i ;
+  p_dom_of_w_0n (A & B) (Var i)      := elim_var_n i ;
+  p_dom_of_w_0n (↑ A)   (Var i)      := elim_var_n i ;
+  p_dom_of_w_0n (¬ A)   (Var i)      := elim_var_n i ;
+  p_dom_of_w_0n (⊥)     (BotL)       := a_empty ;
+  p_dom_of_w_0n (A ⅋ B) (ParL k1 k2) := [ p_dom_of_w_0n A k1 , p_dom_of_w_0n B k2 ] ;
+  p_dom_of_w_0n (A & B) (AndL1 k)    := p_dom_of_w_0n A k ;
+  p_dom_of_w_0n (A & B) (AndL2 k)    := p_dom_of_w_0n B k ;
+  p_dom_of_w_0n (↑ A)   (ShiftNL x)  := a_append a_empty x ;
+  p_dom_of_w_0n (¬ A)   (NegNL v)    := p_dom_of_w_0p A v .
+(*|
+We can now package up all these auxiliary functions into the following ones, abstracting
+polarity and side-annotation.
+|*)
 Equations p_of_v {Γ : neg_ctx} A : val Γ A -> pat A :=
   p_of_v (@VTy pos A) v := p_of_w_0p A v ;
   p_of_v (@KTy pos A) _ := PVarN A ;
   p_of_v (@VTy neg A) _ := PVarP A ;
   p_of_v (@KTy neg A) k := p_of_w_0n A k .
 
-#[derive(eliminator=no)]
-Equations p_dom_of_w_0p {Γ : neg_ctx} (A : ty0 pos) (v : whn Γ (t+ A)) : p_dom (p_of_w_0p A v) =[val]> Γ by struct v :=
-  p_dom_of_w_0p (0)     (Var i) with (s_elt_upg i).(sub_prf) := { | ! } ;
-  p_dom_of_w_0p (1)     (Var i) with (s_elt_upg i).(sub_prf) := { | ! } ;
-  p_dom_of_w_0p (A ⊗ B) (Var i) with (s_elt_upg i).(sub_prf) := { | ! } ;
-  p_dom_of_w_0p (A ⊕ B) (Var i) with (s_elt_upg i).(sub_prf) := { | ! } ;
-  p_dom_of_w_0p (↓ A)  (Var i) with (s_elt_upg i).(sub_prf) := { | ! } ;
-  p_dom_of_w_0p (⊖ A)   (Var i) with (s_elt_upg i).(sub_prf) := { | ! } ;
-  p_dom_of_w_0p (1)     (OneR)       := a_empty ;
-  p_dom_of_w_0p (A ⊗ B) (TenR v1 v2) := [ p_dom_of_w_0p A v1 , p_dom_of_w_0p B v2 ] ;
-  p_dom_of_w_0p (A ⊕ B) (OrR1 v)     := p_dom_of_w_0p A v ;
-  p_dom_of_w_0p (A ⊕ B) (OrR2 v)     := p_dom_of_w_0p B v ;
-  p_dom_of_w_0p (↓ A)  (ShiftPR x)  := a_append a_empty x ;
-  p_dom_of_w_0p (⊖ A)   (NegPR k)    := p_dom_of_w_0n A k ;
-with p_dom_of_w_0n {Γ : neg_ctx} (A : ty0 neg) (k : whn Γ (t- A)) : p_dom (p_of_w_0n A k) =[val]> Γ by struct k :=
-  p_dom_of_w_0n (⊤)     (Var i) with (s_elt_upg i).(sub_prf) := { | ! } ;
-  p_dom_of_w_0n (⊥)     (Var i) with (s_elt_upg i).(sub_prf) := { | ! } ;
-  p_dom_of_w_0n (A ⅋ B) (Var i) with (s_elt_upg i).(sub_prf) := { | ! } ;
-  p_dom_of_w_0n (A & B) (Var i) with (s_elt_upg i).(sub_prf) := { | ! } ;
-  p_dom_of_w_0n (↑ A)  (Var i) with (s_elt_upg i).(sub_prf) := { | ! } ;
-  p_dom_of_w_0n (¬ A)   (Var i) with (s_elt_upg i).(sub_prf) := { | ! } ;
-  p_dom_of_w_0n (⊥)     (BotL)       := a_empty ;
-  p_dom_of_w_0n (A ⅋ B) (ParL k1 k2) := [ p_dom_of_w_0n A k1 , p_dom_of_w_0n B k2 ] ;
-  p_dom_of_w_0n (A & B) (AndL1 k)    := p_dom_of_w_0n A k ;
-  p_dom_of_w_0n (A & B) (AndL2 k)    := p_dom_of_w_0n B k ;
-  p_dom_of_w_0n (↑ A)  (ShiftNL x)  := a_append a_empty x ;
-  p_dom_of_w_0n (¬ A)   (NegNL v)    := p_dom_of_w_0p A v .
-
 Equations p_dom_of_v {Γ : neg_ctx} A (v : val Γ A) : p_dom (p_of_v A v) =[val]> Γ :=
   p_dom_of_v (@VTy pos A) v := p_dom_of_w_0p A v ;
-  p_dom_of_v (@KTy pos A) x := a_append a_empty x ;
-  p_dom_of_v (@VTy neg A) x := a_append a_empty x ;
+  p_dom_of_v (@KTy pos A) x := [ ! ,ₓ x ] ;
+  p_dom_of_v (@VTy neg A) x := [ ! ,ₓ x ] ;
   p_dom_of_v (@KTy neg A) k := p_dom_of_w_0n A k .
 
-Definition nf0 (Γ : t_ctx) (A : ty) : Type := sigT (fun p : pat (t_neg A) => p_dom p =[val]> Γ) .
-Definition nf (Γ : t_ctx) : Type := sigT (fun A => prod (Γ ∋ A) (nf0 Γ A)) .
+Definition v_split_p {Γ : neg_ctx} {A} (v : whn Γ `+A) : (obs_op # val) Γ `-A
+  := (p_of_w_0p A v : o_op obs_op `-A) ⦇ p_dom_of_w_0p A v ⦈.
 
-Definition n_rename {Γ Δ : neg_ctx} : Γ ⊆ Δ -> nf Γ -> nf Δ :=
-  fun r u => (projT1 u ,' (r _ (fst (projT2 u)) , (projT1 (snd (projT2 u)) ,' a_ren r (projT2 (snd (projT2 u)))))) .
+Definition v_split_n {Γ : neg_ctx} {A} (v : whn Γ `-A) : (obs_op # val) Γ `+A
+  := (p_of_w_0n A v : o_op obs_op `+_) ⦇ p_dom_of_w_0n A v ⦈.
+(*|
+Evaluation
+==========
 
-Definition nf0_eq {Γ a} : relation (nf0 Γ a) :=
-  fun a b => exists H : projT1 a = projT1 b, rew H in projT2 a ≡ₐ projT2 b .
-
-Definition nf_eq {Γ} : relation (nf Γ) :=
-  fun a b => exists H : projT1 a = projT1 b,
-      (rew H in fst (projT2 a) = fst (projT2 b)) /\ (nf0_eq (rew H in snd (projT2 a)) (snd (projT2 b))).
-
-#[global] Instance nf0_eq_rfl {Γ t} : Reflexive (@nf0_eq Γ t) .
-  intros [ m a ]; unshelve econstructor; auto.
-Qed.
-
-#[global] Instance nf0_eq_sym {Γ t} : Symmetric (@nf0_eq Γ t) .
-  intros [ m1 a1 ] [ m2 a2 ] [ p q ]; unshelve econstructor; cbn in *.
-  - now symmetry.
-  - revert a1 q ; rewrite p; intros a1 q.
-    now symmetry.
-Qed.
-
-#[global] Instance nf0_eq_tra {Γ t} : Transitive (@nf0_eq Γ t) .
-  intros [ m1 a1 ] [ m2 a2 ] [ m3 a3 ] [ p1 q1 ] [ p2 q2 ]; unshelve econstructor; cbn in *.
-  - now transitivity m2.
-  - transitivity (rew [fun p : pat (t_neg t) => p_dom p =[ val ]> Γ] p2 in a2); auto.
-    now rewrite <- p2.
-Qed.
-
-#[global] Instance nf_eq_rfl {Γ} : Reflexiveᵢ (fun _ : T1 => @nf_eq Γ) .
-  intros _ [ x [ i n ] ].
-  unshelve econstructor; auto.
-Qed.
-
-#[global] Instance nf_eq_sym {Γ} : Symmetricᵢ (fun _ : T1 => @nf_eq Γ) .
-  intros _ [ x1 [ i1 n1 ] ] [ x2 [ i2 n2 ] ] [ p [ q1 q2 ] ].
-  unshelve econstructor; [ | split ]; cbn in *.
-  - now symmetry.
-  - revert i1 q1; rewrite p; intros i1 q1; now symmetry.
-  - revert n1 q2; rewrite p; intros n1 q2; now symmetry.
-Qed.
-
-#[global] Instance nf_eq_tra {Γ} : Transitiveᵢ (fun _ : T1 => @nf_eq Γ) .
-  intros _ [ x1 [ i1 n1 ] ] [ x2 [ i2 n2 ] ] [ x3 [ i3 n3 ] ] [ p1 [ q1 r1 ] ] [ p2 [ q2 r2 ] ].
-  unshelve econstructor; [ | split ]; cbn in *.
-  - now transitivity x2.
-  - transitivity (rew [has Γ] p2 in i2); auto.
-    now rewrite <- p2.
-  - transitivity (rew [nf0 Γ] p2 in n2); auto.
-    now rewrite <- p2.
-Qed.
-
-Definition comp_eq {Γ} : relation (delay (nf Γ)) :=
-  it_eq (fun _ : T1 => nf_eq) (i := T1_0) .
-Notation "u ≋ v" := (comp_eq u v) (at level 40) .
-
-Definition pat_of_nf : nf ⇒ᵢ pat' :=
-  fun Γ u => (projT1 u ,' (fst (projT2 u) , projT1 (snd (projT2 u)))) .
-
-#[derive(eliminator=no)]
+With patterns and observations now in hand we prepare for the definition of evaluation
+and define a shorthand for normal forms. 'Normal forms' are here understood---as in the
+paper---in our slightly non-standard presentation of triplets of a variable, an
+observation and an assignment.
+|*)
+Definition nf : Fam₀ ty neg_ctx := c_var ∥ₛ (obs_op # val).
+(*|
+Now the bulk of evaluation: the step function. Once again we are greatful for
+`Equations` providing us with a justification for the fact that this complex
+dependent pattern-matching is indeed total.
+|*)
 Equations eval_aux {Γ : neg_ctx} : state Γ -> (state Γ + nf Γ) :=
-  eval_aux (Cut pos (Mu c)  (x))    := inl (c ₛ/[ x ]) ;
-  eval_aux (Cut neg (x)     (Mu c)) := inl (c ₛ/[ x ]) ;
+  eval_aux (Cut pos (Mu c)  (x))    := inl (c ₜ⊛ ₁[ x ]) ;
+  eval_aux (Cut neg (x)     (Mu c)) := inl (c ₜ⊛ ₁[ x ]) ;
 
-  eval_aux (Cut pos (Whn v) (Mu c))  := inl (c ₛ/[ v ]) ;
-  eval_aux (Cut neg (Mu c)  (Whn k)) := inl (c ₛ/[ k ]) ;
+  eval_aux (Cut pos (Whn v) (Mu c))  := inl (c ₜ⊛ ₁[ v ]) ;
+  eval_aux (Cut neg (Mu c)  (Whn k)) := inl (c ₜ⊛ ₁[ k ]) ;
 
-  eval_aux (Cut pos (Whn v)  (RecL k)) := inl (Cut pos (Whn v) (k ₜ/[ RecL k ])) ;
-  eval_aux (Cut neg (RecR t) (Whn k))  := inl (Cut neg (t ₜ/[ RecR t ]) (Whn k)) ;
+  eval_aux (Cut pos (Whn v)  (RecL k)) := inl (Cut pos (Whn v) (k `ₜ⊛ ₁[ RecL k ])) ;
+  eval_aux (Cut neg (RecR t) (Whn k))  := inl (Cut neg (t `ₜ⊛ ₁[ RecR t ]) (Whn k)) ;
 
-  eval_aux (Cut pos (Whn v)       (Whn (Var i))) := inr (_ ,' (i , (p_of_w_0p _ v ,' p_dom_of_w_0p _ v))) ;
-  eval_aux (Cut neg (Whn (Var i)) (Whn k))       := inr (_ ,' (i , (p_of_w_0n _ k ,' p_dom_of_w_0n _ k))) ;
+  eval_aux (Cut pos (Whn v)       (Whn (Var i))) := inr (s_var_upg i ⋅ v_split_p v) ;
+  eval_aux (Cut neg (Whn (Var i)) (Whn k))       := inr (s_var_upg i ⋅ v_split_n k) ;
 
-  eval_aux (Cut pos (Whn (Var i)) (Whn _))       with (s_elt_upg i).(sub_prf) := { | (!) } ;
-  eval_aux (Cut neg (Whn _)       (Whn (Var i))) with (s_elt_upg i).(sub_prf) := { | (!) } ;
+  eval_aux (Cut pos (Whn (Var i)) (Whn _))       := elim_var_p i ;
+  eval_aux (Cut neg (Whn _)       (Whn (Var i))) := elim_var_n i ;
 
   eval_aux (Cut pos (Whn (OneR))       (Whn (OneL c)))     := inl c ;
   eval_aux (Cut neg (Whn (BotR c))     (Whn (BotL)))       := inl c ;
-  eval_aux (Cut pos (Whn (TenR v1 v2)) (Whn (TenL c)))     := inl (c ₛ/[ v1 , v2 ]) ;
-  eval_aux (Cut neg (Whn (ParR c))     (Whn (ParL k1 k2))) := inl (c ₛ/[ k1 , k2 ]) ;
-  eval_aux (Cut pos (Whn (OrR1 v))     (Whn (OrL c1 c2)))  := inl (c1 ₛ/[ v ]) ;
-  eval_aux (Cut pos (Whn (OrR2 v))     (Whn (OrL c1 c2)))  := inl (c2 ₛ/[ v ]) ;
-  eval_aux (Cut neg (Whn (AndR c1 c2)) (Whn (AndL1 k)))    := inl (c1 ₛ/[ k ]) ;
-  eval_aux (Cut neg (Whn (AndR c1 c2)) (Whn (AndL2 k)))    := inl (c2 ₛ/[ k ]) ;
-  eval_aux (Cut pos (Whn (ShiftPR x))  (Whn (ShiftPL c)))  := inl (c ₛ/[ x ]) ;
-  eval_aux (Cut neg (Whn (ShiftNR c))  (Whn (ShiftNL x)))  := inl (c ₛ/[ x ]) ;
-  eval_aux (Cut pos (Whn (NegPR k))    (Whn (NegPL c)))    := inl (c ₛ/[ k ]) ;
-  eval_aux (Cut neg (Whn (NegNR c))    (Whn (NegNL v)))    := inl (c ₛ/[ v ]) .
-
+  eval_aux (Cut pos (Whn (TenR v1 v2)) (Whn (TenL c)))     := inl (c ₜ⊛ ₂[ v1 , v2 ]) ;
+  eval_aux (Cut neg (Whn (ParR c))     (Whn (ParL k1 k2))) := inl (c ₜ⊛ ₂[ k1 , k2 ]) ;
+  eval_aux (Cut pos (Whn (OrR1 v))     (Whn (OrL c1 c2)))  := inl (c1 ₜ⊛ ₁[ v ]) ;
+  eval_aux (Cut pos (Whn (OrR2 v))     (Whn (OrL c1 c2)))  := inl (c2 ₜ⊛ ₁[ v ]) ;
+  eval_aux (Cut neg (Whn (AndR c1 c2)) (Whn (AndL1 k)))    := inl (c1 ₜ⊛ ₁[ k ]) ;
+  eval_aux (Cut neg (Whn (AndR c1 c2)) (Whn (AndL2 k)))    := inl (c2 ₜ⊛ ₁[ k ]) ;
+  eval_aux (Cut pos (Whn (ShiftPR x))  (Whn (ShiftPL c)))  := inl (c ₜ⊛ ₁[ x ]) ;
+  eval_aux (Cut neg (Whn (ShiftNR c))  (Whn (ShiftNL x)))  := inl (c ₜ⊛ ₁[ x ]) ;
+  eval_aux (Cut pos (Whn (NegPR k))    (Whn (NegPL c)))    := inl (c ₜ⊛ ₁[ k ]) ;
+  eval_aux (Cut neg (Whn (NegNR c))    (Whn (NegNL v)))    := inl (c ₜ⊛ ₁[ v ]) .
+(*|
+Finally we define evaluation as the iteration of the step function in the Delay monad,
+and also define application of an observation with arguments to a value.
+|*)
 Definition eval {Γ : neg_ctx} : state Γ -> delay (nf Γ)
   := iter_delay (fun c => Ret' (eval_aux c)).
 
-Definition refold {Γ : neg_ctx} (n : nf Γ) : prod (Γ ∋ (projT1 n)) (val Γ (t_neg (projT1 n))) :=
-  (fst (projT2 n) , w_subst (projT2 (snd (projT2 n))) _ (w_of_p (projT1 (snd (projT2 n))))) .
+Definition p_app {Γ A} (v : val Γ A) (m : pat A†) (e : p_dom m =[val]> Γ) : state Γ :=
+  Cut' (t_of_v _ v) (t_of_v _ (w_of_p m `ᵥ⊛ e)) .
+(*|
+Metatheory
+==========
 
-Definition Cut' {Γ A} : term Γ A -> term Γ (t_neg A) -> state Γ :=
-  match A with
-  | t+ A => fun t1 t2 => Cut _ t1 t2
-  | t- A => fun t1 t2 => Cut _ t2 t1
-  end .
-
-Definition p_app {Γ A} (v : val Γ A) (m : pat (t_neg A)) (e : p_dom m =[val]> Γ) : state Γ :=
-  Cut' (t_of_v _ v) (t_of_v _ (w_subst e _ (w_of_p m))) .
-
+Now comes a rather ugly part: the metatheory of our syntax. Comments will be rather more
+sparse. For a thorough explaination of its structure, see `Examples/Lambda/CBVTyped.v`.
+We will here be concerned with extensional equality preservation, identity and composition
+laws for renaming and substitution, and also refolding lemmas for splitting and embedding
+patterns. You are encouraged to just skip until line ~1300.
+|*)
 Scheme term_mut := Induction for term Sort Prop
   with whn_mut := Induction for whn Sort Prop
   with state_mut := Induction for state Sort Prop.
@@ -512,38 +603,38 @@ Record syn_ind_args
   (P_t : forall Γ A, term Γ A -> Prop)
   (P_w : forall Γ A, whn Γ A -> Prop)
   (P_s : forall Γ, state Γ -> Prop) :=
-  {
-    ind_mu : forall Γ A s (H : P_s _ s), P_t Γ A (Mu s) ;
-    ind_recp : forall Γ A t (H : P_t _ _ t), P_t Γ (t- A) (RecL t) ;
-    ind_recn : forall Γ A t (H : P_t _ _ t), P_t Γ (t+ A) (RecR t) ;
-    ind_whn : forall Γ A w (H : P_w _ _ w), P_t Γ A (Whn w) ;
-    ind_var : forall Γ A h, P_w Γ A (Var h) ;
-    ind_zerl : forall Γ, P_w Γ (t- 0) ZerL ;
-    ind_topr : forall Γ, P_w Γ (t+ ⊤) TopR ;
-    ind_oner : forall Γ, P_w Γ (t+ 1) OneR ;
-    ind_onel : forall Γ s, P_s Γ s -> P_w Γ (t- 1) (OneL s) ;
-    ind_botr : forall Γ s, P_s Γ s -> P_w Γ (t+ ⊥) (BotR s) ;
-    ind_botl : forall Γ, P_w Γ (t- ⊥) BotL ;
-    ind_tenr : forall Γ A B w1 (H1 : P_w _ _ w1) w2 (H2 : P_w _ _ w2), P_w Γ (t+ (A ⊗ B)) (TenR w1 w2) ;
-    ind_tenl : forall Γ A B s (H : P_s _ s), P_w Γ (t- (A ⊗ B)) (TenL s) ;
-    ind_parr : forall Γ A B s (H : P_s _ s), P_w Γ (t+ (A ⅋ B)) (ParR s) ;
-    ind_parl : forall Γ A B w1 (H1 : P_w _ _ w1) w2 (H2 : P_w Γ (t- B) w2), P_w Γ (t- (A ⅋ B)) (ParL w1 w2) ;
-    ind_orr1 : forall Γ A B w (H : P_w _ _ w), P_w Γ (t+ (A ⊕ B)) (OrR1 w) ;
-    ind_orr2 : forall Γ A B w (H : P_w _ _ w), P_w Γ (t+ (A ⊕ B)) (OrR2 w) ;
-    ind_orl : forall Γ A B s1 (H1 : P_s _ s1) s2 (H2 : P_s _ s2), P_w Γ (t- (A ⊕ B)) (OrL s1 s2) ;
-    ind_andr : forall Γ A B s1 (H1 : P_s _ s1) s2 (H2 : P_s _ s2), P_w Γ (t+ (A & B)) (AndR s1 s2) ;
-    ind_andl1 : forall Γ A B w (H : P_w _ _ w), P_w Γ (t- (A & B)) (AndL1 w) ;
-    ind_andl2 : forall Γ A B w (H : P_w _ _ w), P_w Γ (t- (A & B)) (AndL2 w) ;
-    ind_shiftpr : forall Γ A t (H : P_t _ _ t), P_w Γ (t+ (↓ A)) (ShiftPR t) ;
-    ind_shiftpl : forall Γ A s (H : P_s _ s), P_w Γ (t- (↓ A)) (ShiftPL s) ;
-    ind_shiftnr : forall Γ A s (H : P_s _ s), P_w Γ (t+ (↑ A)) (ShiftNR s) ;
-    ind_shiftnl : forall Γ A t (H : P_t _ _ t), P_w Γ (t- (↑ A)) (ShiftNL t) ;
-    ind_negpr : forall Γ A w (H : P_w _ _ w), P_w Γ (t+ (⊖ A)) (NegPR w) ;
-    ind_negpl : forall Γ A s (H : P_s _ s), P_w Γ (t- (⊖ A)) (NegPL s) ;
-    ind_negnr : forall Γ A s (H : P_s _ s), P_w Γ (t+ (¬ A)) (NegNR s) ;
-    ind_negnl : forall Γ A w (H : P_w _ _ w), P_w Γ (t- (¬ A)) (NegNL w) ;
-    ind_cut : forall Γ p A t1 (H1 : P_t _ _ t1) t2 (H2 : P_t _ _ t2), P_s Γ (@Cut _ p A t1 t2)
-  } .
+{
+  ind_mu : forall Γ A s (H : P_s _ s), P_t Γ A (Mu s) ;
+  ind_recp : forall Γ A t (H : P_t _ _ t), P_t Γ `-A (RecL t) ;
+  ind_recn : forall Γ A t (H : P_t _ _ t), P_t Γ `+A (RecR t) ;
+  ind_whn : forall Γ A w (H : P_w _ _ w), P_t Γ A (Whn w) ;
+  ind_var : forall Γ A h, P_w Γ A (Var h) ;
+  ind_zerl : forall Γ, P_w Γ `-0 ZerL ;
+  ind_topr : forall Γ, P_w Γ `+⊤ TopR ;
+  ind_oner : forall Γ, P_w Γ `+1 OneR ;
+  ind_onel : forall Γ s, P_s Γ s -> P_w Γ `-1 (OneL s) ;
+  ind_botr : forall Γ s, P_s Γ s -> P_w Γ `+⊥ (BotR s) ;
+  ind_botl : forall Γ, P_w Γ `-⊥ BotL ;
+  ind_tenr : forall Γ A B w1 (H1 : P_w _ _ w1) w2 (H2 : P_w _ _ w2), P_w Γ `+(A ⊗ B) (TenR w1 w2) ;
+  ind_tenl : forall Γ A B s (H : P_s _ s), P_w Γ `-(A ⊗ B) (TenL s) ;
+  ind_parr : forall Γ A B s (H : P_s _ s), P_w Γ `+(A ⅋ B) (ParR s) ;
+  ind_parl : forall Γ A B w1 (H1 : P_w _ _ w1) w2 (H2 : P_w Γ `-B w2), P_w Γ `-(A ⅋ B) (ParL w1 w2) ;
+  ind_orr1 : forall Γ A B w (H : P_w _ _ w), P_w Γ `+(A ⊕ B) (OrR1 w) ;
+  ind_orr2 : forall Γ A B w (H : P_w _ _ w), P_w Γ `+(A ⊕ B) (OrR2 w) ;
+  ind_orl : forall Γ A B s1 (H1 : P_s _ s1) s2 (H2 : P_s _ s2), P_w Γ `-(A ⊕ B) (OrL s1 s2) ;
+  ind_andr : forall Γ A B s1 (H1 : P_s _ s1) s2 (H2 : P_s _ s2), P_w Γ `+(A & B) (AndR s1 s2) ;
+  ind_andl1 : forall Γ A B w (H : P_w _ _ w), P_w Γ `-(A & B) (AndL1 w) ;
+  ind_andl2 : forall Γ A B w (H : P_w _ _ w), P_w Γ `-(A & B) (AndL2 w) ;
+  ind_shiftpr : forall Γ A t (H : P_t _ _ t), P_w Γ `+(↓ A) (ShiftPR t) ;
+  ind_shiftpl : forall Γ A s (H : P_s _ s), P_w Γ `-(↓ A) (ShiftPL s) ;
+  ind_shiftnr : forall Γ A s (H : P_s _ s), P_w Γ `+(↑ A) (ShiftNR s) ;
+  ind_shiftnl : forall Γ A t (H : P_t _ _ t), P_w Γ `-(↑ A) (ShiftNL t) ;
+  ind_negpr : forall Γ A w (H : P_w _ _ w), P_w Γ `+(⊖ A) (NegPR w) ;
+  ind_negpl : forall Γ A s (H : P_s _ s), P_w Γ `-(⊖ A) (NegPL s) ;
+  ind_negnr : forall Γ A s (H : P_s _ s), P_w Γ `+(¬ A) (NegNR s) ;
+  ind_negnl : forall Γ A w (H : P_w _ _ w), P_w Γ `-(¬ A) (NegNL w) ;
+  ind_cut : forall Γ p A t1 (H1 : P_t _ _ t1) t2 (H2 : P_t _ _ t2), P_s Γ (@Cut _ p A t1 t2)
+} .
 
 Lemma term_ind_mut P_t P_w P_s (H : syn_ind_args P_t P_w P_s) Γ A t : P_t Γ A t .
   destruct H; now apply (term_mut P_t P_w P_s).
@@ -558,37 +649,33 @@ Lemma state_ind_mut P_t P_w P_s (H : syn_ind_args P_t P_w P_s) Γ s : P_s Γ s .
 Qed.
 
 Definition t_ren_proper_P Γ A (t : term Γ A) : Prop :=
-  forall Δ (f1 f2 : Γ ⊆ Δ), f1 ≡ₐ f2 -> t_rename f1 A t = t_rename f2 A t .
+  forall Δ (f1 f2 : Γ ⊆ Δ), f1 ≡ₐ f2 -> t ₜ⊛ᵣ f1 = t ₜ⊛ᵣ f2 .
 Definition w_ren_proper_P Γ A (v : whn Γ A) : Prop :=
-  forall Δ (f1 f2 : Γ ⊆ Δ), f1 ≡ₐ f2 -> w_rename f1 A v = w_rename f2 A v .
+  forall Δ (f1 f2 : Γ ⊆ Δ), f1 ≡ₐ f2 -> v `ᵥ⊛ᵣ f1 = v `ᵥ⊛ᵣ f2 .
 Definition s_ren_proper_P Γ (s : state Γ) : Prop :=
-  forall Δ (f1 f2 : Γ ⊆ Δ), f1 ≡ₐ f2 -> s_rename f1 s = s_rename f2 s .
+  forall Δ (f1 f2 : Γ ⊆ Δ), f1 ≡ₐ f2 -> s ₛ⊛ᵣ f1 = s ₛ⊛ᵣ f2 .
 Lemma ren_proper_prf : syn_ind_args t_ren_proper_P w_ren_proper_P s_ren_proper_P.
   econstructor.
   all: unfold t_ren_proper_P, w_ren_proper_P, s_ren_proper_P.
-  all: intros; cbn; f_equal.
-  all: try apply H; try apply H1; try apply H2.
-  all: repeat apply r_shift_eq; auto.
+  all: intros; cbn; f_equal; eauto.
+  all: first [ apply H | apply H1 | apply H2 ]; auto.
+  all: first [ apply r_shift1_eq | apply r_shift2_eq ]; auto.
 Qed.
 
-#[global] Instance t_ren_eq {Γ Δ}
-  : Proper (ass_eq _ _ ==> forall_relation (fun a => eq ==> eq)) (@t_rename Γ Δ).
-  intros f1 f2 H1 a x y ->; now apply (term_ind_mut _ _ _ ren_proper_prf).
+#[global] Instance t_ren_eq {Γ a t Δ} : Proper (asgn_eq _ _ ==> eq) (t_rename Γ a t Δ).
+  intros f1 f2 H1; now apply (term_ind_mut _ _ _ ren_proper_prf).
 Qed.
 
-#[global] Instance w_ren_eq {Γ Δ}
-  : Proper (ass_eq _ _ ==> forall_relation (fun a => eq ==> eq)) (@w_rename Γ Δ).
-  intros f1 f2 H1 a x y ->; now apply (whn_ind_mut _ _ _ ren_proper_prf).
+#[global] Instance w_ren_eq {Γ a v Δ} : Proper (asgn_eq _ _ ==> eq) (w_rename Γ a v Δ).
+  intros f1 f2 H1; now apply (whn_ind_mut _ _ _ ren_proper_prf).
 Qed.
 
-#[global] Instance s_ren_eq {Γ Δ}
-  : Proper (ass_eq _ _ ==> eq ==> eq) (@s_rename Γ Δ).
-  intros f1 f2 H1 x y ->; now apply (state_ind_mut _ _ _ ren_proper_prf).
+#[global] Instance s_ren_eq {Γ s Δ} : Proper (asgn_eq _ _ ==> eq) (s_rename Γ s Δ).
+  intros f1 f2 H1; now apply (state_ind_mut _ _ _ ren_proper_prf).
 Qed.
 
-#[global] Instance v_ren_eq {Γ Δ}
-  : Proper (ass_eq _ _ ==> forall_relation (fun _ => eq ==> eq)) (@v_rename Γ Δ).
-  intros f1 f2 H1 [ [] | [] ] v1 v2 H2.
+#[global] Instance v_ren_eq {Γ a v Δ} : Proper (asgn_eq _ _ ==> eq) (v_rename Γ a v Δ).
+  destruct a as [ [] | [] ].
   now apply w_ren_eq.
   now apply t_ren_eq.
   now apply t_ren_eq.
@@ -596,52 +683,52 @@ Qed.
 Qed.
 
 #[global] Instance a_ren_eq {Γ1 Γ2 Γ3}
-  : Proper (ass_eq _ _ ==> ass_eq _ _ ==> ass_eq _ _) (@a_ren Γ1 Γ2 Γ3).
-  intros r1 r2 H1 a1 a2 H2 ? i; apply (v_ren_eq _ _ H1), H2.
+  : Proper (asgn_eq _ _ ==> asgn_eq _ _ ==> asgn_eq _ _) (@a_ren Γ1 Γ2 Γ3).
+  intros r1 r2 H1 a1 a2 H2 ? i; cbn; now rewrite H1, (v_ren_eq _ _ H2).
 Qed.
 
-#[global] Instance a_shift_eq {Γ Δ A} : Proper (ass_eq _ _ ==> ass_eq _ _) (@a_shift Γ Δ A).
+#[global] Instance a_shift1_eq {Γ Δ A} : Proper (asgn_eq _ _ ==> asgn_eq _ _) (@a_shift1 Γ Δ A).
   intros ? ? H ? h.
   dependent elimination h; auto; cbn; now rewrite H.
 Qed.
 
-#[global] Instance a_shift2_eq {Γ Δ A B} : Proper (ass_eq _ _ ==> ass_eq _ _) (@a_shift2 Γ Δ A B).
-  intros ? ? H ? h.
-  do 2 (dependent elimination h; auto).
+#[global] Instance a_shift2_eq {Γ Δ A B} : Proper (asgn_eq _ _ ==> asgn_eq _ _) (@a_shift2 Γ Δ A B).
+  intros ? ? H ? v.
+  do 2 (dependent elimination v; auto).
   cbn; now rewrite H.
 Qed.
 
 Definition t_ren_ren_P Γ1 A (t : term Γ1 A) : Prop :=
-  forall Γ2 Γ3 (f1 : Γ2 ⊆ Γ3) (f2 : Γ1 ⊆ Γ2),
-    t_rename f1 A (t_rename f2 A t) = t_rename (s_ren f1 f2) A t.
+  forall Γ2 Γ3 (f1 : Γ1 ⊆ Γ2) (f2 : Γ2 ⊆ Γ3),
+    (t ₜ⊛ᵣ f1) ₜ⊛ᵣ f2 = t ₜ⊛ᵣ (f1 ᵣ⊛ f2) .
 Definition w_ren_ren_P Γ1 A (v : whn Γ1 A) : Prop :=
-  forall Γ2 Γ3 (f1 : Γ2 ⊆ Γ3) (f2 : Γ1 ⊆ Γ2),
-    w_rename f1 A (w_rename f2 A v) = w_rename (s_ren f1 f2) A v.
+  forall Γ2 Γ3 (f1 : Γ1 ⊆ Γ2) (f2 : Γ2 ⊆ Γ3),
+    (v `ᵥ⊛ᵣ f1) `ᵥ⊛ᵣ f2 = v `ᵥ⊛ᵣ (f1 ᵣ⊛ f2) .
 Definition s_ren_ren_P Γ1 (s : state Γ1) : Prop :=
-  forall Γ2 Γ3 (f1 : Γ2 ⊆ Γ3) (f2 : Γ1 ⊆ Γ2),
-    s_rename f1 (s_rename f2 s) = s_rename (s_ren f1 f2) s.
+  forall Γ2 Γ3 (f1 : Γ1 ⊆ Γ2) (f2 : Γ2 ⊆ Γ3),
+    (s ₛ⊛ᵣ f1) ₛ⊛ᵣ f2 = s ₛ⊛ᵣ (f1 ᵣ⊛ f2) .
 
 Lemma ren_ren_prf : syn_ind_args t_ren_ren_P w_ren_ren_P s_ren_ren_P.
   econstructor.
   all: unfold t_ren_ren_P, w_ren_ren_P, s_ren_ren_P.
-  all: intros; cbn; f_equal.
-  all: unfold r_shift2; now repeat rewrite r_shift_comp.
+  all: intros; cbn; f_equal; eauto.
+  all: first [ rewrite r_shift1_comp | rewrite r_shift2_comp ]; eauto.
 Qed.
 
-Lemma t_ren_ren {Γ1 Γ2 Γ3} (f1 : Γ2 ⊆ Γ3) (f2 : Γ1 ⊆ Γ2) A (t : term Γ1 A)
-  : t_rename f1 A (t_rename f2 A t) = t_rename (s_ren f1 f2) A t.
+Lemma t_ren_ren {Γ1 Γ2 Γ3} (f1 : Γ1 ⊆ Γ2) (f2 : Γ2 ⊆ Γ3) A (t : term Γ1 A)
+  : (t ₜ⊛ᵣ f1) ₜ⊛ᵣ f2 = t ₜ⊛ᵣ (f1 ᵣ⊛ f2) .
   now apply (term_ind_mut _ _ _ ren_ren_prf).
 Qed.
-Lemma w_ren_ren {Γ1 Γ2 Γ3} (f1 : Γ2 ⊆ Γ3) (f2 : Γ1 ⊆ Γ2) A (v : whn Γ1 A)
-  : w_rename f1 A (w_rename f2 A v) = w_rename (s_ren f1 f2) A v.
+Lemma w_ren_ren {Γ1 Γ2 Γ3} (f1 : Γ1 ⊆ Γ2) (f2 : Γ2 ⊆ Γ3) A (v : whn Γ1 A)
+  : (v `ᵥ⊛ᵣ f1) `ᵥ⊛ᵣ f2 = v `ᵥ⊛ᵣ (f1 ᵣ⊛ f2) .
   now apply (whn_ind_mut _ _ _ ren_ren_prf).
 Qed.
-Lemma s_ren_ren {Γ1 Γ2 Γ3} (f1 : Γ2 ⊆ Γ3) (f2 : Γ1 ⊆ Γ2) (s : state Γ1)
-  : s_rename f1 (s_rename f2 s) = s_rename (s_ren f1 f2) s.
+Lemma s_ren_ren {Γ1 Γ2 Γ3} (f1 : Γ1 ⊆ Γ2) (f2 : Γ2 ⊆ Γ3) (s : state Γ1)
+  : (s ₛ⊛ᵣ f1) ₛ⊛ᵣ f2 = s ₛ⊛ᵣ (f1 ᵣ⊛ f2) .
   now apply (state_ind_mut _ _ _ ren_ren_prf).
 Qed.
-Lemma v_ren_ren {Γ1 Γ2 Γ3} (f1 : Γ2 ⊆ Γ3) (f2 : Γ1 ⊆ Γ2) A (v : val Γ1 A)
-  : v_rename f1 A (v_rename f2 A v) = v_rename (s_ren f1 f2) A v.
+Lemma v_ren_ren {Γ1 Γ2 Γ3} (f1 : Γ1 ⊆ Γ2) (f2 : Γ2 ⊆ Γ3) A (v : val Γ1 A)
+  : (v ᵥ⊛ᵣ f1) ᵥ⊛ᵣ f2 = v ᵥ⊛ᵣ (f1 ᵣ⊛ f2) .
   destruct A as [ [] | [] ].
   now apply w_ren_ren.
   now apply t_ren_ren.
@@ -649,27 +736,27 @@ Lemma v_ren_ren {Γ1 Γ2 Γ3} (f1 : Γ2 ⊆ Γ3) (f2 : Γ1 ⊆ Γ2) A (v : val �
   now apply w_ren_ren.
 Qed.
 
-Definition t_ren_id_l_P Γ A (t : term Γ A) : Prop := t_rename r_id A t = t.
-Definition w_ren_id_l_P Γ A (v : whn Γ A) : Prop := w_rename r_id A v = v.
-Definition s_ren_id_l_P Γ (s : state Γ) : Prop := s_rename r_id s = s.
+Definition t_ren_id_l_P Γ A (t : term Γ A) : Prop := t ₜ⊛ᵣ r_id = t.
+Definition w_ren_id_l_P Γ A (v : whn Γ A) : Prop := v `ᵥ⊛ᵣ r_id = v.
+Definition s_ren_id_l_P Γ (s : state Γ) : Prop := s ₛ⊛ᵣ r_id  = s.
 
 Lemma ren_id_l_prf : syn_ind_args t_ren_id_l_P w_ren_id_l_P s_ren_id_l_P.
   econstructor.
   all: unfold t_ren_id_l_P, w_ren_id_l_P, s_ren_id_l_P.
-  all: intros; cbn; f_equal.
-  all: unfold r_shift2; now repeat rewrite r_shift_id.
+  all: intros; cbn; f_equal; eauto.
+  all: first [ rewrite r_shift1_id | rewrite r_shift2_id ]; eauto.
 Qed.
 
-Lemma t_ren_id_l {Γ} A (t : term Γ A) : t_rename r_id A t = t.
+Lemma t_ren_id_l {Γ} A (t : term Γ A) : t ₜ⊛ᵣ r_id = t.
   now apply (term_ind_mut _ _ _ ren_id_l_prf).
 Qed.
-Lemma w_ren_id_l {Γ} A (v : whn Γ A) : w_rename r_id A v = v.
+Lemma w_ren_id_l {Γ} A (v : whn Γ A) : v `ᵥ⊛ᵣ r_id = v.
   now apply (whn_ind_mut _ _ _ ren_id_l_prf).
 Qed.
-Lemma s_ren_id_l {Γ} (s : state Γ) : s_rename r_id s = s.
+Lemma s_ren_id_l {Γ} (s : state Γ) : s ₛ⊛ᵣ r_id  = s.
   now apply (state_ind_mut _ _ _ ren_id_l_prf).
 Qed.
-Lemma v_ren_id_l {Γ} A (v : val Γ A) : v_rename r_id A v = v.
+Lemma v_ren_id_l {Γ} A (v : val Γ A) : v ᵥ⊛ᵣ r_id = v.
   destruct A as [ [] | [] ].
   now apply w_ren_id_l.
   now apply t_ren_id_l.
@@ -677,51 +764,50 @@ Lemma v_ren_id_l {Γ} A (v : val Γ A) : v_rename r_id A v = v.
   now apply w_ren_id_l.
 Qed.
 
-Lemma v_ren_id_r {Γ Δ} (f : Γ ⊆ Δ) A (i : Γ ∋ A) : v_rename f A (s_var A i) = s_var A (f A i).
-  destruct A as [ [] | [] ]; auto.
+Lemma v_ren_id_r {Γ Δ} (f : Γ ⊆ Δ) A (i : Γ ∋ A) : (var i) ᵥ⊛ᵣ f = var (f _ i).
+  now destruct A as [ [] | [] ].
 Qed.
 
-Lemma a_shift_id {Γ A} : @a_shift Γ Γ A s_var ≡ₐ s_var.
+Lemma a_shift1_id {Γ A} : @a_shift1 Γ Γ A var ≡ₐ var.
   intros [ [] | [] ] i; dependent elimination i; auto.
 Qed.
 
-Lemma a_shift2_id {Γ A B} : @a_shift2 Γ Γ A B s_var ≡ₐ s_var.
-  unfold a_shift2, v_shift2; intros ? h.
-  do 2 (dependent elimination h; cbn; auto).
-  now rewrite v_ren_id_r.
+Lemma a_shift2_id {Γ A B} : @a_shift2 Γ Γ A B var ≡ₐ var.
+  intros ? v; cbn.
+  do 2 (dependent elimination v; cbn; auto).
+  now destruct a as [[]|[]].
 Qed.
 
-Lemma a_shift_a_ren {Γ1 Γ2 Γ3 y} (f1 : Γ2 ⊆ Γ3) (f2 : Γ1 =[ val ]> Γ2)
-      : a_shift (y:=y) (a_ren f1 f2) ≡ₐ a_ren (r_shift f1) (a_shift f2) .
-  unfold r_shift, a_shift, a_ren, v_shift; intros ? h.
-  dependent elimination h; cbn.
+Arguments var : simpl never.
+Lemma a_shift1_ren_r {Γ1 Γ2 Γ3 y} (f1 : Γ1 =[ val ]> Γ2) (f2 : Γ2 ⊆ Γ3)
+      : a_shift1 (y:=y) (f1 ⊛ᵣ f2) ≡ₐ a_shift1 f1 ⊛ᵣ r_shift1 f2 .
+  intros ? h; dependent elimination h; cbn.
   - now rewrite v_ren_id_r.
-  - now rewrite 2 v_ren_ren, a_append_pop.
+  - now unfold v_shift1; rewrite 2 v_ren_ren.
 Qed.
 
-Lemma a_shift_s_ren {Γ1 Γ2 Γ3 y} (f1 : Γ2 =[val]> Γ3) (f2 : Γ1 ⊆ Γ2)
-  : a_shift (y:=y) (s_ren f1 f2) ≡ₐ s_ren (a_shift f1) (r_shift f2) .
+Lemma a_shift2_ren_r {Γ1 Γ2 Γ3 y z} (f1 : Γ1 =[ val ]> Γ2) (f2 : Γ2 ⊆ Γ3)
+      : a_shift2 (y:=y) (z:=z) (f1 ⊛ᵣ f2) ≡ₐ a_shift2 f1 ⊛ᵣ r_shift2 f2 .
+  intros ? v; do 2 (dependent elimination v; cbn; [ now rewrite v_ren_id_r | ]).
+  unfold v_shift2; now rewrite 2 v_ren_ren.
+Qed.
+
+Lemma a_shift1_ren_l {Γ1 Γ2 Γ3 y} (f1 : Γ1 ⊆ Γ2) (f2 : Γ2 =[val]> Γ3)
+  : a_shift1 (y:=y) (f1 ᵣ⊛ f2) ≡ₐ r_shift1 f1 ᵣ⊛ a_shift1 f2 .
   intros ? i; dependent elimination i; auto.
 Qed.
 
-Lemma a_shift2_s_ren {Γ1 Γ2 Γ3 A B} (f1 : Γ2 =[val]> Γ3) (f2 : Γ1 ⊆ Γ2)
-  : @a_shift2 _ _ A B (s_ren f1 f2) ≡ₐ s_ren (a_shift2 f1) (r_shift2 f2) .
-  intros ? h; do 2 (dependent elimination h; auto).
-Qed.
-
-Lemma a_shift2_a_ren {Γ1 Γ2 Γ3 A B} (f1 : Γ2 ⊆ Γ3) (f2 : Γ1 =[ val ]> Γ2)
-      : @a_shift2 _ _ A B (a_ren f1 f2) ≡ₐ a_ren (r_shift2 f1) (a_shift2 f2) .
-  unfold r_shift2, r_shift, a_shift2, v_shift2, a_ren; intros ? h.
-  do 2 (dependent elimination h; cbn; [ now rewrite v_ren_id_r | ]).
-  rewrite 2 v_ren_ren; now apply v_ren_eq.
+Lemma a_shift2_ren_l {Γ1 Γ2 Γ3 y z} (f1 : Γ1 ⊆ Γ2) (f2 : Γ2 =[val]> Γ3)
+      : a_shift2 (y:=y) (z:=z) (f1 ᵣ⊛ f2) ≡ₐ r_shift2 f1 ᵣ⊛ a_shift2 f2 .
+  intros ? v; do 2 (dependent elimination v; auto).
 Qed.
 
 Definition t_sub_proper_P Γ A (t : term Γ A) : Prop :=
-  forall Δ (f1 f2 : Γ =[val]> Δ), f1 ≡ₐ f2 -> t_subst f1 A t = t_subst f2 A t .
+  forall Δ (f1 f2 : Γ =[val]> Δ), f1 ≡ₐ f2 -> t `ₜ⊛ f1 = t `ₜ⊛ f2 .
 Definition w_sub_proper_P Γ A (v : whn Γ A) : Prop :=
-  forall Δ (f1 f2 : Γ =[val]> Δ), f1 ≡ₐ f2 -> w_subst f1 A v = w_subst f2 A v .
+  forall Δ (f1 f2 : Γ =[val]> Δ), f1 ≡ₐ f2 -> v `ᵥ⊛ f1 = v `ᵥ⊛ f2 .
 Definition s_sub_proper_P Γ (s : state Γ) : Prop :=
-  forall Δ (f1 f2 : Γ =[val]> Δ), f1 ≡ₐ f2 -> s_subst f1 s = s_subst f2 s .
+  forall Δ (f1 f2 : Γ =[val]> Δ), f1 ≡ₐ f2 -> s ₜ⊛ f1 = s ₜ⊛ f2 .
 
 Lemma sub_proper_prf : syn_ind_args t_sub_proper_P w_sub_proper_P s_sub_proper_P.
   econstructor.
@@ -731,53 +817,44 @@ Lemma sub_proper_prf : syn_ind_args t_sub_proper_P w_sub_proper_P s_sub_proper_P
        | |- Whn _ = Whn _ => do 2 f_equal
        | _ => f_equal
        end .
-  all: try apply H; try apply H1; try apply H2; auto.
-  all: match goal with
-       | |- a_shift _ ≡ₐ a_shift _ => now apply a_shift_eq
-       | |- a_shift2 _ ≡ₐ a_shift2 _ => now apply a_shift2_eq
-       end .
+  all: first [ apply H | apply H1 | apply H2 ]; auto.
+  all: first [ apply a_shift1_eq | apply a_shift2_eq ]; auto.
 Qed.
 
-#[global] Instance t_sub_eq {Γ Δ}
-  : Proper (ass_eq _ _ ==> forall_relation (fun _ => eq ==> eq)) (@t_subst Γ Δ).
-  intros f1 f2 H1 a x y ->; now apply (term_ind_mut _ _ _ sub_proper_prf).
+#[global] Instance t_sub_eq {Γ a t Δ} : Proper (asgn_eq _ _ ==> eq) (t_subst Γ a t Δ).
+  intros f1 f2 H1; now apply (term_ind_mut _ _ _ sub_proper_prf).
 Qed.
 
-#[global] Instance w_sub_eq {Γ Δ}
-  : Proper (ass_eq _ _ ==> forall_relation (fun _ => eq ==> eq)) (@w_subst Γ Δ).
-  intros f1 f2 H1 a x y ->; now apply (whn_ind_mut _ _ _ sub_proper_prf).
+#[global] Instance w_sub_eq {Γ a v Δ} : Proper (asgn_eq _ _ ==> eq) (w_subst Γ a v Δ).
+  intros f1 f2 H1; now apply (whn_ind_mut _ _ _ sub_proper_prf).
 Qed.
 
-#[global] Instance s_sub_eq {Γ Δ}
-  : Proper (ass_eq _ _ ==> eq ==> eq) (@s_subst Γ Δ).
-  intros f1 f2 H1 x y ->; now apply (state_ind_mut _ _ _ sub_proper_prf).
+#[global] Instance s_sub_eq {Γ s Δ} : Proper (asgn_eq _ _ ==> eq) (s_subst Γ s Δ).
+  intros f1 f2 H1; now apply (state_ind_mut _ _ _ sub_proper_prf).
 Qed.
 
-#[global] Instance v_sub_eq {Γ Δ}
-  : Proper (ass_eq _ _ ==> forall_relation (fun _ => eq ==> eq)) (@v_subst Γ Δ).
-  intros f1 f2 H1 [ [] | [] ] v1 v2 H2.
+#[global] Instance v_sub_eq {Γ a v Δ} : Proper (asgn_eq _ _ ==> eq) (v_subst Γ a v Δ).
+  destruct a as [[]|[]].
   - now apply w_sub_eq.
   - now apply t_sub_eq.
   - now apply t_sub_eq.
   - now apply w_sub_eq.
 Qed.
 
-#[global] Instance a_comp_eq {Γ1 Γ2 Γ3} : Proper (ass_eq _ _ ==> ass_eq _ _ ==> ass_eq _ _) (@a_comp Γ1 Γ2 Γ3).
-  intros ? ? H1 ? ? H2 ? ?; apply v_sub_eq; [ apply H1 | apply H2 ].
+#[global] Instance a_comp_eq {Γ1 Γ2 Γ3}
+  : Proper (asgn_eq _ _ ==> asgn_eq _ _ ==> asgn_eq _ _) (@a_comp _ _ _ _ _ Γ1 Γ2 Γ3).
+  intros ? ? H1 ? ? H2 ? ?; cbn; rewrite H1; now eapply v_sub_eq.
 Qed.
 
 Definition t_ren_sub_P Γ1 A (t : term Γ1 A) : Prop :=
-  forall Γ2 Γ3 (f1 : Γ2 ⊆ Γ3) (f2 : Γ1 =[val]> Γ2),
-    t_rename f1 A (t_subst f2 A t)
-    = t_subst (a_ren f1 f2) A t .
+  forall Γ2 Γ3 (f1 : Γ1 =[val]> Γ2) (f2 : Γ2 ⊆ Γ3),
+    (t `ₜ⊛ f1) ₜ⊛ᵣ f2 = t `ₜ⊛ (f1 ⊛ᵣ f2) .
 Definition w_ren_sub_P Γ1 A (v : whn Γ1 A) : Prop :=
-  forall Γ2 Γ3 (f1 : Γ2 ⊆ Γ3) (f2 : Γ1 =[val]> Γ2),
-    v_rename f1 A (w_subst f2 A v)
-    = w_subst (a_ren f1 f2) A v .
+  forall Γ2 Γ3 (f1 : Γ1 =[val]> Γ2) (f2 : Γ2 ⊆ Γ3),
+    (v `ᵥ⊛ f1) ᵥ⊛ᵣ f2 = v `ᵥ⊛ (f1 ⊛ᵣ f2) .
 Definition s_ren_sub_P Γ1 (s : state Γ1) : Prop :=
-  forall Γ2 Γ3 (f1 : Γ2 ⊆ Γ3) (f2 : Γ1 =[val]> Γ2),
-    s_rename f1 (s_subst f2 s)
-    = s_subst (a_ren f1 f2) s .
+  forall Γ2 Γ3 (f1 : Γ1 =[val]> Γ2) (f2 : Γ2 ⊆ Γ3),
+    (s ₜ⊛ f1) ₛ⊛ᵣ f2 = s ₜ⊛ (f1 ⊛ᵣ f2) .
 Lemma ren_sub_prf : syn_ind_args t_ren_sub_P w_ren_sub_P s_ren_sub_P.
   econstructor.
   all: unfold t_ren_sub_P, w_ren_sub_P, s_ren_sub_P.
@@ -786,26 +863,24 @@ Lemma ren_sub_prf : syn_ind_args t_ren_sub_P w_ren_sub_P s_ren_sub_P.
   all: match goal with
        | |- Whn _ = Whn _ => do 2 f_equal
        | _ => f_equal
-       end .
-  all: try rewrite a_shift_a_ren; try rewrite a_shift2_a_ren; auto.
-  all: try change (w_rename ?f ?a ?b) with (v_rename f a b).
-  all: try apply H; try apply H1; try apply H2; auto.
+       end ; eauto.
+  all: first [ rewrite a_shift1_ren_r | rewrite a_shift2_ren_r ]; auto.
 Qed.
 
-Lemma t_ren_sub {Γ1 Γ2 Γ3} (f1 : Γ2 ⊆ Γ3) (f2 : Γ1 =[val]> Γ2) A (t : term Γ1 A)
-  : t_rename f1 A (t_subst f2 A t) = t_subst (a_ren f1 f2) A t.
+Lemma t_ren_sub {Γ1 Γ2 Γ3} (f1 : Γ1 =[val]> Γ2) (f2 : Γ2 ⊆ Γ3) A (t : term Γ1 A)
+  : (t `ₜ⊛ f1) ₜ⊛ᵣ f2 = t `ₜ⊛ (f1 ⊛ᵣ f2) .
   now apply (term_ind_mut _ _ _ ren_sub_prf).
 Qed.
-Lemma w_ren_sub {Γ1 Γ2 Γ3} (f1 : Γ2 ⊆ Γ3) (f2 : Γ1 =[val]> Γ2) A (v : whn Γ1 A)
-  : v_rename f1 A (w_subst f2 A v) = w_subst (a_ren f1 f2) A v.
+Lemma w_ren_sub {Γ1 Γ2 Γ3} (f1 : Γ1 =[val]> Γ2) (f2 : Γ2 ⊆ Γ3) A (v : whn Γ1 A)
+  : (v `ᵥ⊛ f1) ᵥ⊛ᵣ f2 = v `ᵥ⊛ (f1 ⊛ᵣ f2) .
   now apply (whn_ind_mut _ _ _ ren_sub_prf).
 Qed.
-Lemma s_ren_sub {Γ1 Γ2 Γ3} (f1 : Γ2 ⊆ Γ3) (f2 : Γ1 =[val]> Γ2) (s : state Γ1)
-  : s_rename f1 (s_subst f2 s) = s_subst (a_ren f1 f2) s.
+Lemma s_ren_sub {Γ1 Γ2 Γ3} (f1 : Γ1 =[val]> Γ2) (f2 : Γ2 ⊆ Γ3) (s : state Γ1)
+  : (s ₜ⊛ f1) ₛ⊛ᵣ f2 = s ₜ⊛ (f1 ⊛ᵣ f2) .
   now apply (state_ind_mut _ _ _ ren_sub_prf).
 Qed.
-Lemma v_ren_sub {Γ1 Γ2 Γ3} (f1 : Γ2 ⊆ Γ3) (f2 : Γ1 =[val]> Γ2) A (v : val Γ1 A)
-  : v_rename f1 A (v_subst f2 A v) = v_subst (a_ren f1 f2) A v.
+Lemma v_ren_sub {Γ1 Γ2 Γ3} (f1 : Γ1 =[val]> Γ2) (f2 : Γ2 ⊆ Γ3) A (v : val Γ1 A)
+  : (v ᵥ⊛ f1) ᵥ⊛ᵣ f2 = v ᵥ⊛ (f1 ⊛ᵣ f2) .
   destruct A as [ [] | [] ]; cbn [ v_subst ].
   - now apply w_ren_sub.
   - now apply t_ren_sub.
@@ -814,17 +889,14 @@ Lemma v_ren_sub {Γ1 Γ2 Γ3} (f1 : Γ2 ⊆ Γ3) (f2 : Γ1 =[val]> Γ2) A (v : v
 Qed.
 
 Definition t_sub_ren_P Γ1 A (t : term Γ1 A) : Prop :=
-  forall Γ2 Γ3 (f1 : Γ2 =[val]> Γ3) (f2 : Γ1 ⊆ Γ2),
-    t_subst f1 A (t_rename f2 A t)
-    = t_subst (s_ren f1 f2) A t .
+  forall Γ2 Γ3 (f1 : Γ1 ⊆ Γ2) (f2 : Γ2 =[val]> Γ3),
+    (t ₜ⊛ᵣ f1) `ₜ⊛ f2 = t `ₜ⊛ (f1 ᵣ⊛ f2).
 Definition w_sub_ren_P Γ1 A (v : whn Γ1 A) : Prop :=
-  forall Γ2 Γ3 (f1 : Γ2 =[val]> Γ3) (f2 : Γ1 ⊆ Γ2),
-    w_subst f1 A (w_rename f2 A v)
-    = w_subst (s_ren f1 f2) A v .
+  forall Γ2 Γ3 (f1 : Γ1 ⊆ Γ2) (f2 : Γ2 =[val]> Γ3),
+    (v `ᵥ⊛ᵣ f1) `ᵥ⊛ f2 = v `ᵥ⊛ (f1 ᵣ⊛ f2).
 Definition s_sub_ren_P Γ1 (s : state Γ1) : Prop :=
-  forall Γ2 Γ3 (f1 : Γ2 =[val]> Γ3) (f2 : Γ1 ⊆ Γ2),
-    s_subst f1 (s_rename f2 s)
-    = s_subst (s_ren f1 f2) s .
+  forall Γ2 Γ3 (f1 : Γ1 ⊆ Γ2) (f2 : Γ2 =[val]> Γ3),
+    (s ₛ⊛ᵣ f1) ₜ⊛ f2 = s ₜ⊛ (f1 ᵣ⊛ f2).
 
 Lemma sub_ren_prf : syn_ind_args t_sub_ren_P w_sub_ren_P s_sub_ren_P.
   econstructor.
@@ -833,24 +905,24 @@ Lemma sub_ren_prf : syn_ind_args t_sub_ren_P w_sub_ren_P s_sub_ren_P.
   all: match goal with
        | |- Whn _ = Whn _ => do 2 f_equal
        | _ => f_equal
-       end .
-  all: try rewrite a_shift_s_ren; try rewrite a_shift2_s_ren; auto.
+       end ; eauto.
+  all: first [ rewrite a_shift1_ren_l | rewrite a_shift2_ren_l ]; auto.
 Qed.
 
-Lemma t_sub_ren {Γ1 Γ2 Γ3} (f1 : Γ2 =[val]> Γ3) (f2 : Γ1 ⊆ Γ2) A (t : term Γ1 A)
-  : t_subst f1 A (t_rename f2 A t) = t_subst (s_ren f1 f2) A t.
+Lemma t_sub_ren {Γ1 Γ2 Γ3} (f1 : Γ1 ⊆ Γ2) (f2 : Γ2 =[val]> Γ3) A (t : term Γ1 A)
+  : (t ₜ⊛ᵣ f1) `ₜ⊛ f2 = t `ₜ⊛ (f1 ᵣ⊛ f2).
   now apply (term_ind_mut _ _ _ sub_ren_prf).
 Qed.
-Lemma w_sub_ren {Γ1 Γ2 Γ3} (f1 : Γ2 =[val]> Γ3) (f2 : Γ1 ⊆ Γ2) A (v : whn Γ1 A)
-  : w_subst f1 A (w_rename f2 A v) = w_subst (s_ren f1 f2) A v.
+Lemma w_sub_ren {Γ1 Γ2 Γ3} (f1 : Γ1 ⊆ Γ2) (f2 : Γ2 =[val]> Γ3) A (v : whn Γ1 A)
+  : (v `ᵥ⊛ᵣ f1) `ᵥ⊛ f2 = v `ᵥ⊛ (f1 ᵣ⊛ f2).
   now apply (whn_ind_mut _ _ _ sub_ren_prf).
 Qed.
-Lemma s_sub_ren {Γ1 Γ2 Γ3} (f1 : Γ2 =[val]> Γ3) (f2 : Γ1 ⊆ Γ2) (s : state Γ1)
-  : s_subst f1 (s_rename f2 s) = s_subst (s_ren f1 f2) s.
+Lemma s_sub_ren {Γ1 Γ2 Γ3} (f1 : Γ1 ⊆ Γ2) (f2 : Γ2 =[val]> Γ3) (s : state Γ1)
+  : (s ₛ⊛ᵣ f1) ₜ⊛ f2 = s ₜ⊛ (f1 ᵣ⊛ f2).
   now apply (state_ind_mut _ _ _ sub_ren_prf).
 Qed.
-Lemma v_sub_ren {Γ1 Γ2 Γ3} (f1 : Γ2 =[val]> Γ3) (f2 : Γ1 ⊆ Γ2) A (v : val Γ1 A)
-  : v_subst f1 A (v_rename f2 A v) = v_subst (s_ren f1 f2) A v.
+Lemma v_sub_ren {Γ1 Γ2 Γ3} (f1 : Γ1 ⊆ Γ2) (f2 : Γ2 =[val]> Γ3) A (v : val Γ1 A)
+  : (v ᵥ⊛ᵣ f1) ᵥ⊛ f2 = v ᵥ⊛ (f1 ᵣ⊛ f2).
   destruct A as [ [] | [] ].
   - now apply w_sub_ren.
   - now apply t_sub_ren.
@@ -858,33 +930,32 @@ Lemma v_sub_ren {Γ1 Γ2 Γ3} (f1 : Γ2 =[val]> Γ3) (f2 : Γ1 ⊆ Γ2) A (v : v
   - now apply w_sub_ren.
 Qed.
 
-Lemma v_sub_id_r {Γ Δ} (f : Γ =[val]> Δ) A (i : Γ ∋ A) : v_subst f A (s_var A i) = f A i.
+Lemma v_sub_id_r {Γ Δ} (f : Γ =[val]> Δ) A (i : Γ ∋ A) : var i ᵥ⊛ f = f A i.
   destruct A as [ [] | [] ]; auto.
 Qed.
 
-Lemma a_shift_comp {Γ1 Γ2 Γ3 A} (f1 : Γ2 =[val]> Γ3) (f2 : Γ1 =[val]> Γ2)
-  : @a_shift _ _ A (a_comp f1 f2) ≡ₐ a_comp (a_shift f1) (a_shift f2) .
-  intros x i; dependent elimination i; unfold a_shift, a_comp, v_shift; cbn.
+Lemma a_shift1_comp {Γ1 Γ2 Γ3 A} (f1 : Γ1 =[val]> Γ2) (f2 : Γ2 =[val]> Γ3)
+  : @a_shift1 _ _ A (f1 ⊛ f2) ≡ₐ a_shift1 f1 ⊛ a_shift1 f2 .
+  intros x i; dependent elimination i; cbn.
   - now rewrite v_sub_id_r.
-  - rewrite v_ren_sub, v_sub_ren; now apply v_sub_eq.
+  - now unfold v_shift1; rewrite v_ren_sub, v_sub_ren.
 Qed.
 
-Lemma a_shift2_comp {Γ1 Γ2 Γ3 A B} (f1 : Γ2 =[val]> Γ3) (f2 : Γ1 =[val]> Γ2)
-  : @a_shift2 _ _ A B (a_comp f1 f2) ≡ₐ a_comp (a_shift2 f1) (a_shift2 f2) .
-  unfold a_shift2, v_shift2, a_comp; intros ? h.
-  do 2 (dependent elimination h; cbn; [ now rewrite v_sub_id_r | ]).
-  rewrite v_ren_sub, v_sub_ren; now apply v_sub_eq.
+Lemma a_shift2_comp {Γ1 Γ2 Γ3 A B} (f1 : Γ1 =[val]> Γ2) (f2 : Γ2 =[val]> Γ3)
+  : @a_shift2 _ _ A B (f1 ⊛ f2) ≡ₐ a_shift2 f1 ⊛ a_shift2 f2 .
+  intros ? v; do 2 (dependent elimination v; cbn; [ now rewrite v_sub_id_r | ]).
+  now unfold v_shift2; rewrite v_ren_sub, v_sub_ren.
 Qed.
 
 Definition t_sub_sub_P Γ1 A (t : term Γ1 A) : Prop :=
-  forall Γ2 Γ3 (f1 : Γ2 =[val]> Γ3) (f2 : Γ1 =[val]> Γ2),
-    t_subst f1 A (t_subst f2 A t) = t_subst (a_comp f1 f2) A t.
+  forall Γ2 Γ3 (f1 : Γ1 =[val]> Γ2) (f2 : Γ2 =[val]> Γ3),
+    (t `ₜ⊛ f1) `ₜ⊛ f2 = t `ₜ⊛ (f1 ⊛ f2) .
 Definition w_sub_sub_P Γ1 A (v : whn Γ1 A) : Prop :=
-  forall Γ2 Γ3 (f1 : Γ2 =[val]> Γ3) (f2 : Γ1 =[val]> Γ2),
-    v_subst f1 A (w_subst f2 A v) = w_subst (a_comp f1 f2) A v.
+  forall Γ2 Γ3 (f1 : Γ1 =[val]> Γ2) (f2 : Γ2 =[val]> Γ3),
+    (v `ᵥ⊛ f1) ᵥ⊛ f2 = v `ᵥ⊛ (f1 ⊛ f2) .
 Definition s_sub_sub_P Γ1 (s : state Γ1) : Prop :=
-  forall Γ2 Γ3 (f1 : Γ2 =[val]> Γ3) (f2 : Γ1 =[val]> Γ2),
-    s_subst f1 (s_subst f2 s) = s_subst (a_comp f1 f2) s.
+  forall Γ2 Γ3 (f1 : Γ1 =[val]> Γ2) (f2 : Γ2 =[val]> Γ3),
+    (s ₜ⊛ f1) ₜ⊛ f2 = s ₜ⊛ (f1 ⊛ f2) .
 
 Lemma sub_sub_prf : syn_ind_args t_sub_sub_P w_sub_sub_P s_sub_sub_P.
   econstructor.
@@ -893,27 +964,24 @@ Lemma sub_sub_prf : syn_ind_args t_sub_sub_P w_sub_sub_P s_sub_sub_P.
   all: match goal with
        | |- Whn _ = Whn _ => do 2 f_equal
        | _ => f_equal
-       end .
-  all: try rewrite a_shift_comp; try rewrite a_shift2_comp; auto.
-  all: try change (w_subst ?f ?a ?b) with (v_subst f a b).
-  all: try change (t_subst ?f ?a ?b) with (v_subst f a b).
-  all: try apply H; try apply H1; try apply H2; auto.
+       end ; eauto.
+  all: first [ rewrite a_shift1_comp | rewrite a_shift2_comp ]; auto.
 Qed.
 
-Lemma t_sub_sub {Γ1 Γ2 Γ3} (f1 : Γ2 =[val]> Γ3) (f2 : Γ1 =[val]> Γ2) A (t : term Γ1 A)
-  : t_subst f1 A (t_subst f2 A t) = t_subst (a_comp f1 f2) A t.
+Lemma t_sub_sub {Γ1 Γ2 Γ3} (f1 : Γ1 =[val]> Γ2) (f2 : Γ2 =[val]> Γ3) A (t : term Γ1 A)
+  : (t `ₜ⊛ f1) `ₜ⊛ f2 = t `ₜ⊛ (f1 ⊛ f2) .
   now apply (term_ind_mut _ _ _ sub_sub_prf).
 Qed.
-Lemma w_sub_sub {Γ1 Γ2 Γ3} (f1 : Γ2 =[val]> Γ3) (f2 : Γ1 =[val]> Γ2) A (v : whn Γ1 A)
-  : v_subst f1 A (w_subst f2 A v) = w_subst (a_comp f1 f2) A v.
+Lemma w_sub_sub {Γ1 Γ2 Γ3} (f1 : Γ1 =[val]> Γ2) (f2 : Γ2 =[val]> Γ3) A (v : whn Γ1 A)
+  : (v `ᵥ⊛ f1) ᵥ⊛ f2 = v `ᵥ⊛ (f1 ⊛ f2) .
   now apply (whn_ind_mut _ _ _ sub_sub_prf).
 Qed.
-Lemma s_sub_sub {Γ1 Γ2 Γ3} (f1 : Γ2 =[val]> Γ3) (f2 : Γ1 =[val]> Γ2) (s : state Γ1)
-  : s_subst f1 (s_subst f2 s) = s_subst (a_comp f1 f2) s.
+Lemma s_sub_sub {Γ1 Γ2 Γ3} (f1 : Γ1 =[val]> Γ2) (f2 : Γ2 =[val]> Γ3) (s : state Γ1)
+  : (s ₜ⊛ f1) ₜ⊛ f2 = s ₜ⊛ (f1 ⊛ f2) .
   now apply (state_ind_mut _ _ _ sub_sub_prf).
 Qed.
-Lemma v_sub_sub {Γ1 Γ2 Γ3} (f1 : Γ2 =[val]> Γ3) (f2 : Γ1 =[val]> Γ2) A (v : val Γ1 A)
-  : v_subst f1 A (v_subst f2 A v) = v_subst (a_comp f1 f2) A v.
+Lemma v_sub_sub {Γ1 Γ2 Γ3} (f1 : Γ1 =[val]> Γ2) (f2 : Γ2 =[val]> Γ3) A (v : val Γ1 A)
+  : (v ᵥ⊛ f1) ᵥ⊛ f2 = v ᵥ⊛ (f1 ⊛ f2) .
   destruct A as [ [] | [] ].
   - now apply w_sub_sub.
   - now apply t_sub_sub.
@@ -921,14 +989,14 @@ Lemma v_sub_sub {Γ1 Γ2 Γ3} (f1 : Γ2 =[val]> Γ3) (f2 : Γ1 =[val]> Γ2) A (v
   - now apply w_sub_sub.
 Qed.
 
-Lemma a_comp_assoc {Γ1 Γ2 Γ3 Γ4} (u : Γ3 =[val]> Γ4) (v : Γ2 =[val]> Γ3) (w : Γ1 =[val]> Γ2)
-           : a_comp u (a_comp v w) ≡ₐ a_comp (a_comp u v) w .
+Lemma a_comp_assoc {Γ1 Γ2 Γ3 Γ4} (u : Γ1 =[val]> Γ2) (v : Γ2 =[val]> Γ3) (w : Γ3 =[val]> Γ4)
+           : (u ⊛ v) ⊛ w ≡ₐ u ⊛ (v ⊛ w).
   intros ? i; unfold a_comp; now apply v_sub_sub.
 Qed.
 
-Definition t_sub_id_l_P Γ A (t : term Γ A) : Prop := t_subst s_var A t = t.
-Definition w_sub_id_l_P Γ A (v : whn Γ A) : Prop := w_subst s_var A v = v_of_w A v.
-Definition s_sub_id_l_P Γ (s : state Γ) : Prop := s_subst s_var s = s.
+Definition t_sub_id_l_P Γ A (t : term Γ A) : Prop := t `ₜ⊛ var = t.
+Definition w_sub_id_l_P Γ A (v : whn Γ A) : Prop := v `ᵥ⊛ var = v_of_w _ v.
+Definition s_sub_id_l_P Γ (s : state Γ) : Prop := s ₜ⊛ var = s.
 
 Lemma sub_id_l_prf : syn_ind_args t_sub_id_l_P w_sub_id_l_P s_sub_id_l_P.
   econstructor.
@@ -937,20 +1005,20 @@ Lemma sub_id_l_prf : syn_ind_args t_sub_id_l_P w_sub_id_l_P s_sub_id_l_P.
   all: match goal with
        | |- Whn _ = Whn _ => do 2 f_equal
        | _ => f_equal
-       end; auto.
-  all: try rewrite a_shift_id; try rewrite a_shift2_id; auto.
+       end; eauto.
+  all: first [ rewrite a_shift1_id | rewrite a_shift2_id ]; auto.
 Qed.
 
-Lemma t_sub_id_l {Γ} A (t : term Γ A) : t_subst s_var A t = t.
+Lemma t_sub_id_l {Γ} A (t : term Γ A) : t `ₜ⊛ var = t.
   now apply (term_ind_mut _ _ _ sub_id_l_prf).
 Qed.
-Lemma w_sub_id_l {Γ} A (v : whn Γ A) : w_subst s_var A v = v_of_w A v.
+Lemma w_sub_id_l {Γ} A (v : whn Γ A) : v `ᵥ⊛ var = v_of_w _ v.
   now apply (whn_ind_mut _ _ _ sub_id_l_prf).
 Qed.
-Lemma s_sub_id_l {Γ} (s : state Γ) : s_subst s_var s = s.
+Lemma s_sub_id_l {Γ} (s : state Γ) : s ₜ⊛ var = s.
   now apply (state_ind_mut _ _ _ sub_id_l_prf).
 Qed.
-Lemma v_sub_id_l {Γ} A (v : val Γ A) : v_subst s_var A v = v.
+Lemma v_sub_id_l {Γ} A (v : val Γ A) : v ᵥ⊛ var = v.
   destruct A as [ [] | [] ].
   - now apply w_sub_id_l.
   - now apply t_sub_id_l.
@@ -959,332 +1027,106 @@ Lemma v_sub_id_l {Γ} A (v : val Γ A) : v_subst s_var A v = v.
 Qed.
 
 Lemma sub1_sub {Γ Δ A} (f : Γ =[val]> Δ) (v : val Γ A) :
-  a_comp (ass1 (v_subst f A v)) (a_shift f) ≡ₐ a_comp f (ass1 v).
-  intros ? h; dependent elimination h.
-  - unfold a_comp; cbn; now rewrite v_sub_id_r.
-  - unfold a_comp, a_shift, v_shift; cbn.
-    rewrite v_sub_ren, v_sub_id_r.
-    apply v_sub_id_l.
+  a_shift1 f ⊛ asgn1 (v ᵥ⊛ f) ≡ₐ asgn1 v ⊛ f.
+  intros ? h; dependent elimination h; cbn.
+  - now rewrite v_sub_id_r.
+  - unfold v_shift1; rewrite v_sub_ren, v_sub_id_r.
+    now apply v_sub_id_l.
 Qed.
 
 Lemma sub1_ren {Γ Δ A} (f : Γ ⊆ Δ) (v : val Γ A) :
-  ass1 (v_rename f A v) ⊛ᵣ r_shift f ≡ₐ a_ren f (ass1 v) .
+  r_shift1 f ᵣ⊛ asgn1 (v ᵥ⊛ᵣ f) ≡ₐ asgn1 v ⊛ᵣ f.
   intros ? h; dependent elimination h; auto.
-  unfold a_ren, ass1; cbn; now rewrite v_ren_id_r.
+  cbn; now rewrite v_ren_id_r.
 Qed.
 
-Lemma v_sub1_sub {Γ Δ A B} (f : Γ =[val]> Δ) (v : val Γ A) (w : val (Γ ▶ A) B)
-  : v_subst (a_shift f) B w ᵥ/[ v_subst f A v ] = v_subst f B (w ᵥ/[ v ]) .
-  unfold v_subst1; rewrite 2 v_sub_sub.
-  apply v_sub_eq; auto.
-  now rewrite sub1_sub.
+Lemma v_sub1_sub {Γ Δ A B} (f : Γ =[val]> Δ) (v : val Γ A) (w : val (Γ ▶ₓ A) B)
+  : (w ᵥ⊛ a_shift1 f) ᵥ⊛ ₁[ v ᵥ⊛ f ] = (w ᵥ⊛ ₁[ v ]) ᵥ⊛ f .
+  cbn; rewrite 2 v_sub_sub.
+  apply v_sub_eq; now rewrite sub1_sub.
 Qed.
 
-Lemma v_sub1_ren {Γ Δ A B} (f : Γ ⊆ Δ) (v : val Γ A) (w : val (Γ ▶ A) B)
-  : v_rename (r_shift f) B w ᵥ/[ v_rename f A v ] = v_rename f B (w ᵥ/[ v ]) .
-  unfold v_subst1; rewrite v_sub_ren, v_ren_sub.
-  apply v_sub_eq; auto.
-  now rewrite sub1_ren.
+Lemma v_sub1_ren {Γ Δ A B} (f : Γ ⊆ Δ) (v : val Γ A) (w : val (Γ ▶ₓ A) B)
+  : (w ᵥ⊛ᵣ r_shift1 f) ᵥ⊛ ₁[ v ᵥ⊛ᵣ f ] = (w ᵥ⊛ ₁[ v ]) ᵥ⊛ᵣ f .
+  cbn; rewrite v_sub_ren, v_ren_sub.
+  apply v_sub_eq; now rewrite sub1_ren.
 Qed.
 
-Lemma s_sub1_sub {Γ Δ A} (f : Γ =[val]> Δ) (v : val Γ A) (s : state (Γ ▶ A))
-  : s_subst (a_shift f) s ₛ/[ v_subst f A v ] = s_subst f (s ₛ/[ v ]) .
-  unfold s_subst1; now rewrite 2 s_sub_sub, sub1_sub.
+Lemma s_sub1_sub {Γ Δ A} (f : Γ =[val]> Δ) (v : val Γ A) (s : state (Γ ▶ₓ A))
+  : (s ₜ⊛ a_shift1 f) ₜ⊛ ₁[ v ᵥ⊛ f ] = (s ₜ⊛ ₁[ v ]) ₜ⊛ f .
+  cbn; now rewrite 2 s_sub_sub, sub1_sub.
 Qed.
 
-Lemma s_sub2_sub {Γ Δ A B} (f : Γ =[val]> Δ) (s : state (Γ ▶ A ▶ B)) u v
-  : s_subst (a_shift2 f) s ₛ/[ v_subst f A u , v_subst f B v ] = s_subst f (s ₛ/[ u , v ]) .
-  unfold s_subst2; rewrite 2 s_sub_sub; apply s_sub_eq; auto.
-  intros ? h; unfold a_comp, a_shift2, v_shift2.
-  do 2 (dependent elimination h; cbn; [ now rewrite v_sub_id_r | ]).
-  rewrite v_sub_ren, v_sub_id_r, <- v_sub_id_l.
+Lemma s_sub2_sub {Γ Δ A B} (f : Γ =[val]> Δ) (s : state (Γ ▶ₓ A ▶ₓ B)) u v
+  : (s ₜ⊛ a_shift2 f) ₜ⊛ ₂[ u ᵥ⊛ f , v ᵥ⊛ f ] = (s ₜ⊛ ₂[ u, v ]) ₜ⊛ f .
+  cbn; rewrite 2 s_sub_sub; apply s_sub_eq.
+  intros ? v0; cbn.
+  do 2 (dependent elimination v0; cbn; [ now rewrite v_sub_id_r | ]).
+  unfold v_shift2; rewrite v_sub_ren, v_sub_id_r, <- v_sub_id_l.
   now apply v_sub_eq.
 Qed.
 
-Lemma s_sub1_ren {Γ Δ A} (f : Γ ⊆ Δ) (v : val Γ A) (s : state (Γ ▶ A))
-  : s_rename (r_shift f) s ₛ/[ v_rename f A v ] = s_rename f (s ₛ/[ v ]) .
-  unfold s_subst1; now rewrite s_sub_ren, s_ren_sub, sub1_ren.
+Lemma s_sub1_ren {Γ Δ A} (f : Γ ⊆ Δ) (v : val Γ A) (s : state (Γ ▶ₓ A))
+  : (s ₛ⊛ᵣ r_shift1 f) ₜ⊛ ₁[ v ᵥ⊛ᵣ f ] = (s ₜ⊛ ₁[ v ]) ₛ⊛ᵣ f .
+  cbn; now rewrite s_sub_ren, s_ren_sub, sub1_ren.
 Qed.
 
-Lemma t_sub1_sub {Γ Δ A B} (f : Γ =[val]> Δ) (v : val Γ A) (t : term (Γ ▶ A) B)
-  : t_subst (a_shift f) B t ₜ/[ v_subst f A v ] = t_subst f B (t ₜ/[ v ]) .
-  unfold t_subst1; rewrite 2 t_sub_sub.
-  apply t_sub_eq; auto.
-  rewrite sub1_sub; reflexivity.
+Lemma t_sub1_sub {Γ Δ A B} (f : Γ =[val]> Δ) (v : val Γ A) (t : term (Γ ▶ₓ A) B)
+  : (t `ₜ⊛ a_shift1 f) `ₜ⊛ ₁[ v ᵥ⊛ f ] = (t `ₜ⊛ ₁[ v ]) `ₜ⊛ f .
+  cbn; rewrite 2 t_sub_sub.
+  apply t_sub_eq; now rewrite sub1_sub.
 Qed.
 
-Lemma t_sub1_ren {Γ Δ A B} (f : Γ ⊆ Δ) (v : val Γ A) (t : term (Γ ▶ A) B)
-  : t_rename (r_shift f) B t ₜ/[ v_rename f A v ] = t_rename f B (t ₜ/[ v ]) .
-  unfold t_subst1; rewrite t_sub_ren, t_ren_sub.
-  apply t_sub_eq; auto.
-  now rewrite sub1_ren.
+Lemma t_sub1_ren {Γ Δ A B} (f : Γ ⊆ Δ) (v : val Γ A) (t : term (Γ ▶ₓ A) B)
+  : (t ₜ⊛ᵣ r_shift1 f) `ₜ⊛ ₁[ v ᵥ⊛ᵣ f ] = (t `ₜ⊛ ₁[ v ]) ₜ⊛ᵣ f .
+  cbn; rewrite t_sub_ren, t_ren_sub.
+  apply t_sub_eq; now rewrite sub1_ren.
 Qed.
 
-#[global] Instance p_app_eq {Γ A} (v : val Γ A) (m : pat (t_neg A)) : Proper (ass_eq _ _ ==> eq) (p_app v m) .
-  intros u1 u2 H; destruct A as [ [] | []]; cbn; now erewrite (w_sub_eq u1 u2 H).
+#[global] Instance p_app_eq {Γ A} (v : val Γ A) (m : pat (t_neg A))
+  : Proper (asgn_eq _ _ ==> eq) (p_app v m) .
+  intros u1 u2 H; destruct A as [ [] | []]; cbn; now rewrite (w_sub_eq u1 u2 H).
 Qed.
 
 Definition refold_id_aux_P (Γ : neg_ctx) p : ty0 p -> Prop :=
   match p with
-  | pos => fun A => forall (v : whn Γ (t+ A)), w_subst (p_dom_of_w_0p A v) (t+ A) (w_of_p (p_of_w_0p A v)) = v
-  | neg => fun A => forall (v : whn Γ (t- A)), w_subst (p_dom_of_w_0n A v) (t- A) (w_of_p (p_of_w_0n A v)) = v
+  | pos => fun A => forall (v : whn Γ `+A), w_of_p (p_of_w_0p _ v) `ᵥ⊛ p_dom_of_w_0p _ v = v
+  | neg => fun A => forall (v : whn Γ `-A), w_of_p (p_of_w_0n _ v) `ᵥ⊛ p_dom_of_w_0n _ v = v
   end .
 
 Lemma refold_id_aux {Γ p} A : refold_id_aux_P Γ p A .
   induction A; intros v.
-  - dependent elimination v.
-    pose (nope := (s_elt_upg h).(sub_prf)); dependent elimination nope.
-  - dependent elimination v.
-    pose (nope := (s_elt_upg h).(sub_prf)); dependent elimination nope.
-  - dependent elimination v.
-    pose (nope := (s_elt_upg h).(sub_prf)); dependent elimination nope.
-    reflexivity.
-  - dependent elimination v.
-    pose (nope := (s_elt_upg h).(sub_prf)); dependent elimination nope.
-    reflexivity.
-  - dependent elimination v.
-    pose (nope := (s_elt_upg h).(sub_prf)); dependent elimination nope.
-    change (w_subst _ _ _) with
-      (w_subst ([ p_dom_of_w_0p A0 w , p_dom_of_w_0p B w0 ]) _
-         (TenR (w_rename r_concat_l _ (w_of_p (p_of_w_0p A0 w)))
-               (w_rename r_concat_r _ (w_of_p (p_of_w_0p B w0))))); cbn.
-    rewrite 2 w_sub_ren.
-    erewrite (w_sub_eq _ _ (s_eq_cat_l _ _)); auto.
-    erewrite (w_sub_eq _ _ (s_eq_cat_r _ _)); auto.
-    f_equal; [ apply IHA1 | apply IHA2 ].
-  - dependent elimination v.
-    pose (nope := (s_elt_upg h).(sub_prf)); dependent elimination nope.
-    change (w_subst _ _ _) with
-      (w_subst ([ p_dom_of_w_0n A5 w1 , p_dom_of_w_0n B2 w2 ]) _
-         (ParL (w_rename r_concat_l _ (w_of_p (p_of_w_0n A5 w1)))
-               (w_rename r_concat_r _ (w_of_p (p_of_w_0n B2 w2))))); cbn.
-    rewrite 2 w_sub_ren.
-    erewrite (w_sub_eq _ _ (s_eq_cat_l _ _)); auto.
-    erewrite (w_sub_eq _ _ (s_eq_cat_r _ _)); auto.
-    f_equal; [ apply IHA1 | apply IHA2 ].
-  - dependent elimination v.
-    pose (nope := (s_elt_upg h).(sub_prf)); dependent elimination nope.
-    exact (f_equal OrR1 (IHA1 w3)).
-    exact (f_equal OrR2 (IHA2 w4)).
-  - dependent elimination v.
-    pose (nope := (s_elt_upg h).(sub_prf)); dependent elimination nope.
-    exact (f_equal AndL1 (IHA1 w5)).
-    exact (f_equal AndL2 (IHA2 w6)).
-  - dependent elimination v.
-    pose (nope := (s_elt_upg h).(sub_prf)); dependent elimination nope.
-    reflexivity.
-  - dependent elimination v.
-    pose (nope := (s_elt_upg h).(sub_prf)); dependent elimination nope.
-    reflexivity.
-  - dependent elimination v.
-    pose (nope := (s_elt_upg h).(sub_prf)); dependent elimination nope.
-    exact (f_equal NegPR (IHA w7)).
-  - dependent elimination v.
-    pose (nope := (s_elt_upg h).(sub_prf)); dependent elimination nope.
-    exact (f_equal NegNL (IHA w8)).
+  - dependent elimination v; destruct (s_prf c).
+  - dependent elimination v; destruct (s_prf c).
+  - dependent elimination v; [ destruct (s_prf c) | ]; auto.
+  - dependent elimination v; [ destruct (s_prf c) | ]; auto.
+  - dependent elimination v; [ destruct (s_prf c) | ].
+    cbn; f_equal; rewrite w_sub_ren.
+    rewrite <- IHA1; apply w_sub_eq; exact (a_cat_proj_l _ _).
+    rewrite <- IHA2; apply w_sub_eq; exact (a_cat_proj_r _ _).
+  - dependent elimination v; [ destruct (s_prf c) | ].
+    cbn; f_equal; rewrite w_sub_ren.
+    rewrite <- IHA1; apply w_sub_eq; exact (a_cat_proj_l _ _).
+    rewrite <- IHA2; apply w_sub_eq; exact (a_cat_proj_r _ _).
+  - dependent elimination v; [ destruct (s_prf c) | | ];
+      cbn; f_equal; [ apply IHA1 | apply IHA2 ].
+  - dependent elimination v; [ destruct (s_prf c) | | ];
+      cbn; f_equal; [ apply IHA1 | apply IHA2 ].
+  - dependent elimination v; [ destruct (s_prf c) | ]; cbn; f_equal.
+  - dependent elimination v; [ destruct (s_prf c) | ]; cbn; f_equal.
+  - dependent elimination v; [ destruct (s_prf c) | ].
+    cbn; f_equal; apply IHA.
+  - dependent elimination v; [ destruct (s_prf c) | ].
+    cbn; f_equal; apply IHA.
 Qed.
 
 Lemma refold_id {Γ : neg_ctx} A (v : val Γ A)
-  : w_subst (p_dom_of_v A v) A (w_of_p (p_of_v A v)) = v.
-  destruct A as [ [] A | [] A ].
-  - apply (refold_id_aux A v).
-  - reflexivity.
-  - reflexivity.
-  - apply (refold_id_aux A v).
+  : w_of_p (p_of_v A v) `ᵥ⊛ p_dom_of_v A v = v.
+  destruct A as [ [] A | [] A ]; auto; exact (refold_id_aux A v).
 Qed.
 
-Lemma var_inj {Γ A} (i j : Γ ∋ A) (H : s_var A i = s_var A j) : i = j .
-  destruct A as [ [] | [] ] ; now dependent induction H.
-Qed.
-
-From Coinduction Require Import coinduction lattice rel tactics.
-From OGS.Utils Require Import Psh Rel.
-From OGS.ITree Require Import ITree Eq Structure.
-
-(* the final version we would like to have in the hypothesis, in terms of [p_app] *)
-Definition then_eval1 {Γ Δ : neg_ctx} (e : Γ =[val]> Δ) (n : nf Γ) : delay (nf Δ)
-  := eval (p_app (e _ (fst (projT2 n))) (projT1 (snd (projT2 n))) (a_comp e (projT2 (snd (projT2 n))))) .
-
-(* the clean version with simplified substitutions we would like to have in the proof *)
-Definition then_eval2 {Γ Δ : neg_ctx} (e : Γ =[val]> Δ) (n : nf Γ) : delay (nf Δ) :=
-  let '(i , v) := refold n in
-  eval (Cut' (t_of_v _ (e _ i)) (t_of_v _ (v_subst e _ v))).
-
-(* both are the same thing up to substitution shenenigans *)
-Lemma then_eval_eq {Γ Δ : neg_ctx} (e : Γ =[val]> Δ) (n : nf Γ) : then_eval1 e n ≊ then_eval2 e n.
-  unfold then_eval1, then_eval2, p_app, refold.
-  now rewrite <- w_sub_sub.
-Qed.
-
-(* we can prove the hypothesis:
-
-    eval (c / e) == eval c >>= λ n => eval (⌊ n ⌋ / e)
-*)
-
-Lemma fmap_comp_eq {Γ} {u v : delay (nf Γ)} : u ≋ v -> fmap_delay (pat_of_nf Γ) u ≊ fmap_delay (pat_of_nf Γ) v .
-  intro H.
-  unfold it_eq; revert u v H; coinduction L CIH; intros u v H.
-  unfold comp_eq in H; apply it_eq_step in H; cbn in *; unfold observe in H.
-  remember (_observe u) as ou; remember (_observe v) as ov; clear Heqou u Heqov v.
-  dependent elimination H; cbn; econstructor; auto.
-  destruct r1 as [ x1 [ i1 [ m1 e1 ] ] ].
-  destruct r2 as [ x2 [ i2 [ m2 e2 ] ] ].
-  destruct r_rel as [ H1 [ H2 [ H3 _ ] ] ]; cbn in *.
-  unfold pat_of_nf; cbn.
-  revert i1 m1 e1 H2 H3; rewrite H1; clear x1 H1; intros i1 m1 e1 H2 H3; cbn in H2,H3.
-  now rewrite H2,H3.
-  destruct q.
-Qed.
-
-Lemma clean_hyp {Γ Δ : neg_ctx} (c : state Γ) (e : Γ =[val]> Δ)
-   : eval (s_subst e c) ≊ bind_delay' (eval c) (then_eval1 e) .
-  transitivity (bind_delay' (eval c) (then_eval2 e)); cycle 1.
-  apply (proj1 (t_gfp (it_eq_map ∅ₑ (eqᵢ _)) _ _ _)).
-  eapply (it_eq_up2bind_t (eqᵢ _)); econstructor; auto.
-  intros [] ? ? <-; symmetry; exact (then_eval_eq e x1).
-  unfold iter_delay, it_eq, bind.
-  revert Γ c e; coinduction L CIH; intros Γ c e.
-  dependent elimination c.
-  destruct p.
-  - dependent elimination t0.
-    + cbn; econstructor.
-      change (t_subst e (t- A) t1) with (v_subst e (t- A) t1).
-      rewrite s_sub1_sub; apply CIH.
-    + dependent elimination t1.
-      * cbn; econstructor.
-        change (w_subst e (t+ A) w) with (v_subst e (t+ A) w).
-        rewrite s_sub1_sub; apply CIH.
-      * cbn; econstructor.
-        change (RecL (t_subst (a_shift e) (t- ?A) t0)) with (t_subst e (t- A) (RecL t0)).
-        change (t_subst ?f (t- ?A) ?w) with (v_subst f (t- A) w) at 2.
-        rewrite t_sub1_sub; apply CIH.
-      * dependent elimination w.
-        -- pose (nope := (s_elt_upg h).(sub_prf)); dependent elimination nope.
-        -- dependent elimination w0.
-           ++ unfold eval at 2; cbn -[eval then_eval2].
-              unfold then_eval2; simp eval_aux; cbn -[eval].
-              rewrite (refold_id_aux 1).
-              now change (it_eqF _ ?RX ?RY _ (observe ?a) (_observe ?b)) with (it_eq_map ∅ₑ RX RY T1_0 a b).
-           ++ cbn; econstructor; apply CIH.
-        -- dependent elimination w0.
-           ++ unfold eval at 2; cbn -[eval then_eval2].
-              unfold then_eval2; simp eval_aux; cbn -[eval].
-              rewrite (refold_id_aux (A1 ⊗ B0)).
-              now change (it_eqF _ ?RX ?RY _ (observe ?a) (_observe ?b)) with (it_eq_map ∅ₑ RX RY T1_0 a b).
-           ++ cbn; econstructor.
-              change (w_subst ?f (t+ ?A) ?w) with (v_subst f (t+ A) w).
-              rewrite s_sub2_sub; apply CIH.
-        -- dependent elimination w0.
-           ++ unfold eval at 2; cbn -[eval then_eval2].
-              unfold then_eval2; simp eval_aux; cbn -[eval].
-              rewrite (refold_id_aux (A5 ⊕ B4)).
-              now change (it_eqF _ ?RX ?RY _ (observe ?a) (_observe ?b)) with (it_eq_map ∅ₑ RX RY T1_0 a b).
-           ++ cbn; econstructor.
-              change (w_subst ?f (t+ ?A) ?w) with (v_subst f (t+ A) w).
-              rewrite s_sub1_sub; apply CIH.
-        -- dependent elimination w0.
-           ++ unfold eval at 2; cbn -[eval then_eval2].
-              unfold then_eval2; simp eval_aux; cbn -[eval].
-              rewrite (refold_id_aux (A6 ⊕ B5)).
-              now change (it_eqF _ ?RX ?RY _ (observe ?a) (_observe ?b)) with (it_eq_map ∅ₑ RX RY T1_0 a b).
-           ++ cbn; econstructor.
-              change (w_subst ?f (t+ ?A) ?w) with (v_subst f (t+ A) w).
-              rewrite s_sub1_sub; apply CIH.
-        -- dependent elimination w0.
-           ++ unfold eval at 2; cbn -[eval then_eval2].
-              unfold then_eval2; simp eval_aux; cbn -[eval].
-              rewrite (refold_id_aux (↓ A11)).
-              now change (it_eqF _ ?RX ?RY _ (observe ?a) (_observe ?b)) with (it_eq_map ∅ₑ RX RY T1_0 a b).
-           ++ cbn; econstructor.
-              change (Whn (ShiftPL (s_subst _ _))) with (t_subst e (t- _) (Whn (ShiftPL s7))).
-              change (t_subst ?f ?A ?w) with (v_subst f A w).
-              rewrite s_sub1_sub; apply CIH.
-        -- dependent elimination w0.
-           ++ unfold eval at 2; cbn -[eval then_eval2].
-              unfold then_eval2; simp eval_aux; cbn -[eval].
-              rewrite (refold_id_aux (⊖ A15)).
-              now change (it_eqF _ ?RX ?RY _ (observe ?a) (_observe ?b)) with (it_eq_map ∅ₑ RX RY T1_0 a b).
-           ++ cbn; econstructor.
-              change (w_subst ?f (t- ?A) ?w) with (v_subst f (t- A) w).
-              rewrite s_sub1_sub; apply CIH.
-  - dependent elimination t1.
-    + cbn; econstructor.
-      change (t_subst e (t+ A) t0) with (v_subst e (t+ A) t0).
-      rewrite s_sub1_sub; apply CIH.
-    + dependent elimination t0.
-      * cbn; econstructor.
-        change (w_subst e (t- A) w) with (v_subst e (t- A) w).
-        rewrite s_sub1_sub; apply CIH.
-      * cbn; econstructor.
-        change (RecR (t_subst (a_shift e) (t+ ?A) t1)) with (t_subst e (t+ A) (RecR t1)).
-        change (t_subst ?f (t+ ?A) ?w) with (v_subst f (t+ A) w) at 2.
-        rewrite t_sub1_sub; apply CIH.
-      * dependent elimination w.
-        -- pose (nope := (s_elt_upg h).(sub_prf)); dependent elimination nope.
-        -- dependent elimination w0.
-           ++ unfold eval at 2; cbn -[eval then_eval2].
-              unfold then_eval2; simp eval_aux; cbn -[eval].
-              now change (it_eqF _ ?RX ?RY _ (observe ?a) (_observe ?b)) with (it_eq_map ∅ₑ RX RY T1_0 a b).
-           ++ cbn; econstructor; apply CIH.
-        -- dependent elimination w0.
-           ++ unfold eval at 2; cbn -[eval then_eval2].
-              unfold then_eval2; simp eval_aux; cbn -[eval].
-              rewrite 2 w_sub_ren.
-              erewrite (w_sub_eq _ _ (s_eq_cat_l _ _)); auto.
-              erewrite (w_sub_eq _ _ (s_eq_cat_r _ _)); auto.
-              rewrite (refold_id_aux A4).
-              rewrite (refold_id_aux B3).
-              now change (it_eqF _ ?RX ?RY _ (observe ?a) (_observe ?b)) with (it_eq_map ∅ₑ RX RY T1_0 a b).
-           ++ cbn; econstructor.
-              change (w_subst ?f (t- ?A) ?w) with (v_subst f (t- A) w).
-              rewrite s_sub2_sub; apply CIH.
-        -- dependent elimination w0.
-           ++ unfold eval at 2; cbn -[eval then_eval2].
-              unfold then_eval2; simp eval_aux; cbn -[eval].
-              rewrite (refold_id_aux A9).
-              now change (it_eqF _ ?RX ?RY _ (observe ?a) (_observe ?b)) with (it_eq_map ∅ₑ RX RY T1_0 a b).
-           ++ cbn; econstructor.
-              change (w_subst ?f (t- ?A) ?w) with (v_subst f (t- A) w).
-              rewrite s_sub1_sub; apply CIH.
-        -- dependent elimination w0.
-           ++ unfold eval at 2; cbn -[eval then_eval2].
-              unfold then_eval2; simp eval_aux; cbn -[eval].
-              rewrite (refold_id_aux B9).
-              now change (it_eqF _ ?RX ?RY _ (observe ?a) (_observe ?b)) with (it_eq_map ∅ₑ RX RY T1_0 a b).
-           ++ cbn; econstructor.
-              change (w_subst ?f (t- ?A) ?w) with (v_subst f (t- A) w).
-              rewrite s_sub1_sub; apply CIH.
-        -- dependent elimination w0.
-           ++ unfold eval at 2; cbn -[eval then_eval2].
-              unfold then_eval2; simp eval_aux; cbn -[eval].
-              now change (it_eqF _ ?RX ?RY _ (observe ?a) (_observe ?b)) with (it_eq_map ∅ₑ RX RY T1_0 a b).
-           ++ cbn; econstructor.
-              change (Whn (ShiftNR (s_subst _ _))) with (t_subst e (t+ _) (Whn (ShiftNR s8))).
-              change (t_subst ?f ?A ?w) with (v_subst f A w).
-              rewrite s_sub1_sub; apply CIH.
-        -- dependent elimination w0.
-           ++ unfold eval at 2; cbn -[eval then_eval2].
-              unfold then_eval2; simp eval_aux; cbn -[eval].
-              rewrite (refold_id_aux A18).
-              now change (it_eqF _ ?RX ?RY _ (observe ?a) (_observe ?b)) with (it_eq_map ∅ₑ RX RY T1_0 a b).
-           ++ cbn; econstructor.
-              change (w_subst ?f (t+ ?A) ?w) with (v_subst f (t+ A) w).
-              rewrite s_sub1_sub; apply CIH.
-Qed.
-
-Definition is_var {Γ A} (v : val Γ A) : Type := sigT (fun i : Γ ∋ A => v = s_var A i) .
-Definition is_var_get {Γ A} {v : val Γ A} (p : is_var v) : Γ ∋ A := projT1 p .
-
-Lemma is_var_dec {Γ A} (v : val Γ A) : is_var v + (is_var v -> False) .
-  destruct A as [ [] A | [] A ].
-  2,3: dependent elimination v; [ apply inr; intros [ i H ]; inversion H | | ].
-  all: try dependent elimination v; try dependent elimination w.
-  all: try now (apply inr; intros [ i H ]; inversion H).
-  all: apply inl; econstructor; auto.
-Qed.
-
-Equations p_of_w_eq_aux_p {Γ : neg_ctx} (A : ty0 pos) (p : pat (t+ A)) (e : p_dom p =[val]> Γ)
-          : p_of_w_0p A (w_subst e (t+ A) (w_of_p p) : whn Γ (t+ A)) = p
+Equations p_of_w_eq_aux_p {Γ : neg_ctx} (A : ty0 pos) (p : pat `+A) (e : p_dom p =[val]> Γ)
+          : p_of_w_0p A (w_of_p p `ᵥ⊛ e) = p
           by struct p :=
   p_of_w_eq_aux_p (1)     (POne)       e := eq_refl ;
   p_of_w_eq_aux_p (A ⊗ B) (PTen p1 p2) e := f_equal2 PTen
@@ -1292,11 +1134,11 @@ Equations p_of_w_eq_aux_p {Γ : neg_ctx} (A : ty0 pos) (p : pat (t+ A)) (e : p_d
         (eq_trans (f_equal _ (w_sub_ren _ _ _ _)) (p_of_w_eq_aux_p B p2 _)) ;
   p_of_w_eq_aux_p (A ⊕ B) (POr1 p)     e := f_equal POr1 (p_of_w_eq_aux_p A p e) ;
   p_of_w_eq_aux_p (A ⊕ B) (POr2 p)     e := f_equal POr2 (p_of_w_eq_aux_p B p e) ;
-  p_of_w_eq_aux_p (↓ A)  (PShiftP _)  e := eq_refl ;
+  p_of_w_eq_aux_p (↓ A)   (PShiftP _)  e := eq_refl ;
   p_of_w_eq_aux_p (⊖ A)   (PNegP p)    e := f_equal PNegP (p_of_w_eq_aux_n A p e) ;
 
-     with p_of_w_eq_aux_n {Γ : neg_ctx} (A : ty0 neg) (p : pat (t- A)) (e : p_dom p =[val]> Γ)
-         : p_of_w_0n A (w_subst e (t- A) (w_of_p p) : whn Γ (t- A)) = p
+with p_of_w_eq_aux_n {Γ : neg_ctx} (A : ty0 neg) (p : pat `-A) (e : p_dom p =[val]> Γ)
+         : p_of_w_0n A (w_of_p p `ᵥ⊛ e) = p
          by struct p :=
   p_of_w_eq_aux_n (⊥)     (PBot)       e := eq_refl ;
   p_of_w_eq_aux_n (A ⅋ B) (PPar p1 p2) e := f_equal2 PPar
@@ -1304,58 +1146,59 @@ Equations p_of_w_eq_aux_p {Γ : neg_ctx} (A : ty0 pos) (p : pat (t+ A)) (e : p_d
         (eq_trans (f_equal _ (w_sub_ren _ _ _ _)) (p_of_w_eq_aux_n B p2 _)) ;
   p_of_w_eq_aux_n (A & B) (PAnd1 p)    e := f_equal PAnd1 (p_of_w_eq_aux_n A p e) ;
   p_of_w_eq_aux_n (A & B) (PAnd2 p)    e := f_equal PAnd2 (p_of_w_eq_aux_n B p e) ;
-  p_of_w_eq_aux_n (↑ A)  (PShiftN _)  e := eq_refl ;
+  p_of_w_eq_aux_n (↑ A)   (PShiftN _)  e := eq_refl ;
   p_of_w_eq_aux_n (¬ A)   (PNegN p)    e := f_equal PNegN (p_of_w_eq_aux_p A p e) .
 
 Definition p_dom_of_w_eq_P (Γ : neg_ctx) p : ty0 p -> Prop :=
   match p with
-  | pos => fun A => forall (p : pat (t+ A)) (e : p_dom p =[val]> Γ),
-      rew [fun p => p_dom p =[ val ]> Γ] p_of_w_eq_aux_p A p e in p_dom_of_w_0p A (w_subst e (t+ A) (w_of_p p)) ≡ₐ e
-  | neg => fun A => forall (p : pat (t- A)) (e : p_dom p =[val]> Γ),
-      rew [fun p => p_dom p =[ val ]> Γ] p_of_w_eq_aux_n A p e in p_dom_of_w_0n A (w_subst e (t- A) (w_of_p p)) ≡ₐ e
+  | pos => fun A => forall (p : pat `+A) (e : p_dom p =[val]> Γ),
+      rew [fun p => p_dom p =[ val ]> Γ] p_of_w_eq_aux_p A p e in p_dom_of_w_0p A (w_of_p p `ᵥ⊛ e) ≡ₐ e
+  | neg => fun A => forall (p : pat `-A) (e : p_dom p =[val]> Γ),
+      rew [fun p => p_dom p =[ val ]> Γ] p_of_w_eq_aux_n A p e in p_dom_of_w_0n A (w_of_p p `ᵥ⊛ e) ≡ₐ e
   end .
 
 Lemma p_dom_of_v_eq {Γ p} A : p_dom_of_w_eq_P Γ p A .
-
-  induction A; intros p e; dependent elimination p; cbn.
+  induction A; intros p e; dependent elimination p; cbn - [ r_cat_l r_cat_r ].
   - intros ? h; repeat (dependent elimination h; auto).
   - intros ? h; repeat (dependent elimination h; auto).
-  - change (p_dom_of_w_0p _ (TenR ?v1 ?v2)) with ([ p_dom_of_w_0p A3 v1 , p_dom_of_w_0p B0 v2 ]).
-    pose (H1 := w_sub_ren e r_concat_l (t+ A3) (w_of_p p)) .
-    pose (H2 := w_sub_ren e r_concat_r (t+ B0) (w_of_p p0)) .
-    pose (x1 := w_subst e (t+ A3) (w_rename r_concat_l (t+ A3) (w_of_p p))).
-    pose (x2 := w_subst e (t+ B0) (w_rename r_concat_r (t+ B0) (w_of_p p0))).
-    change (w_sub_ren e r_concat_l _ _) with H1.
-    change (w_sub_ren e r_concat_r _ _) with H2.
-    change (w_subst e (t+ A3) _) with x1 in H1 |- *.
-    change (w_subst e (t+ B0) _) with x2 in H2 |- *.
-    rewrite H1, H2; clear H1 H2 x1 x2; cbn.
-    pose (H1 := p_of_w_eq_aux_p A3 p (e ⊛ᵣ r_concat_l)); change (p_of_w_eq_aux_p A3 _ _) with H1 in IHA1 |- *.
-    pose (H2 := p_of_w_eq_aux_p B0 p0 (e ⊛ᵣ r_concat_r)); change (p_of_w_eq_aux_p B0 _ _) with H2 in IHA2 |- *.
-    transitivity ([ rew [fun p : pat (t+ A3) => p_dom p =[ val ]> Γ] H1
-                     in p_dom_of_w_0p A3 (w_subst (e ⊛ᵣ r_concat_l) (t+ A3) (w_of_p p)) ,
-                    rew [fun p : pat (t+ B0) => p_dom p =[ val ]> Γ] H2
-                     in p_dom_of_w_0p B0 (w_subst (e ⊛ᵣ r_concat_r) (t+ B0) (w_of_p p0)) ]).
+  - pose (H1 := w_sub_ren r_cat_l e `+A3 (w_of_p p)) .
+    pose (H2 := w_sub_ren r_cat_r e `+B (w_of_p p0)) .
+    pose (x1 := w_of_p p `ᵥ⊛ᵣ r_cat_l `ᵥ⊛ e).
+    pose (x2 := w_of_p p0 `ᵥ⊛ᵣ r_cat_r `ᵥ⊛ e).
+    change (w_sub_ren r_cat_l e _ _) with H1.
+    change (w_sub_ren r_cat_r e _ _) with H2.
+    change (_ `ᵥ⊛ᵣ r_cat_l `ᵥ⊛ e) with x1 in H1 |- *.
+    change (_ `ᵥ⊛ᵣ r_cat_r `ᵥ⊛ e) with x2 in H2 |- *.
+    rewrite H1, H2; clear H1 H2 x1 x2; cbn - [ r_cat_l r_cat_r ].
+    pose (H1 := p_of_w_eq_aux_p A3 p (r_cat_l ᵣ⊛ e));
+      change (p_of_w_eq_aux_p A3 _ _) with H1 in IHA1 |- *.
+    pose (H2 := p_of_w_eq_aux_p B p0 (r_cat_r ᵣ⊛ e));
+      change (p_of_w_eq_aux_p B _ _) with H2 in IHA2 |- *.
+    transitivity ([ rew [fun p : pat `+A3 => p_dom p =[ val ]> Γ] H1
+                     in p_dom_of_w_0p A3 (w_of_p p `ᵥ⊛ r_cat_l ᵣ⊛ e) ,
+                    rew [fun p : pat `+B => p_dom p =[ val ]> Γ] H2
+                     in p_dom_of_w_0p B (w_of_p p0 `ᵥ⊛ r_cat_r ᵣ⊛ e) ])%asgn.
     now rewrite <- H1, <- H2, eq_refl_map2_distr.
-    apply s_eq_cover_uniq; [ apply IHA1 | apply IHA2 ] .
-  - change (p_dom_of_w_0n _ (ParL ?v1 ?v2)) with ([ p_dom_of_w_0n _ v1 , p_dom_of_w_0n _ v2 ]).
-    pose (H1 := w_sub_ren e r_concat_l (t- A4) (w_of_p p1)) .
-    pose (H2 := w_sub_ren e r_concat_r (t- B1) (w_of_p p2)) .
-    pose (x1 := w_subst e (t- A4) (w_rename r_concat_l (t- A4) (w_of_p p1))).
-    pose (x2 := w_subst e (t- B1) (w_rename r_concat_r (t- B1) (w_of_p p2))).
-    change (w_sub_ren e r_concat_l _ _) with H1.
-    change (w_sub_ren e r_concat_r _ _) with H2.
-    change (w_subst e (t- A4) _) with x1 in H1 |- *.
-    change (w_subst e (t- B1) _) with x2 in H2 |- *.
-    rewrite H1, H2; clear H1 H2 x1 x2; cbn.
-    pose (H1 := p_of_w_eq_aux_n A4 p1 (e ⊛ᵣ r_concat_l)); change (p_of_w_eq_aux_n A4 _ _) with H1 in IHA1 |- *.
-    pose (H2 := p_of_w_eq_aux_n B1 p2 (e ⊛ᵣ r_concat_r)); change (p_of_w_eq_aux_n B1 _ _) with H2 in IHA2 |- *.
-    transitivity ([ rew [fun p : pat (t- A4) => p_dom p =[ val ]> Γ] H1
-                     in p_dom_of_w_0n A4 (w_subst (e ⊛ᵣ r_concat_l) (t- A4) (w_of_p p1)) ,
-                    rew [fun p : pat (t- B1) => p_dom p =[ val ]> Γ] H2
-                     in p_dom_of_w_0n B1 (w_subst (e ⊛ᵣ r_concat_r) (t- B1) (w_of_p p2)) ]).
+    refine (a_cat_uniq _ _ _ _ _); [ apply IHA1 | apply IHA2 ] .
+  - pose (H1 := w_sub_ren r_cat_l e `-A4 (w_of_p p1)) .
+    pose (H2 := w_sub_ren r_cat_r e `-B0 (w_of_p p2)) .
+    pose (x1 := w_of_p p1 `ᵥ⊛ᵣ r_cat_l `ᵥ⊛ e).
+    pose (x2 := w_of_p p2 `ᵥ⊛ᵣ r_cat_r `ᵥ⊛ e).
+    change (w_sub_ren r_cat_l e _ _) with H1.
+    change (w_sub_ren r_cat_r e _ _) with H2.
+    change (_ `ᵥ⊛ᵣ r_cat_l `ᵥ⊛ e) with x1 in H1 |- *.
+    change (_ `ᵥ⊛ᵣ r_cat_r `ᵥ⊛ e) with x2 in H2 |- *.
+    rewrite H1, H2; clear H1 H2 x1 x2; cbn - [ r_cat_l r_cat_r ].
+    pose (H1 := p_of_w_eq_aux_n A4 p1 (r_cat_l ᵣ⊛ e));
+      change (p_of_w_eq_aux_n A4 _ _) with H1 in IHA1 |- *.
+    pose (H2 := p_of_w_eq_aux_n B0 p2 (r_cat_r ᵣ⊛ e));
+      change (p_of_w_eq_aux_n B0 _ _) with H2 in IHA2 |- *.
+    transitivity ([ rew [fun p : pat `-A4 => p_dom p =[ val ]> Γ] H1
+                     in p_dom_of_w_0n A4 (w_of_p p1 `ᵥ⊛ r_cat_l ᵣ⊛ e) ,
+                    rew [fun p : pat `-B0 => p_dom p =[ val ]> Γ] H2
+                     in p_dom_of_w_0n B0 (w_of_p p2 `ᵥ⊛ r_cat_r ᵣ⊛ e) ])%asgn.
     now rewrite <- H1, <- H2, eq_refl_map2_distr.
-    apply s_eq_cover_uniq; [ apply IHA1 | apply IHA2 ] .
+    refine (a_cat_uniq _ _ _ _ _); [ apply IHA1 | apply IHA2 ] .
   - match goal with | |- ?s ≡ₐ e => pose (xx := s); change (_ ≡ₐ e) with (xx ≡ₐ e) end .
     remember xx as xx'; unfold xx in Heqxx'; clear xx.
     rewrite (eq_trans Heqxx' (eq_sym (rew_map _ POr1 _ _))).
@@ -1372,8 +1215,8 @@ Lemma p_dom_of_v_eq {Γ p} A : p_dom_of_w_eq_P Γ p A .
     remember xx as xx'; unfold xx in Heqxx'; clear xx.
     rewrite (eq_trans Heqxx' (eq_sym (rew_map _ PAnd2 _ _))).
     apply IHA2.
-  - intros ? h; repeat (dependent elimination h; auto).
-  - intros ? h; repeat (dependent elimination h; auto).
+  - intros ? v; repeat (dependent elimination v; auto).
+  - intros ? v; repeat (dependent elimination v; auto).
   - match goal with | |- ?s ≡ₐ e => pose (xx := s); change (_ ≡ₐ e) with (xx ≡ₐ e) end .
     remember xx as xx'; unfold xx in Heqxx'; clear xx.
     rewrite (eq_trans Heqxx' (eq_sym (rew_map _ PNegP _ _))).
@@ -1384,831 +1227,317 @@ Lemma p_dom_of_v_eq {Γ p} A : p_dom_of_w_eq_P Γ p A .
     apply IHA.
 Qed.
 
-Lemma eval_nf_ret {Γ : neg_ctx} (u : nf Γ) : eval (p_app (s_var _ (fst (projT2 u))) (projT1 (snd (projT2 u))) (projT2 (snd (projT2 u)))) ≋ ret_delay u .
-  unfold eval, iter_delay.
-  rewrite iter_unfold.
-  unfold comp_eq. apply it_eq_unstep; cbn.
-  change (iter _ T1_0 ?x) with (iter_delay (fun c : state Γ => Ret' (eval_aux c)) x).
-  destruct u as [ A [ i [ m γ ]]]; simpl t_neg in m; cbn [ fst snd projT1 projT2 ].
-  unfold p_app.
-  funelim (w_of_p m); cbn.
-  - simpl_depind.
-    destruct A0; inversion eqargs; clear - H0.
-    revert t i m γ eqargs; rewrite <- H0; intros t i.
-    pose (nope := (s_elt_upg i).(sub_prf)); dependent elimination nope.
-  - simpl_depind.
-    destruct A; inversion eqargs; clear - H0.
-    revert t i m γ eqargs; rewrite <- H0; intros t i.
-    pose (nope := (s_elt_upg i).(sub_prf)); dependent elimination nope.
-  - simpl_depind.
-    destruct A; inversion eqargs; cbn in eqargs.
-    revert t i m γ eqargs H1 H2; rewrite <- H0; intros t i m γ eqargs H1 H2.
-    dependent elimination H1; dependent elimination H2.
-    rewrite (YesUIP _ _ _ eqargs eq_refl); clear eqargs.
-    cbn; econstructor.
-    unshelve econstructor; auto.
-    split; [ reflexivity | unshelve econstructor; auto ].
-    intros ? h; dependent elimination h.
-  - simpl_depind.
-    destruct A; inversion eqargs; cbn in eqargs.
-    revert t i m γ eqargs H1 H2; rewrite <- H0; intros t i m γ eqargs H1 H2.
-    dependent elimination H1; dependent elimination H2.
-    rewrite (YesUIP _ _ _ eqargs eq_refl); clear eqargs.
-    cbn; econstructor.
-    unshelve econstructor; auto.
-    split; [ reflexivity | unshelve econstructor; auto ].
-    intros ? h; dependent elimination h.
-  - simpl_depind.
-    destruct A; inversion eqargs; cbn in eqargs.
-    revert t i m γ eqargs H3 H4; rewrite <- H2; intros t i m γ eqargs H3 H4.
-    dependent elimination H3; dependent elimination H4.
-    rewrite (YesUIP _ _ _ eqargs eq_refl); clear eqargs.
-    cbn; econstructor.
-    unshelve econstructor; auto.
-    split; [ reflexivity | unshelve econstructor; cbn ].
-    apply (p_of_w_eq_aux_p _ (PTen p1 p2)).
-    apply (p_dom_of_v_eq (_ ⊗ _) (PTen p1 p2)).
-  - simpl_depind.
-    destruct A; inversion eqargs; cbn in eqargs.
-    revert t i m γ eqargs H3 H4; rewrite <- H2; intros t i m γ eqargs H3 H4.
-    dependent elimination H3; dependent elimination H4.
-    rewrite (YesUIP _ _ _ eqargs eq_refl); clear eqargs.
-    cbn; econstructor.
-    unshelve econstructor; auto.
-    split; [ reflexivity | unshelve econstructor; cbn ].
-    apply (p_of_w_eq_aux_n _ (PPar p1 p2)).
-    apply (p_dom_of_v_eq (_ ⅋ _) (PPar p1 p2)).
-  - simpl_depind.
-    destruct A; inversion eqargs; cbn in eqargs.
-    revert t i m γ eqargs H2 H3; rewrite <- H1; intros t i m γ eqargs H2 H3.
-    dependent elimination H2; dependent elimination H3.
-    rewrite (YesUIP _ _ _ eqargs eq_refl); clear eqargs.
-    cbn; econstructor.
-    unshelve econstructor; auto.
-    split; [ reflexivity | unshelve econstructor; cbn ].
-    apply (p_of_w_eq_aux_p _ (POr1 p)).
-    apply (p_dom_of_v_eq (_ ⊕ _) (POr1 p)).
-  - simpl_depind.
-    destruct A; inversion eqargs; cbn in eqargs.
-    revert t i m γ eqargs H2 H3; rewrite <- H1; intros t i m γ eqargs H2 H3.
-    dependent elimination H2; dependent elimination H3.
-    rewrite (YesUIP _ _ _ eqargs eq_refl); clear eqargs.
-    cbn; econstructor.
-    unshelve econstructor; auto.
-    split; [ reflexivity | unshelve econstructor; cbn ].
-    apply (p_of_w_eq_aux_p _ (POr2 p)).
-    apply (p_dom_of_v_eq (_ ⊕ _) (POr2 p)).
-  - simpl_depind.
-    destruct A; inversion eqargs; cbn in eqargs.
-    revert t i m γ eqargs H2 H3; rewrite <- H1; intros t i m γ eqargs H2 H3.
-    dependent elimination H2; dependent elimination H3.
-    rewrite (YesUIP _ _ _ eqargs eq_refl); clear eqargs.
-    cbn; econstructor.
-    unshelve econstructor; auto.
-    split; [ reflexivity | unshelve econstructor; cbn ].
-    apply (p_of_w_eq_aux_n _ (PAnd1 p)).
-    apply (p_dom_of_v_eq (_ & _) (PAnd1 p)).
-  - simpl_depind.
-    destruct A; inversion eqargs; cbn in eqargs.
-    revert t i m γ eqargs H2 H3; rewrite <- H1; intros t i m γ eqargs H2 H3.
-    dependent elimination H2; dependent elimination H3.
-    rewrite (YesUIP _ _ _ eqargs eq_refl); clear eqargs.
-    cbn; econstructor.
-    unshelve econstructor; auto.
-    split; [ reflexivity | unshelve econstructor; cbn ].
-    apply (p_of_w_eq_aux_n _ (PAnd2 p)).
-    apply (p_dom_of_v_eq (_ & _) (PAnd2 p)).
-  - simpl_depind.
-    destruct A; inversion eqargs; cbn in eqargs.
-    revert t i m γ eqargs H1 H2; rewrite <- H0; intros t i m γ eqargs H1 H2.
-    dependent elimination H1; dependent elimination H2.
-    rewrite (YesUIP _ _ _ eqargs eq_refl); clear eqargs.
-    cbn; econstructor.
-    unshelve econstructor; auto.
-    split; [ reflexivity | unshelve econstructor; auto ].
-    apply (p_dom_of_v_eq (↓ _) (PShiftP _)).
-  - simpl_depind.
-    destruct A; inversion eqargs; cbn in eqargs.
-    revert t i m γ eqargs H1 H2; rewrite <- H0; intros t i m γ eqargs H1 H2.
-    dependent elimination H1; dependent elimination H2.
-    rewrite (YesUIP _ _ _ eqargs eq_refl); clear eqargs.
-    cbn; econstructor.
-    unshelve econstructor; auto.
-    split; [ reflexivity | unshelve econstructor; auto ].
-    apply (p_dom_of_v_eq (↑ _) (PShiftN _)).
-  - simpl_depind.
-    destruct A; inversion eqargs; cbn in eqargs.
-    revert t i m γ eqargs H2 H3; rewrite <- H1; intros t i m γ eqargs H2 H3.
-    dependent elimination H2; dependent elimination H3.
-    rewrite (YesUIP _ _ _ eqargs eq_refl); clear eqargs.
-    cbn; econstructor.
-    unshelve econstructor; auto.
-    split; [ reflexivity | unshelve econstructor; cbn ].
-    apply (p_of_w_eq_aux_p _ (PNegP p)).
-    apply (p_dom_of_v_eq (⊖ _) (PNegP p)).
-  - simpl_depind.
-    destruct A; inversion eqargs; cbn in eqargs.
-    revert t i m γ eqargs H2 H3; rewrite <- H1; intros t i m γ eqargs H2 H3.
-    dependent elimination H2; dependent elimination H3.
-    rewrite (YesUIP _ _ _ eqargs eq_refl); clear eqargs.
-    cbn; econstructor.
-    unshelve econstructor; auto.
-    split; [ reflexivity | unshelve econstructor; cbn ].
-    apply (p_of_w_eq_aux_n _ (PNegN p)).
-    apply (p_dom_of_v_eq (¬ _) (PNegN p)).
+(* coq unification drives me crazy!! *)
+Definition upg_vp {Γ} {A : ty0 pos} : whn Γ `+A  -> val Γ `+A := fun v => v.
+Definition upg_kp {Γ} {A : ty0 pos} : term Γ `-A -> val Γ `-A := fun v => v.
+Definition upg_vn {Γ} {A : ty0 neg} : term Γ `+A -> val Γ `+A := fun v => v.
+Definition upg_kn {Γ} {A : ty0 neg} : whn Γ `-A  -> val Γ `-A := fun v => v.
+Definition dwn_vp {Γ} {A : ty0 pos} : val Γ `+A -> whn Γ `+A  := fun v => v.
+Definition dwn_kp {Γ} {A : ty0 pos} : val Γ `-A -> term Γ `-A := fun v => v.
+Definition dwn_vn {Γ} {A : ty0 neg} : val Γ `+A -> term Γ `+A := fun v => v.
+Definition dwn_kn {Γ} {A : ty0 neg} : val Γ `-A -> whn Γ `-A  := fun v => v.
+
+Lemma nf_eq_split_p {Γ : neg_ctx} {A : ty0 pos} (i : Γ ∋ `-A) p γ
+  : nf_eq (i ⋅ v_split_p (dwn_vp (w_of_p p `ᵥ⊛ γ)))
+          (i ⋅ (p : o_op obs_op `-A) ⦇ γ ⦈).
+  unfold v_split_p, dwn_vp; cbn.
+  pose proof (p_dom_of_v_eq A p γ).
+  pose (H' := p_of_w_eq_aux_p A p γ); fold H' in H.
+  pose (a := p_dom_of_w_0p A (w_of_p p `ᵥ⊛ γ)); fold a in H |- *.
+  remember a as a'; clear a Heqa'.
+  revert a' H; rewrite H'; intros; now econstructor.
 Qed.
-
-Lemma foo {I : Type} {E : event I I} {X : psh I} {LX LY : relᵢ X X}
-  : Subrelationᵢ LX LY -> Subrelationᵢ (it_eq (E:=E) LX) (it_eq (E:=E) LY) .
-  intros H1 i a b H2.
-  unfold it_eq; revert i a b H2; coinduction L CIH; intros i a b H2.
-  apply it_eq_step in H2; cbn in *.
-  remember (observe a) as oa; clear Heqoa a.
-  remember (observe b) as ob; clear Heqob b.
-  dependent elimination H2.
-  - econstructor; now apply H1.
-  - econstructor; now apply CIH.
-  - econstructor; intro; now apply CIH.
+Lemma nf_eq_split_n {Γ : neg_ctx} {A : ty0 neg} (i : Γ ∋ `+A) p γ
+  : nf_eq (i ⋅ v_split_n (dwn_kn (w_of_p p `ᵥ⊛ γ)))
+          (i ⋅ (p : o_op obs_op `+A) ⦇ γ ⦈).
+  unfold v_split_n, dwn_kn; cbn.
+  pose proof (p_dom_of_v_eq A p γ).
+  pose (H' := p_of_w_eq_aux_n A p γ); fold H' in H.
+  pose (a := p_dom_of_w_0n A (w_of_p p `ᵥ⊛ γ)); fold a in H |- *.
+  remember a as a'; clear a Heqa'.
+  revert a' H; rewrite H'; intros; now econstructor.
 Qed.
+(*|
+Finally we can return to saner pursuits.
 
-Lemma clean_hyp_ren {Γ Δ : neg_ctx} (c : state Γ) (e : Γ ⊆ Δ)
-   : eval (s_rename e c) ≋ fmap_delay (n_rename e) (eval c) .
-  rewrite <- (s_sub_id_l c) at 1.
-  rewrite s_ren_sub.
-  unfold comp_eq.
-  etransitivity.
-  eapply (foo (LX := eqᵢ _)).
-  intros ? ? ? ->; now apply nf_eq_rfl.
-  exact (clean_hyp c (a_ren e s_var)).
-  remember (eval c) as t; clear Heqt c.
-  unfold then_eval1.
-  unfold fmap_delay, bind_delay'.
-  rewrite bind_ret.
-  apply (proj1 (t_gfp (it_eq_map ∅ₑ (fun _ : T1 => nf_eq)) _ _ _)).
-  eapply (it_eq_up2bind_t (eqᵢ _)); econstructor; auto.
-  intros [] u v ->.
-  destruct v as [ x [ i [ m e' ] ] ]; cbn in *.
-  unfold n_rename; cbn.
-  unfold a_ren at 1; rewrite v_ren_id_r.
-  rewrite (eval_nf_ret (x ,' (e x i , (m ,' a_comp (a_ren e s_var) e')))).
-  change (gfp _ _ ?a ?b) with (it_eq (fun _ : T1 => nf_eq) a b).
-  apply it_eq_unstep.
-  econstructor.
-  unshelve econstructor; auto; cbn.
-  unshelve econstructor; auto; cbn.
-  unshelve econstructor; auto; cbn.
-  clear; intros ? i.
-  unfold a_comp, a_ren; cbn.
-  erewrite (v_sub_eq _ (s_var ⊛ᵣ e)); auto.
-  now rewrite <- v_sub_ren, v_sub_id_l.
-  intros ? j; now rewrite v_ren_id_r.
-Qed.
+OGS Instanciation
+=================
 
-Variant head_inst_nostep (u : sigT (fun A => pat (t_neg A))) : sigT (fun A => pat (t_neg A)) -> Prop :=
-| HeadInst {Γ : neg_ctx} {A} (v : val Γ A) (m : pat (t_neg A)) (e : p_dom m =[val]> Γ)
-      (p : is_var v -> False) (i : Γ ∋ (projT1 u : ty))
-      (H : fmap_delay (pat_of_nf Γ) (eval (p_app v m e)) ≊ ret_delay ((projT1 u : ty) ,' (i , projT2 u)))
-      : head_inst_nostep u (A ,' m) .
+The notion of values and configurations we will pass to the generic OGS construction
+are our mu-mu-tilde values and states, but restricted to negative typing contexts. As
+such, while we have proven all the metatheory for arbitrary typing contexts, we still
+need a tiny bit of work to provide the laws in this special case. Once again, thanks to
+our tricky notion of subset context (`Ctx/Subset.v`), there is no need to cross a
+complex isomorphism (between contexts of negative types and contexts of types where
+all types are negative). We start by instanciating the substitution structures and
+their laws.
+|*)
+Notation val_n := (val ∘ neg_c_coe).
+Notation state_n := (state ∘ neg_c_coe).
 
-Lemma eval_app_not_var : well_founded head_inst_nostep .
-  intros A; econstructor; intros [ B m ] H; dependent elimination H; cbn in *.
-  destruct A0 as [ [] | [] ].
-  1,3: cycle 1.
-  all: dependent elimination v; try now destruct (p (_ ,' eq_refl)).
-  all: clear p.
-  all: dependent elimination m0; cbn in H.
-  all: match goal with
-       | u : assignment _ (neg_c_coe (p_dom (PVarN _))) _ |- _ =>
-           cbn in H;
-           pose (vv := e _ Ctx.top); change (e _ Ctx.top) with vv in H;
-           remember vv as v'; clear e vv Heqv'; cbn in v'
-       | _ => idtac
-       end.
-  all: match goal with
-       | u : assignment _ (neg_c_coe (p_dom (PVarP _))) _ |- _ =>
-           cbn in H;
-           pose (vv := e _ Ctx.top); change (e _ Ctx.top) with vv in H;
-           remember vv as v'; clear e vv Heqv'; cbn in v'
-       | _ => idtac
-       end.
-  1-12,25-36: apply it_eq_step in H; now inversion H.
-  1-12: match goal with
-       | t : term _ (t- _) |- _ =>
-           dependent elimination t;
-           [ apply it_eq_step in H; now inversion H | apply it_eq_step in H; now inversion H | ]
-       | _ => idtac
-       end.
-  13-24: match goal with
-       | t : term _ (t+ _) |- _ =>
-           dependent elimination t;
-           [ apply it_eq_step in H; now inversion H | apply it_eq_step in H; now inversion H | ]
-       | _ => idtac
-       end.
-  1-12: match goal with
-       | w : whn _ (t- _) |- _ =>
-           dependent elimination w;
-           [ | apply it_eq_step in H; now inversion H ];
-           try now destruct (p (_ ,' eq_refl))
-       | _ => idtac
-       end.
-  13-24: match goal with
-       | w : whn _ (t+ _) |- _ =>
-           dependent elimination w;
-           [ | apply it_eq_step in H; now inversion H ];
-           try now destruct (p (_ ,' eq_refl))
-       | _ => idtac
-       end.
-   all: apply it_eq_step in H; cbn in H; simp eval_aux in H; dependent elimination H.
-   all: cbn in r_rel; inversion_sigma r_rel as [ H1 H2 ].
-   all: revert m i H2; rewrite <- H1; intros m i H2; inversion_clear H2; cbn; clear.
-   all: econstructor; intros [ A ee ] H; dependent elimination H; cbn in *.
-   all: dependent elimination v; [ apply it_eq_step in H; now inversion H | apply it_eq_step in H; now inversion H | ].
-  1-12: match goal with
-       | w : whn _ (t- _) |- _ =>
-           dependent elimination w;
-           [ | apply it_eq_step in H; now inversion H ];
-           try now destruct (p (_ ,' eq_refl))
-       | _ => idtac
-       end.
-  now destruct (p1 (_ ,' eq_refl)).
-  1-12: match goal with
-       | w : whn _ (t+ _) |- _ =>
-           dependent elimination w;
-           [ | apply it_eq_step in H; now inversion H ];
-           try now destruct (p (_ ,' eq_refl))
-       | _ => idtac
-       end.
-Qed.
-
-#[local] Instance sysD_typ  : baseT := {| typ := neg_ty |}.
-
-#[local] Instance sysD_spec : observation_structure :=
-  {| obs A := pat (t_neg (neg_coe A)) ;
-     dom _ p := ctx_s_to (p_dom p) |} .
-
-Definition state' (Γ : ctx neg_ty) : Type := state (ctx_s_from Γ).
-Definition val' (Γ : ctx neg_ty) (a : neg_ty) : Type := val (ctx_s_from Γ) a.(sub_elt).
-
-Definition from_has_F {Γ : neg_ctx} {t} (i : ctx_s_to Γ ∋ t) : Γ ∋ t.(sub_elt) :=
-  match view_s_has_map _ _ i in (s_has_map_view _ _ y h) return (Γ ∋ sub_elt y) with
-  | SHasMapV j => j
-  end .
-
-Definition to_has_F {Γ : neg_ctx} {t} (i : Γ ∋ t) : ctx_s_to Γ ∋ s_elt_upg i :=
-  s_map_has _ _ i .
-
-Lemma to_from_has_F {Γ : neg_ctx} {t} (i : ctx_s_to Γ ∋ t) : to_has_F (from_has_F i) = i .
-  unfold to_has_F, from_has_F.
-  pose (xx := view_s_has_map (fun x : sigS is_neg => x) Γ i).
-  change (view_s_has_map (fun x : sigS is_neg => x) Γ i) with xx.
-  now destruct xx.
-Qed.
-
-Lemma from_to_has_F {Γ : neg_ctx} {t} (i : Γ ∋ t) : from_has_F (to_has_F i) = i .
-  unfold from_has_F, to_has_F.
-  pose proof (s_has_map_view_simpl (f := fun x : neg_ty => x) (i := i)).
-  pose (xx := view_s_has_map (fun x : neg_ty => x) Γ (s_map_has (fun x : neg_ty => x) Γ i)).
-  change (view_s_has_map _ _ _) with xx in H |- *.
-  now rewrite H.
-Qed.
-
-Definition from_has_L {Γ : ctx neg_ty} {t} (i : Γ ∋ t) : ctx_s_from Γ ∋ t.(sub_elt) .
-  unfold ctx_s_from; destruct (ctx_s_to_inv Γ).
-  exact (from_has_F i).
+#[global] Instance val_n_monoid : subst_monoid val_n .
+  esplit.
+  - intros Γ x i; exact (var i).
+  - intros Γ x v Δ f; exact (v ᵥ⊛ f).
 Defined.
 
-Definition to_has_L {Γ : ctx neg_ty} {t} (i : ctx_s_from Γ ∋ t) : Γ ∋ s_elt_upg i .
-  unfold s_elt_upg; unfold ctx_s_from in *; destruct (ctx_s_to_inv Γ).
-  exact (to_has_F i).
+#[global] Instance state_n_module : subst_module val_n state_n .
+  esplit; intros Γ s Δ f; exact (s ₜ⊛ (f : Γ =[val]> Δ)).
 Defined.
 
-Lemma from_to_has_L {Γ : ctx neg_ty} {t} (i : ctx_s_from Γ ∋ t) : from_has_L (to_has_L i) = i .
-  unfold from_has_L, to_has_L, s_elt_upg; unfold ctx_s_from in *.
-  destruct (ctx_s_to_inv Γ).
-  unfold from_has_F.
-  pose proof (s_has_map_view_simpl (f := fun x : neg_ty => x) (i := i)).
-  pose (xx := view_s_has_map (fun x : neg_ty => x) a (s_map_has (fun x : neg_ty => x) a i)).
-  change (view_s_has_map _ _ _) with xx in H |- *.
-  now rewrite H.
+#[global] Instance val_n_laws : subst_monoid_laws val_n .
+  esplit.
+  - intros ???? <- ????; now apply v_sub_eq.
+  - intros ?????; now apply v_sub_id_r.
+  - intros ???; now apply v_sub_id_l.
+  - intros ???????; symmetry; now apply v_sub_sub.
 Qed.
 
-Lemma to_from_has_L {Γ : ctx neg_ty} {t} (i : Γ ∋ t) : to_has_L (from_has_L i) = i .
-  unfold to_has_L, from_has_L; unfold ctx_s_from.
-  destruct (ctx_s_to_inv Γ).
-  apply to_from_has_F.
+#[global] Instance state_n_laws : subst_module_laws val_n state_n .
+  esplit.
+  - intros ??? <- ????; now apply s_sub_eq.
+  - intros ??; now apply s_sub_id_l.
+  - intros ??????; symmetry; now apply s_sub_sub.
 Qed.
-
-Definition r_from_to_l {Γ : neg_ctx} : ctx_s_from (ctx_s_to Γ) ⊆ Γ :=
-  fun _ i => from_has_F (to_has_L i) .
-
-Definition r_from_to_r {Γ : neg_ctx} : Γ ⊆ ctx_s_from (ctx_s_to Γ) :=
-  fun _ i => from_has_L (to_has_F i) .
-
-Lemma r_from_to_lr {Γ : neg_ctx} : r_from_to_l ⊛ᵣ r_from_to_r ≡ₐ @r_id _ Γ .
-  intros ? i.
-  refine (rew <- [fun x : ctx_s_to Γ ∋ s_elt_upg _ => from_has_F x = i ] to_from_has_L (to_has_F i) in _).
-  exact (from_to_has_F i).
+(*|
+Variable assumptions, that is, lemmata related to decidability of a value being a variable
+are easily proven inline.
+|*)
+#[global] Instance var_laws : var_assumptions val_n.
+  esplit.
+  - intros ? [[]|[]] ?? H; now dependent destruction H.
+  - intros ? [[]|[]] v; dependent elimination v.
+    10,13: dependent elimination w.
+    all: try exact (Yes _ (Vvar _)).
+    all: apply No; intro H; dependent destruction H.
+  - intros ?? [[]|[]] ???; cbn in v; dependent induction v.
+    all: try now dependent destruction X; exact (Vvar _).
+    all: dependent induction w; dependent destruction X; exact (Vvar _).
 Qed.
+(*|
+And we conclude the easy part by instanciating the relevant part of the language
+machine.
+|*)
+#[global] Instance sysd_machine : machine val_n state_n obs_op :=
+  {| Machine.eval := @eval ; oapp := @p_app |} .
+(*|
+It now suffices to prove the remaining assumptions on the language machine: that
+evaluation respects substitution and that the 'bad-instanciation' relation has finite
+chains. For this we pull in some tooling for coinductive reasoning.
+|*)
+From Coinduction Require Import coinduction lattice rel tactics.
 
-Lemma r_from_to_rl {Γ : neg_ctx} : r_from_to_r ⊛ᵣ r_from_to_l ≡ₐ @r_id _ (ctx_s_from (ctx_s_to Γ)) .
-  intros ? i.
-  refine (rew <- [fun x : ctx_s_to Γ ∋ s_elt_upg _ => from_has_L x = i ] to_from_has_F (to_has_L i) in _).
-  exact (from_to_has_L i).
+Ltac refold_eval :=
+  change (Structure.iter _ _ ?a) with (eval a);
+  change (Structure.subst (fun pat : T1 => let 'T1_0 := pat in ?f) T1_0 ?u)
+    with (bind_delay' u f).
+(*|
+Let's go.
+|*)
+#[global] Instance machine_law : machine_laws val_n state_n obs_op.
+(*|
+First we have easy lemmata on observation application.
+|*)
+  esplit.
+  - intros; apply p_app_eq.
+  - intros ?? [[]|[]] ????; cbn.
+    1,4: change (?a `ₜ⊛ ?b) with (a ᵥ⊛ b); now rewrite (w_sub_sub _ _ _ _).
+    all: change (?a `ᵥ⊛ ?b) with (a ᵥ⊛ b) at 1; now rewrite (w_sub_sub _ _ _ _).
+(*|
+Next we prove the core argument of OGS soundness: evaluating a substitution is like
+evaluating the configuration, substituting the result and evaluating again.
+While tedious the proof is basically direct, going by induction on the structure of
+one-step evaluation.
+|*)
+  - cbn; intros Γ Δ; unfold comp_eq, it_eq; coinduction R CIH; intros c a.
+    cbn; funelim (eval_aux c); try now destruct (s_prf i).
+    + cbn; econstructor; refold_eval.
+      change (?t `ₜ⊛ ?a) with (upg_kp t ᵥ⊛ a); rewrite s_sub1_sub.
+      apply CIH.
+    + cbn; econstructor; refold_eval.
+      change (?t `ᵥ⊛ ?a) with (upg_vp t ᵥ⊛ a); rewrite s_sub1_sub.
+      apply CIH.
+    + cbn; econstructor; refold_eval.
+      change (RecL (?t `ₜ⊛ a_shift1 ?a)) with (upg_kp (RecL t) ᵥ⊛ a); rewrite t_sub1_sub.
+      apply CIH.
+    + change (it_eqF _ ?RX ?RY _ _ _) with
+        (it_eq_map ∅ₑ RX RY T1_0
+           (eval (Cut _ (Whn (v `ᵥ⊛ a)) (a `- A i)))
+           (eval (Cut _
+              (Whn ((w_of_p (p_of_w_0p A v) `ᵥ⊛ nf_args (s_var_upg i ⋅ v_split_p v)) `ᵥ⊛ a))
+              (var (s_var_upg i) `ₜ⊛ a)))).
+      unfold nf_args, v_split_p, cut_r, fill_args.
+      now rewrite (refold_id_aux A v).
+    + cbn; econstructor; refold_eval; apply CIH.
+    + cbn; econstructor; refold_eval.
+      change (?v `ᵥ⊛ ?a) with (upg_vp v ᵥ⊛ a); rewrite s_sub2_sub.
+      apply CIH.
+    + cbn; econstructor; refold_eval.
+      change (?v `ᵥ⊛ ?a) with (upg_vp v ᵥ⊛ a); rewrite s_sub1_sub.
+      apply CIH.
+    + cbn; econstructor; refold_eval.
+      change (?v `ᵥ⊛ ?a) with (upg_vp v ᵥ⊛ a); rewrite s_sub1_sub.
+      apply CIH.
+    + cbn; econstructor; refold_eval.
+      change (?v `ₜ⊛ ?a) with (upg_vn v ᵥ⊛ a); rewrite s_sub1_sub.
+      apply CIH.
+    + cbn; econstructor; refold_eval.
+      change (?v `ᵥ⊛ ?a) with (upg_kn v ᵥ⊛ a); rewrite s_sub1_sub.
+      apply CIH.
+    + cbn; econstructor; refold_eval.
+      change (?v `ₜ⊛ ?a) with (upg_vn v ᵥ⊛ a); rewrite s_sub1_sub.
+      apply CIH.
+    + cbn; econstructor; refold_eval.
+      change (?v `ᵥ⊛ ?a) with (upg_kn v ᵥ⊛ a); rewrite s_sub1_sub.
+      apply CIH.
+    + cbn; econstructor; refold_eval.
+      change (RecR (?t `ₜ⊛ a_shift1 ?a)) with (upg_vn (RecR t) ᵥ⊛ a); rewrite t_sub1_sub.
+      apply CIH.
+    + change (it_eqF _ ?RX ?RY _ _ _) with
+        (it_eq_map ∅ₑ RX RY T1_0
+           (eval (Cut _ (a `+ A i) (Whn (k `ᵥ⊛ a))))
+           (eval (Cut _
+              (var (s_var_upg i) `ₜ⊛ a)
+              (Whn ((w_of_p (p_of_w_0n A k) `ᵥ⊛ nf_args (s_var_upg i ⋅ v_split_n k))
+                      `ᵥ⊛ a))))).
+      unfold nf_args, v_split_n, cut_r, fill_args.
+      now rewrite (refold_id_aux A k).
+    + cbn; econstructor; refold_eval; apply CIH.
+    + cbn; econstructor; refold_eval.
+      change (?v `ᵥ⊛ ?a) with (upg_kn v ᵥ⊛ a); rewrite s_sub2_sub.
+      apply CIH.
+    + cbn; econstructor; refold_eval.
+      change (?v `ᵥ⊛ ?a) with (upg_kn v ᵥ⊛ a); rewrite s_sub1_sub.
+      apply CIH.
+    + cbn; econstructor; refold_eval.
+      change (?v `ᵥ⊛ ?a) with (upg_kn v ᵥ⊛ a); rewrite s_sub1_sub.
+      apply CIH.
+    + cbn; econstructor; refold_eval.
+      change (?v `ₜ⊛ ?a) with (upg_kp v ᵥ⊛ a); rewrite s_sub1_sub.
+      apply CIH.
+    + cbn; econstructor; refold_eval.
+      change (?v `ᵥ⊛ ?a) with (upg_vp v ᵥ⊛ a); rewrite s_sub1_sub.
+      apply CIH.
+(*|
+Next we prove that evaluating a normal form is just returning this normal form. This
+goes by approximately induction on observations. 
+|*)
+  - cbn; intros ? [ A i [ o γ ]]; cbn; unfold p_app, nf_args, cut_r, fill_args.
+    cbn in o; funelim (w_of_p o); simpl_depind; inversion eqargs.
+    all: match goal with
+         | H : _ = ?A† |- _ => destruct A; dependent destruction H
+         end.
+    1-2: unfold c_var in i; destruct (s_prf i).
+    all: dependent destruction eqargs; cbn.
+    all: apply it_eq_unstep; cbn -[w_of_p]; econstructor.
+    1-2: now econstructor.
+    all: match goal with
+         | γ : dom ?p =[val_n]> _ |- _ => first [ exact (nf_eq_split_p _ p γ)
+                                              | exact (nf_eq_split_n _ p γ) ]
+         end.
+(*|
+Finally we prove the finite chain property. The proof here is quite tedious again, with
+numerous cases, but it is still by brutally walking through the structure of one-step
+evaluation and finding the needed redex.
+|*)
+  - intros A; econstructor; intros [ B m ] H; dependent elimination H;
+      cbn [projT1 projT2] in i, i0.
+    destruct y as [ [] | [] ].
+    all: dependent elimination v; try now destruct (t0 (Vvar _)).
+    all: clear t0.
+    all: dependent elimination o; cbn in i0.
+    all: match goal with
+         | u : dom _ =[val_n]> _ |- _ =>
+             cbn in i0;
+             pose (vv := u _ Ctx.top); change (u _ Ctx.top) with vv in i0;
+             remember vv as v'; clear u vv Heqv'; cbn in v'
+         | _ => idtac
+       end.
+    7-18,25-36: apply it_eq_step in i0; now inversion i0.
+    1-9,19-24: match goal with
+       | t : term _ _ |- _ =>
+           dependent elimination t;
+           [ apply it_eq_step in i0; now inversion i0
+           | apply it_eq_step in i0; now inversion i0
+           | ]
+       | _ => idtac
+         end.
+    all: 
+      match goal with
+      | t : evalₒ (Cut _ (Whn ?w) _) ≊ _ |- _ =>
+          dependent elimination w;
+          [ | apply it_eq_step in i0; now inversion i0 ]
+      | t : evalₒ (Cut _ _ (Whn ?w)) ≊ _ |- _ =>
+          dependent elimination w;
+          [ | apply it_eq_step in i0; now inversion i0 ]
+      | _ => idtac
+      end.
+    all:
+      apply it_eq_step in i0; cbn in i0; dependent elimination i0; cbn in r_rel;
+      apply noConfusion_inv in r_rel; unfold v_split_n,v_split_p in r_rel;
+      cbn in r_rel; unfold NoConfusionHom_f_cut,s_var_upg in r_rel; cbn in r_rel;
+      pose proof (H := f_equal pr1 r_rel); cbn in H; dependent destruction H;
+      apply DepElim.pr2_uip in r_rel;
+      pose proof (H := f_equal pr1 r_rel); cbn in H; dependent destruction H;
+      apply DepElim.pr2_uip in r_rel; dependent destruction r_rel.
+    all:
+      econstructor; intros [ t o ] H; cbn in t,o; dependent elimination H;
+      dependent elimination v;
+      [ apply it_eq_step in i0; cbn in i0; now inversion i0
+      | apply it_eq_step in i0; cbn in i0; now inversion i0 
+      | ].
+    all:
+      match goal with
+      | H : is_var (Whn ?w) -> _ |- _ =>
+          dependent elimination w;
+          try now destruct (H (Vvar _))
+      end.
+    all: apply it_eq_step in i0; cbn in i0; dependent elimination i0.
 Qed.
+(*|
+Final theorem
+=============
 
-Definition r_to_from_l {Γ : ctx neg_ty} : ctx_s_to (ctx_s_from Γ) ⊆ Γ :=
-  fun _ i => to_has_L (from_has_F i) .
-
-Definition r_to_from_r {Γ : ctx neg_ty} : Γ ⊆ ctx_s_to (ctx_s_from Γ) :=
-  fun _ i => to_has_F (from_has_L i) .
-
-Lemma r_to_from_lr {Γ : ctx neg_ty} : r_to_from_l ⊛ᵣ r_to_from_r ≡ₐ @r_id _ Γ .
-  intros ? i.
-  refine (rew <- [fun x : ctx_s_from Γ ∋ a.(sub_elt) => to_has_L x = i ] from_to_has_F (from_has_L i) in _).
-  exact (to_from_has_L i).
-Qed.
-
-Lemma r_to_from_rl {Γ : ctx neg_ty} : r_to_from_r ⊛ᵣ r_to_from_l ≡ₐ @r_id _ (ctx_s_to (ctx_s_from Γ)) .
-  intros ? i.
-  refine (rew <- [fun x : ctx_s_from Γ ∋ a.(sub_elt) => to_has_F x = i ] from_to_has_L (from_has_F i) in _).
-  exact (to_from_has_F i).
-Qed.
-
-Definition to_FB {Γ1 : neg_ctx} {Γ2} (u : Γ1 =[val]> ctx_s_from Γ2) : ctx_s_to Γ1 =[val']> Γ2 :=
-  fun _ i => u _ (from_has_F i) .
-
-#[global] Instance to_FB_proper {Γ1 Γ2} : Proper (ass_eq _ _ ==> ass_eq _ _) (@to_FB Γ1 Γ2).
-  intros u1 u2 H ? i; apply (H _ (from_has_F i)).
-Qed.
-
-Definition from_FB {Γ1 : neg_ctx} {Γ2} (u : ctx_s_to Γ1 =[val']> Γ2) : Γ1 =[val]> ctx_s_from Γ2 :=
-  fun _ i => u _ (to_has_F i) .
-
-#[global] Instance from_FB_proper {Γ1 Γ2} : Proper (ass_eq _ _ ==> ass_eq _ _) (@from_FB Γ1 Γ2).
-  intros u1 u2 H ? i; unfold from_FB.
-  exact (H _ (s_map_has _ _ i)).
-Qed.
-
-Lemma to_from_FB {Γ1 : neg_ctx} {Γ2} (u : ctx_s_to Γ1 =[val']> Γ2) : to_FB (from_FB u) ≡ₐ u .
-  intros ? i; unfold to_FB, from_FB.
-  f_equal; apply to_from_has_F.
-Qed.
-
-Lemma from_to_FB {Γ1 : neg_ctx} {Γ2} (u : Γ1 =[val]> ctx_s_from Γ2) : from_FB (to_FB u) ≡ₐ u.
-  intros ? i; unfold to_FB, from_FB.
-  now rewrite from_to_has_F.
-Qed.
-
-Definition to_FF {Γ1 Γ2 : neg_ctx} (u : Γ1 =[val]> Γ2) : ctx_s_to Γ1 =[val']> ctx_s_to Γ2 :=
-  to_FB (a_ren r_from_to_r u).
-
-#[global] Instance to_FF_proper {Γ1 Γ2} : Proper (ass_eq _ _ ==> ass_eq _ _) (@to_FF Γ1 Γ2).
-  intros u1 u2 H ? i; unfold to_FF.
-  apply to_FB_proper.
-  now rewrite H.
-Qed.
-
-Definition from_FF {Γ1 Γ2 : neg_ctx} (u : ctx_s_to Γ1 =[val']> ctx_s_to Γ2) : Γ1 =[val]> Γ2 :=
-  a_ren r_from_to_l (from_FB u) .
-
-#[global] Instance from_FF_proper {Γ1 Γ2} : Proper (ass_eq _ _ ==> ass_eq _ _) (@from_FF Γ1 Γ2).
-  intros u1 u2 H ? i; unfold from_FF.
-  apply a_ren_eq; auto.
-  now apply from_FB_proper.
-Qed.
-
-Definition to_BB {Γ1 Γ2} (u : ctx_s_from Γ1 =[val]> ctx_s_from Γ2) : Γ1 =[val']> Γ2 :=
-  fun _ i => u _ (from_has_L i) .
-
-#[global] Instance to_BB_proper {Γ1 Γ2} : Proper (ass_eq _ _ ==> ass_eq _ _) (@to_BB Γ1 Γ2).
-  intros ? ? H ? i; exact (H _ (from_has_L i)).
-Qed.
-
-Definition from_BB {Γ1 Γ2} (u : Γ1 =[val']> Γ2) : ctx_s_from Γ1 =[val]> ctx_s_from Γ2 :=
-  fun _ i => u _ (to_has_L i).
-
-#[global] Instance from_BB_proper {Γ1 Γ2} : Proper (ass_eq _ _ ==> ass_eq _ _) (@from_BB Γ1 Γ2).
-  intros u1 u2 H ? i; exact (H _ (to_has_L i)).
-Qed.
-
-Lemma to_from_BB {Γ1 Γ2} (u : Γ1 =[val']> Γ2) : to_BB (from_BB u) ≡ₐ u .
-  unfold to_BB, from_BB.
-  intros ? i; f_equal.
-  apply to_from_has_L.
-Qed.
-
-Lemma from_to_BB {Γ1 Γ2} (u : ctx_s_from Γ1 =[val]> ctx_s_from Γ2) : from_BB (to_BB u) ≡ₐ u .
-  unfold to_BB, from_BB.
-  intros ? i; f_equal.
-  apply from_to_has_L.
-Qed.
-
-Definition to_BF {Γ1 : ctx neg_ty} {Γ2 : neg_ctx} (u : ctx_s_from Γ1 =[val]> Γ2) : Γ1 =[val']> ctx_s_to Γ2 :=
-  to_FF u ⊛ᵣ r_to_from_r.
-
-#[global] Instance to_BF_proper {Γ1 Γ2} : Proper (ass_eq _ _ ==> ass_eq _ _) (@to_BF Γ1 Γ2).
-  intros u1 u2 H ? i; apply (to_FF_proper _ _ H _ _).
-Qed.
-
-Definition from_BF {Γ1 : ctx neg_ty} {Γ2 : neg_ctx} (u : Γ1 =[val']> ctx_s_to Γ2) : ctx_s_from Γ1 =[val]> Γ2 :=
-  from_FF (u ⊛ᵣ r_to_from_l) .
-
-#[global] Instance from_BF_proper {Γ1 Γ2} : Proper (ass_eq _ _ ==> ass_eq _ _) (@from_BF Γ1 Γ2).
-  intros u1 u2 H ? i; unfold from_BF.
-  apply from_FF_proper; now rewrite H.
-Qed.
-
-Lemma from_BB_to_FF {Δ Γ : neg_ctx} (e : Γ =[ val ]> Δ) : a_ren r_from_to_l (from_BB (to_FF e)) ≡ₐ e ⊛ᵣ r_from_to_l .
-  unfold from_BB, to_FF, to_FB, a_ren, s_map; cbn; intros ? i.
-  now rewrite v_ren_ren, r_from_to_lr, v_ren_id_l.
-Qed.
-
-Definition ugly_var {Γ} : Γ =[val']> Γ := fun _ i => s_var _ (from_has_L i) .
-
-Lemma from_BB_var {Γ} : from_BB (@ugly_var Γ) ≡ₐ s_var .
-  unfold from_BB, from_FB, ugly_var, ctx_s_from, s_ren, s_map, from_has_L, to_has_L, r_to_from_l, s_elt_upg.
-  intros ? i; f_equal.
-  destruct (ctx_s_to_inv Γ); cbn in *.
-  unfold from_has_F; change (s_map_has' ?a _ _ i) with (s_map_has a a0 i).
-  pose proof (s_has_map_view_simpl (f := fun x : neg_ty => x) (Γ := a0) (i := i)).
-  pose (x := view_s_has_map (fun x => x) a0 (s_map_has (fun x => x) a0 i)).
-  change (view_s_has_map _ _ _) with x in H |- *.
-  now rewrite H.
-Qed.
-
-Lemma ugly_var_inj {Γ x} (i j : Γ ∋ x) : ugly_var x i = ugly_var x j -> i = j .
-  intro H.
-  unfold ugly_var, from_has_L, from_has_F in H.
-  apply var_inj in H.
-  pose (xx := ctx_s_to_inv Γ).
-  fold xx in H.
-  dependent induction xx; clear xx0.
-  pose (xx := ctx_s_to_inv (ctx_s_to a)).
-  change (ctx_s_to_inv (ctx_s_to a)) with xx in x , H.
-  change (sigS _) with neg_ty in H.
-
-  (* >> !!!! rewrite is borked *)
-  pose proof (@eq_ind (fiber ctx_s_to (ctx_s_to a)) xx
-           (fun u =>
-  match u as f in (fiber _ b) return (b ∋ x0 -> fib_extr f ∋ sub_elt x0) with
-      | Fib a =>
-          fun i : ctx_s_to a ∋ x0 =>
-          match view_s_has_map (fun x : neg_ty => x) a i in (s_has_map_view _ _ y h) return (a ∋ sub_elt y) with
-          | SHasMapV j => j
-          end
-      end i =
-      match u as f in (fiber _ b) return (b ∋ x0 -> fib_extr f ∋ sub_elt x0) with
-      | Fib a =>
-          fun i : ctx_s_to a ∋ x0 =>
-          match view_s_has_map (fun x : neg_ty => x) a i in (s_has_map_view _ _ y h) return (a ∋ sub_elt y) with
-          | SHasMapV j => j
-          end
-      end j
-        ) H _ (eq_sym x)).
-  clear H x xx; cbn in H0.
-  (* << !!!! rewrite is borked *)
-
-  destruct (view_s_has_map (fun x : neg_ty => x) _ i).
-  rewrite H0; clear H0.
-
-  (* >> !!!! remember is borked *)
-  unfold s_elt_upg in j; revert j.
-  refine (((fun p => _) : forall (p : is_neg x) (j : @ctx_s_to ty is_neg a ∋ {| sub_elt := x; sub_prf := p |}),
-  @s_map_has ty is_neg neg_ty (fun x0 : neg_ty => x0) a x
-    match
-      @view_s_has_map ty is_neg neg_ty (fun x0 : neg_ty => x0) a
-        {| sub_elt := x; sub_prf := p |} j in (s_has_map_view _ _ y h)
-      return (a ∋ @sub_elt _ _ y)
-    with
-    | SHasMapV j0 => j0
-    end = j) (sub_prf a x i)).
-  clear i; intro j.
-  pose (xx := view_s_has_map (fun x0 : neg_ty => x0) a j); fold xx.
-  dependent induction xx; clear xx0.
-  (* >> !!!! remember is borked *)
-
-  pose (xx := view_s_has_map (fun x1 : neg_ty => x1) a (s_map_has (fun x1 : sigS is_neg => x1) a i)).
-  change (view_s_has_map _ _ _) with xx in x |- *.
-  now rewrite <- x.
-Qed.
-
-Lemma ugly_var_dec {Γ x} (v : val' Γ x) : sigT (fun i : Γ ∋ x => v = ugly_var x i)
-                                          + (sigT (fun i : Γ ∋ x => v = ugly_var x i) -> False) .
- destruct (is_var_dec v); [ apply inl | apply inr ].
- + unfold val' in v; unfold ugly_var, from_has_L; unfold ctx_s_from in *.
-   destruct i; unshelve econstructor.
-   * clear e; destruct (ctx_s_to_inv Γ).
-     exact (s_map_has _ _ x0).
-   * refine (eq_trans e _); clear e; f_equal.
-     destruct (ctx_s_to_inv Γ); cbn.
-     unfold from_has_F.
-     pose (xx := view_s_has_map (fun x1 : sigS is_neg => x1) a (s_map_has (fun x1 : sigS is_neg => x1) a x0)).
-     pose proof (s_has_map_view_simpl (f := fun x : neg_ty => x) (i := x0)).
-     change (view_s_has_map _ _ _) with xx in H |- *.
-     now rewrite H.
- + intros []; apply f.
-   exact (from_has_L x0 ,' e).
-Qed.
-
-Lemma ugly_is_var_ren {Γ1 Γ2 x} (v : val' Γ1 x) (e : Γ1 ⊆ Γ2) :
-  sigT (fun i : Γ2 ∋ x => v_subst (from_BB (ugly_var ⊛ᵣ e)) (sub_elt x) v = ugly_var x i) ->
-  sigT (fun i : Γ1 ∋ x => v = ugly_var x i) .
-  intros p; unfold val' in v.
-  destruct p as [ i H ].
-  destruct x as [ [ [] A | [] A ] p ].
-  all: try now destruct p.
-  all: dependent elimination v; try now inversion H.
-  all: dependent induction w; cbn in *; try now inversion H.
-  all: apply (substS (fun p => sigT (fun i0 : Γ1 ∋ {| sub_elt := _ ; sub_prf := p |} => Whn (Var h) = Whn (Var (from_has_L i0)))) ((ctx_s_from Γ1).(sub_prf) _ h) p).
-  all: exact (to_has_L h ,' f_equal (fun h => Whn (Var h)) (eq_sym (from_to_has_L h))).
-Qed.
-
-Lemma from_BB_comp {Γ1 Γ2 Γ3} (u : Γ2 =[ val' ]> Γ3) (v : Γ1 =[ val' ]> Γ2)
-  : a_comp (from_BB u) (from_BB v) ≡ₐ from_BB (fun _ i => v_subst (from_BB u) _ (v _ i)) .
-  reflexivity.
-Qed.
-
-Lemma ugly_comp_weird {Γ1 : neg_ctx} {Γ2 Γ3} (u : Γ2 =[ val' ]> Γ3) (v : ctx_s_to Γ1 =[ val' ]> Γ2)
-  : a_comp (from_BB u) (from_FB v)
-      ≡ₐ from_FB (fun _ i => v_subst (from_BB u) _ (v _ i)) .
-  reflexivity.
-Qed.
-
-Definition to_nf {Γ} (u : nf (ctx_s_from Γ)) :
-  sigT (fun t : neg_ty => prod (Γ ∋ t) (sigT (fun m : pat (t_neg t) => ctx_s_to (p_dom m) =[ val' ]> Γ ))) :=
-  (_ ,' (to_has_L (fst (projT2 u)) , (projT1 (snd (projT2 u)) ,' to_FB (projT2 (snd (projT2 u)))))) .
-
-#[local] Instance sysD_val  : baseV := {| Subst.val := val' |}.
-#[local] Instance sysD_conf : baseC := {| Subst.conf := state' |}.
-
-#[local] Instance sysD_val_mon : subst_monoid _ :=
-  {| v_var := @ugly_var ;
-     v_sub := fun _ _ a _ v => v_subst (from_BB a) _ v |} .
-
-#[local] Instance sysD_val_laws : subst_monoid_laws .
-  econstructor.
-  - intros Γ Δ u1 u2 H1 i v1 v2 H2.
-    apply v_sub_eq; auto.
-    now rewrite H1.
-  - intros Γ1 Γ2 u ? i; cbn.
-    etransitivity.
-    unfold ugly_var, from_has_L; apply v_sub_id_r.
-    unfold from_BB, from_has_F, r_to_from_l, s_elt_upg, ctx_s_from, to_has_L.
-    destruct (ctx_s_to_inv Γ1); cbn.
-    pose (xx := view_s_has_map (fun x : sigS is_neg => x) a0 i).
-    fold xx; now destruct xx.
-  - intros Γ1 Γ2 u ? i; cbn.
-    etransitivity.
-    apply v_sub_eq; [ apply from_BB_var | reflexivity ].
-    apply v_sub_id_l.
-  - intros Γ1 Γ2 Γ3 Γ4 p q r ? i; cbn.
-    rewrite v_sub_sub.
-    apply v_sub_eq; auto.
-Qed.
-
-#[local] Instance sysD_conf_mod : subst_module _ _ :=
-  {| c_sub := fun _ _ a s => s_subst (from_BB a) s |} .
-
-#[local] Instance sysD_conf_laws : subst_module_laws .
-  econstructor.
-  - intros Γ Δ u1 u2 H1 s1 s2 H2; cbn.
-    apply s_sub_eq; auto.
-    now rewrite H1.
-  - intros Γ c; cbn.
-    rewrite from_BB_var.
-    apply s_sub_id_l.
-  - intros Γ1 Γ2 Γ3 u v c; cbn.
-    rewrite s_sub_sub.
-    apply s_sub_eq; auto.
-Qed.
-
-#[local] Instance sysD_var_laws : var_assumptions.
-  econstructor.
-  - exact @ugly_var_inj.
-  - exact @ugly_var_dec.
-  - exact @ugly_is_var_ren.
-Qed.
-
-Lemma to_comp_eq {Γ} (u v : delay (nf (ctx_s_from Γ))) (H : u ≋ v) :
-  Obs.comp_eq (fmap_delay to_nf u) (fmap_delay to_nf v) .
-  unfold Obs.comp_eq, fmap_delay.
-  eapply (fmap_eq (RX := fun _ => nf_eq)); auto.
-  intros [] ? ?  H1.
-  destruct x as [ x1 [ i1 [ m1 γ1 ] ] ].
-  destruct y as [ x2 [ i2 [ m2 γ2 ] ] ].
-  destruct H1 as [ H1 [ H2 [ H3 H4 ] ] ].
-  cbn in *.
-  revert i1 m1 γ1 H2 H3 H4; rewrite H1; clear H1 x1; intros i1 m1 γ1 H2 H3 H4; cbn in *.
-  rewrite H2; clear H2 i1.
-  revert γ1 H4; rewrite H3; clear H3 m1; intros γ1 H4; cbn in *.
-  unshelve econstructor; auto; cbn.
-  unshelve econstructor; auto; cbn.
-  unshelve econstructor; auto; cbn.
-  now rewrite H4.
-Qed.
-
-Definition from_pat_L {Γ : ctx neg_ty} : sigT (fun x : neg_ty => prod (Γ ∋ x) (pat (t_neg x))) -> pat' (ctx_s_from Γ) :=
-  fun u => (_ ,' (from_has_L (fst (projT2 u)) , snd (projT2 u))) .
-
-Definition from_pat_F {Γ : neg_ctx} : sigT (fun x : neg_ty => prod (ctx_s_to Γ ∋ x) (pat (t_neg x))) -> pat' Γ :=
-  fun u => (_ ,' (from_has_F (fst (projT2 u)) , snd (projT2 u))) .
-
-Definition to_pat {Γ : ctx neg_ty} : pat' (ctx_s_from Γ) -> sigT (fun x : neg_ty => prod (Γ ∋ x) (pat (t_neg x))) :=
-  fun u => (_ ,' (to_has_L (fst (projT2 u)) , snd (projT2 u))) .
-
-Lemma from_to_pat_F {Γ : neg_ctx} (x y : nf (ctx_s_from (ctx_s_to Γ))) (H : x = y)
-  : from_pat_F (obs'_of_nf' _ (to_nf x)) = pat_of_nf _ (n_rename r_from_to_l y) .
-  now rewrite H.
-Qed.
-
-#[local] Instance sysD_machine : machine :=
-  {| Machine.eval := fun _ c => fmap_delay to_nf (eval c) ;
-     Machine.app := fun _ _ v m e => p_app v m (from_FB e) |} .
-
-#[local] Instance sysD_machine_law : machine_laws.
-  econstructor; unfold sysD_spec, sysD_val in *; cbn in *.
-  - intros Γ x v m u1 u2 H.
-    destruct x as [ [ [] | [] ] neg ]; cbn in *; try now destruct neg.
-    all: do 2 f_equal; apply w_sub_eq; [ now rewrite H | reflexivity ].
-  - intros Γ1 Γ2 x e v m r; cbn.
-    destruct x as [ [ [] | [] ] neg]; cbn in *; try now destruct neg.
-    all: do 2 f_equal; change (w_subst ?u ?t) with (v_subst u t); rewrite v_sub_sub.
-    all: apply v_sub_eq; auto.
-  - intros Γ Δ c e .
-    unfold Obs.comp_eq, fmap_delay.
-    etransitivity.
-    unshelve eapply fmap_eq. 5: exact (clean_hyp c (from_BB e)).
-    exact ((fun _ => to_nf)).
-    intros ? u v ->; unshelve econstructor; auto.
-    unfold bind_delay', then_eval1.
-    rewrite fmap_bind_com, bind_fmap_com.
-    apply (proj1 (t_gfp (it_eq_map ∅ₑ (fun _ : T1 => Obs.nf'_eq)) _ _ _)).
-    eapply (it_eq_up2bind_t (eqᵢ _)); econstructor; auto.
-    intros [] u v ->.
-    change (gfp _ _ ?a ?b) with (Obs.comp_eq a b).
-    apply to_comp_eq.
-    erewrite p_app_eq; auto.
-    now rewrite <- (from_to_FB (projT2 (snd (projT2 v)))).
-  - intros Γ [ x [ j [ m γ ] ] ] ; cbn in *.
-    pose proof (eval_nf_ret ((x : ty) ,' (from_has_L j , (m ,' from_FB γ)))); cbn in H.
-    apply to_comp_eq in H.
-    rewrite H; clear H.
-    unfold Obs.comp_eq; apply it_eq_unstep; cbn; econstructor.
-    unshelve econstructor; auto; cbn.
-    unshelve econstructor; auto; cbn.
-    + exact (to_from_has_L _).
-    + unshelve econstructor; auto; cbn.
-      apply to_from_FB.
-  - intros [ [ t H ] p ]; simpl in p.
-    pose (u := (t ,' p) : sigT (fun t : ty => pat (t_neg t))); simpl in u.
-    change t with (projT1 u) in H |- *.
-    change p with (projT2 u).
-    revert H.
-    remember u; clear t p u Heqs.
-    induction (eval_app_not_var s).
-    intro H1.
-    econstructor. intros y H2.
-    eassert (H3 : _). refine (H0 ((projT1 y).(sub_elt) ,' projT2 y) _ ((projT1 y).(sub_prf))).
-    * dependent elimination H2.
-      cbn in *.
-      (*unfold Spec.eval_to_msg in i0.*)
-      destruct x as [ t m ]; cbn in *.
-      unshelve econstructor.
-      + clear - Γ ; exact (ctx_s_from Γ).
-      + clear - v ; exact v.
-      + clear - e ; exact (from_FB e).
-      + exact (from_has_L i).
-      + intros []; apply p. (*; unfold Spec.is_var, Spec.v_var.*)
-        apply (substS (fun u => sigT (fun i1 : Γ ∋ {| sub_elt := t; sub_prf := u |} => v = ugly_var {| sub_elt := t; sub_prf := u |} i1)) ((ctx_s_from Γ).(sub_prf) _ x)).
-        refine (to_has_L x ,' _).
-        rewrite e0; unfold ugly_var; f_equal; symmetry.
-        apply from_to_has_L.
-      + cbn in *.
-        eapply (fmap_eq (RY := eqᵢ _) (fun _ => from_pat_L) (fun _ => from_pat_L)) in i0; [ | intros ? ? ? ->; auto ].
-        unfold eval_to_obs, Machine.eval in i0; cbn in i0; unfold fmap_delay in i0.
-        rewrite 2 fmap_fmap_com in i0.
-        transitivity (((fun (_ : T1) (x : nf (ctx_s_from Γ)) => from_pat_L (obs'_of_nf' Γ (to_nf x))) <$>
-        eval (p_app v m (from_FB e)))).
-        unfold fmap_delay.
-        eapply fmap_eq; auto.
-        ** intros [] n1 n2 H'; cbn.
-           destruct n1 as [ x1 [ i1 [ m1 γ1 ]] ].
-           destruct n2 as [ x2 [ i2 [ m2 γ2 ]] ].
-           destruct H' as [ H2 [ H3 [ H4 _ ] ] ]; cbn in *.
-           unfold Obs.obs'_of_nf', pat_of_nf, from_pat_L; cbn.
-           revert i1 m1 γ1 H3 H4; rewrite H2; clear H2 x1; intros i1 m1 γ1 H3 H4; cbn in H3,H4.
-           now rewrite H3, H4, from_to_has_L.
-        ** rewrite i0; clear.
-           apply it_eq_unstep; cbn; econstructor; reflexivity.
-    * clear - H3; cbn in H3.
-      change ({| sub_elt := sub_elt (projT1 y); sub_prf := sub_prf (projT1 y) |}) with (projT1 y) in H3.
-      assert (H4 : (projT1 y,' projT2 y) = y) ; [ | rewrite H4 in H3; exact H3 ].
-      clear; destruct y; cbn in *.
-      reflexivity.
-Qed.
-
-Definition sem_act (Δ Γ : neg_ctx) : Type := ogs_act (ctx_s_to Δ) (∅ ▶ ctx_s_to Γ) .
-Definition sem_pas (Δ Γ : neg_ctx) : Type := ogs_pas (ctx_s_to Δ) (∅ ▶ ctx_s_to Γ) .
-
-Definition ugly_state {Γ : neg_ctx} (c : state Γ) : state (ctx_s_from (ctx_s_to Γ)) :=
-  match ctx_s_to_inv (ctx_s_to Γ) as f in (fiber _ b) return (b = ctx_s_to Γ -> state (fib_extr f)) with
-  | Fib a => fun H => rew <- [state ∘ coe_ctx] ctx_s_to_inj H in c
-  end eq_refl .
-
-Definition from_to_state {Γ : neg_ctx} (c : state Γ) : state (ctx_s_from (ctx_s_to Γ)) :=
-  s_rename r_from_to_r c .
-
-Definition interp_act_s Δ {Γ : neg_ctx} (c : state Γ) : sem_act Δ Γ :=
-  m_strat (∅ ▶ ctx_s_to Γ) (inj_init_act (ctx_s_to Δ) (from_to_state c)) .
-Notation "⟦ t ⟧ₛ" := (interp_act_s _ t) .
-
-Definition ogs_weq_act Δ {Γ} : relation (sem_act Δ Γ) := fun u v => u ≈ v .
-Notation "u ≈[ Δ ]≈ v" := (ogs_weq_act Δ u v) (at level 40).
-
-Definition eval_to_msg {Γ : neg_ctx} (c : state Γ) : delay (pat' Γ) :=
-  fmap_delay (pat_of_nf Γ) (eval c) .
-
+We have finished instanciating our generic OGS construction on the System D calculus. For
+good measure we give here the concrete instanciation of the soundness theorem, stating
+that bisimilarity of the OGS strategies substitution equivalence.
+|*)
 Definition subst_eq (Δ : neg_ctx) {Γ} : relation (state Γ) :=
-  fun u v => forall (σ : Γ =[val]> Δ), eval_to_msg (s_subst σ u) ≈ eval_to_msg (s_subst σ v) .
+  fun u v => forall (σ : Γ =[val]> Δ), evalₒ (u ₜ⊛ σ : state_n Δ) ≈ evalₒ (v ₜ⊛ σ : state_n Δ) .
+Notation "x ≈⟦sub Δ ⟧≈ y" := (subst_eq Δ x y) (at level 50).
 
-Theorem sysD_subst_correct (Δ : neg_ctx) {Γ : neg_ctx} (x y : state Γ)
-  : ⟦ x ⟧ₛ ≈[ Δ ]≈ ⟦ y ⟧ₛ -> subst_eq Δ x y .
-  intros H σ.
-  apply (ogs_correction (M := sysD_machine)
-            (ctx_s_to Δ)
-            (from_to_state x)
-            (from_to_state y)) in H.
-  specialize (H (to_FF σ)).
+Theorem subst_correct (Δ : neg_ctx) {Γ : neg_ctx} (x y : state Γ)
+  : x ≈⟦ogs Δ ⟧≈ y -> x ≈⟦sub Δ ⟧≈ y.
+  exact (ogs_correction _ x y).
+Qed.
+(*|
+Finally it does not cost much to recover the more standard CIU equivalence, which we
+derive here for the case of terms (not co-terms).
+|*)
+Definition c_of_t {Γ : neg_ctx} {A : ty0 pos} (t : term Γ `+A)
+           : state_n (Γ ▶ₛ {| sub_elt := `-A ; sub_prf := stt |}) :=
+  Cut _ (t_shift1 _ t) (Whn (Var Ctx.top)) .
+Notation "'name⁺'" := c_of_t.
 
-  unfold eval_in_env, eval_to_msg, eval_to_obs in H ; cbn in H.
+Definition a_of_sk {Γ Δ : neg_ctx} {A : ty0 pos} (s : Γ =[val]> Δ) (k : term Δ `-A)
+  : (Γ ▶ₛ {| sub_elt := `-A ; sub_prf := stt |}) =[val_n]> Δ :=
+  [ s ,ₓ k : val Δ `-A ].
 
-  unshelve eapply (fmap_weq (RY := eqᵢ _) (fun _ : T1 => from_pat_F) (fun _ : T1 => from_pat_F) _ _ _ _) in H.
-  intros [] ? ? ->; auto.
-
-  unfold fmap_delay in H.
-  rewrite 4 fmap_fmap_com in H.
-  rewrite 2 (fmap_eq (RY := eqᵢ _) _ _ (fun _ a b H => from_to_pat_F a b H) _ _ _ (reflexivity _)) in H.
-  rewrite <- 2 (fmap_fmap_com (g := fun _ : T1 => pat_of_nf Δ) (f := fun _ : T1 => n_rename r_from_to_l)) in H.
-  fold (fmap_delay (pat_of_nf Δ)) in H.
-  fold (fmap_delay (n_rename (Δ := Δ) r_from_to_l)) in H.
-  rewrite <- 2 (fmap_comp_eq (clean_hyp_ren _ _)) in H.
-  rewrite 2 s_ren_sub in H.
-  rewrite 2 (s_sub_eq _ _ (from_BB_to_FF σ) _ _ eq_refl) in H.
-  unfold from_to_state in H.
-  rewrite <- 2 s_sub_ren, 2 s_ren_ren in H.
-  rewrite 2 (s_ren_eq _ _ (r_from_to_lr) _ _ eq_refl) in H.
-  rewrite 2 s_ren_id_l in H.
-  exact H.
+Lemma sub_csk {Γ Δ : neg_ctx} {A : ty0 pos} (t : term Γ `+A) (s : Γ =[val]> Δ)
+  (k : term Δ `-A)
+  : Cut _ (t `ₜ⊛ s) k = c_of_t t ₜ⊛ a_of_sk s k.
+Proof.
+  cbn; f_equal; unfold t_shift1; rewrite t_sub_ren; now apply t_sub_eq.
 Qed.
 
-Definition c_of_t_p {Γ : neg_ctx} {x : ty0 pos} (t : term Γ (t+ x)) : state (Γ ▶ₛ {| sub_elt := t- x ; sub_prf := stt |}) :=
-  Cut _ (t_shift _ t) (Whn (Var Ctx.top)) .
-Notation "⟦ t ⟧ₚ" := (interp_act_s _ (c_of_t_p t)) .
+Definition ciu_eq (Δ : neg_ctx) {Γ} {A : ty0 pos} : relation (term Γ `+A) :=
+  fun u v =>
+    forall (σ : Γ =[val]> Δ) (k : term Δ `-A),
+      evalₒ (Cut _ (u `ₜ⊛ σ) k : state_n Δ) ≈ evalₒ (Cut _ (v `ₜ⊛ σ) k : state_n Δ) .
+Notation "x ≈⟦ciu Δ ⟧⁺≈ y" := (ciu_eq Δ x y) (at level 50).
 
-Definition a_of_sk_p {Γ Δ : neg_ctx} {x : ty0 pos} (s : Γ =[val]> Δ) (k : term Δ (t- x))
-  : (Γ ▶ₛ {| sub_elt := t- x ; sub_prf := stt |}) =[val]> Δ :=
-  a_append s (k : val Δ (t- x)) .
-
-Lemma sub_csk_p {Γ Δ : neg_ctx} {x : ty0 pos} (t : term Γ (t+ x)) (s : Γ =[val]> Δ) (k : term Δ (t- x))
-              : Cut _ (t_subst s _ t) k = s_subst (a_of_sk_p s k) (c_of_t_p t) .
-  cbn; f_equal.
-  unfold t_shift; rewrite t_sub_ren.
-  now apply t_sub_eq.
-Qed.
-
-Definition ciu_p_eq (Δ : neg_ctx) {Γ} {x : ty0 pos} : relation (term Γ (t+ x)) :=
-  fun u v => forall (σ : Γ =[val]> Δ) (k : term Δ (t- x)),
-      eval_to_msg (Cut _ (t_subst σ _ u) k) ≈ eval_to_msg (Cut _ (t_subst σ _ v) k) .
-
-Theorem sysD_ciu_p_correct (Δ : neg_ctx) {Γ : neg_ctx} {t} (x y : term Γ (t+ t))
-  : ⟦ x ⟧ₚ ≈[ Δ ]≈ ⟦ y ⟧ₚ -> ciu_p_eq Δ x y .
-  intros H σ k.
-  rewrite 2 sub_csk_p.
-  now apply sysD_subst_correct.
-Qed.
-
-Definition ciu_n_eq (Δ : neg_ctx) {Γ} {x : ty0 neg} : relation (term Γ (t- x)) :=
-  fun u v => forall (σ : Γ =[val]> Δ) (k : term Δ (t+ x)),
-      eval_to_msg (Cut _ k (t_subst σ _ u)) ≈ eval_to_msg (Cut _ k (t_subst σ _ v)) .
-
-Definition c_of_t_n {Γ : neg_ctx} {x : ty0 neg} (t : term Γ (t- x)) : state (Γ ▶ₛ {| sub_elt := t+ x ; sub_prf := stt |}) :=
-  Cut _ (Whn (Var Ctx.top)) (t_shift _ t) .
-Notation "⟦ t ⟧ₙ" := (interp_act_s _ (c_of_t_n t)) .
-
-Definition a_of_sk_n {Γ Δ : neg_ctx} {x : ty0 neg} (s : Γ =[val]> Δ) (k : term Δ (t+ x))
-  : (Γ ▶ₛ {| sub_elt := t+ x ; sub_prf := stt |}) =[val]> Δ :=
-  a_append s (k : val Δ (t+ x)) .
-
-Lemma sub_csk_n {Γ Δ : neg_ctx} {x : ty0 neg} (t : term Γ (t- x)) (s : Γ =[val]> Δ) (k : term Δ (t+ x))
-              : Cut _ k (t_subst s _ t) = s_subst (a_of_sk_n s k) (c_of_t_n t) .
-  cbn; f_equal.
-  unfold t_shift; rewrite t_sub_ren.
-  now apply t_sub_eq.
-Qed.
-
-Theorem sysD_ciu_n_correct (Δ : neg_ctx) {Γ : neg_ctx} {t} (x y : term Γ (t- t))
-  : ⟦ x ⟧ₙ ≈[ Δ ]≈ ⟦ y ⟧ₙ -> ciu_n_eq Δ x y .
-  intros H σ k.
-  rewrite 2 sub_csk_n.
+Theorem ciu_correct (Δ : neg_ctx) {Γ : neg_ctx} {A} (x y : term Γ `+A)
+  : (name⁺ x) ≈⟦ogs Δ ⟧≈ (name⁺ y) -> x ≈⟦ciu Δ ⟧⁺≈ y.
+  intros H σ k; rewrite 2 sub_csk.
   now apply sysD_subst_correct.
 Qed.
